theories/Core/Syntactic/System/Lemmas.v
@@ -3,7 +3,44 @@ From McPTS.Core Require Import Base.
 From McPTS.Core.Syntactic.System Require Import Definitions.
 Import Syntax_Notations.
 
+
 (** ** Basic Context Properties *)
+    
+Lemma functional_gctx_lookup {P} : forall {Δ : gctx P} {A A' x},
+    {{ `#x : A ∈ Δ }} ->
+    {{ `#x : A' ∈ Δ }} ->
+    A = A'.
+Proof.
+  intros * Hx Hx'; gen A'.
+  dependent induction Hx;
+    intros; dependent destruction Hx';
+    intuition.
+Qed.
+
+#[export]
+Hint Resolve functional_gctx_lookup : mcpts.
+ 
+Lemma gctx_decomp {P : PtsSig} : forall {Δ : gctx P} {x A}, {{ ⊢ Δ, x : A }} -> {{ ⊢ Δ }} /\ {{ Δ ; ⋅ ⊢ A }}.
+Proof with now eauto.
+  inversion 1; split; mauto 2.
+Qed.
+
+#[export]
+Hint Resolve gctx_decomp : mcpts.
+
+Corollary gctx_decomp_left {P : PtsSig} : forall {Δ : gctx P} {x A}, {{ ⊢ Δ, x : A }} -> {{ ⊢ Δ }}. 
+Proof with easy.
+  intros * ?%gctx_decomp...
+Qed.
+
+Corollary gctx_decomp_right {P : PtsSig} : forall {Δ : gctx P} {x A}, {{ ⊢ Δ, x : A }} -> {{ Δ ; ⋅ ⊢ A }}.
+Proof with easy.
+  intros * ?%gctx_decomp...
+Qed.
+
+#[export]
+Hint Resolve gctx_decomp_left gctx_decomp_right : mcpts.
+
 
 Lemma ctx_lookup_lt {P : PtsSig} : forall {Γ : ctx P} {A x},
     {{ #x : A ∈ Γ }} ->
@@ -25,7 +62,7 @@ Proof with mautosolve.
     intuition.
 Qed.
 
-Lemma ctx_decomp {P : PtsSig} : forall {Γ : ctx P} {A}, {{ ⊢ Γ, A }} -> {{ ⊢ Γ }} /\ {{ Γ ⊢ A }}.
+Lemma ctx_decomp {P : PtsSig} : forall {Δ : gctx P} {Γ A}, {{ Δ ⊢ Γ, A }} -> {{ Δ ⊢ Γ }} /\ {{ Δ ; Γ ⊢ A }}.
 Proof with now eauto.
   inversion 1; split; mauto 2.
 Qed.
@@ -33,12 +70,12 @@ Qed.
 #[export]
 Hint Resolve ctx_decomp : mcpts.
 
-Corollary ctx_decomp_left {P : PtsSig} : forall {Γ : ctx P} {A}, {{ ⊢ Γ, A }} -> {{ ⊢ Γ }}.
+Corollary ctx_decomp_left {P : PtsSig} : forall {Δ : gctx P} {Γ A}, {{ Δ ⊢ Γ, A }} -> {{ Δ ⊢ Γ }}.
 Proof with easy.
   intros * ?%ctx_decomp...
 Qed.
 
-Corollary ctx_decomp_right {P : PtsSig} : forall {Γ : ctx P} {A}, {{ ⊢ Γ, A }} -> {{ Γ ⊢ A }}.
+Corollary ctx_decomp_right {P : PtsSig} : forall {Δ : gctx P} {Γ A}, {{ Δ ⊢ Γ, A }} -> {{ Δ ; Γ ⊢ A }}.
 Proof with easy.
   intros * ?%ctx_decomp...
 Qed.
@@ -46,833 +83,693 @@ Qed.
 #[export]
 Hint Resolve ctx_decomp_left ctx_decomp_right : mcpts.
 
-(** ** Core Presuppositions *)
 
-(** *** Context Presuppositions *)
 
-Lemma presup_ctx_eq {P : PtsSig} : forall {Γ Δ : ctx P}, {{ ⊢ Γ ≈ Δ }} -> {{ ⊢ Γ }} /\ {{ ⊢ Δ }}.
+(** * Core presupposition results *)
+
+(** For equality of global contexts *)
+Lemma presup_gctx_eq {P} : forall {Δ Δ' : gctx P}, {{ ⊢ Δ ≈ Δ' }} -> {{ ⊢ Δ }} /\ {{ ⊢ Δ' }}.
 Proof with mautosolve.
   induction 1; destruct_pairs...
 Qed.
 
-Corollary presup_ctx_eq_left {P : PtsSig} : forall {Γ Δ : ctx P}, {{ ⊢ Γ ≈ Δ }} -> {{ ⊢ Γ }}.
+Corollary presup_gctx_eq_left {P} : forall {Δ Δ' : gctx P}, {{ ⊢ Δ ≈ Δ' }} -> {{ ⊢ Δ }}.
 Proof with easy.
-  intros * ?%presup_ctx_eq...
+  intros * ?%presup_gctx_eq...
 Qed.
 
-Corollary presup_ctx_eq_right {P : PtsSig} : forall {Γ Δ : ctx P}, {{ ⊢ Γ ≈ Δ }} -> {{ ⊢ Δ }}.
+Corollary presup_gctx_eq_right {P} : forall {Δ Δ' : gctx P}, {{ ⊢ Δ ≈ Δ' }} -> {{ ⊢ Δ' }}.
 Proof with easy.
-  intros * ?%presup_ctx_eq...
+  intros * ?%presup_gctx_eq...
 Qed.
 
 #[export]
-Hint Resolve presup_ctx_eq presup_ctx_eq_left presup_ctx_eq_right : mcpts.
+Hint Resolve presup_gctx_eq presup_gctx_eq_left presup_gctx_eq_right : mcpts.
 
-Lemma presup_sub {P : PtsSig} : forall {Γ : ctx P} {Δ σ}, {{ Γ ⊢s σ : Δ }} -> {{ ⊢ Γ }} /\ {{ ⊢ Δ }}.
+(** For subtyping of global contexts *)
+Lemma presup_gctx_subtyp {P} : forall {Δ Δ' : gctx P}, {{ ⊢ Δ ⊆ Δ' }} -> {{ ⊢ Δ }} /\ {{ ⊢ Δ' }}.
 Proof with mautosolve.
   induction 1; destruct_pairs...
 Qed.
 
-Corollary presup_sub_left {P : PtsSig} : forall {Γ : ctx P} {Δ σ}, {{ Γ ⊢s σ : Δ }} -> {{ ⊢ Γ }}.
+Corollary presup_gctx_subtyp_left {P} : forall {Δ Δ' : gctx P}, {{ ⊢ Δ ⊆ Δ' }} -> {{ ⊢ Δ }}.
 Proof with easy.
-  intros * ?%presup_sub...
+  intros * ?%presup_gctx_subtyp...
 Qed.
 
-Corollary presup_sub_right {P : PtsSig} : forall {Γ : ctx P} {Δ σ}, {{ Γ ⊢s σ : Δ }} -> {{ ⊢ Δ }}.
+Corollary presup_gctx_subtyp_right {P} : forall {Δ Δ' : gctx P}, {{ ⊢ Δ ⊆ Δ' }} -> {{ ⊢ Δ' }}.
 Proof with easy.
-  intros * ?%presup_sub...
+  intros * ?%presup_gctx_subtyp...
 Qed.
 
 #[export]
-Hint Resolve presup_sub presup_sub_left presup_sub_right : mcpts.
+Hint Resolve presup_gctx_subtyp presup_gctx_subtyp_left presup_gctx_subtyp_right : mcpts.
 
-(** With [presup_sub], we can prove similar for [exp]. *)
-
-Lemma presup_exp_ctx {P : PtsSig} : forall {Γ : ctx P} {M A}, {{ Γ ⊢ M : A }} -> {{ ⊢ Γ }}.
+(** For well-formedness of local contexts *)
+Lemma presup_wf_ctx {P : PtsSig} : forall {Δ : gctx P} {Γ : ctx P}, {{ Δ ⊢ Γ }} -> {{ ⊢ Δ }}.
 Proof with mautosolve.
   induction 1...
 Qed.
 
 #[export]
-Hint Resolve presup_exp_ctx : mcpts.
-
-Lemma presup_typ {P} : forall {Γ : ctx P} {A}, {{ Γ ⊢ A }} -> {{ ⊢ Γ }}.
-Proof with mautosolve.
-  induction 1...
-Qed.
-
-#[export]
-Hint Resolve presup_typ : mcpts.
-
-(** and other presuppositions about context well-formedness. *)
-
-Lemma presup_sub_eq_ctx {P : PtsSig} : forall {Γ : ctx P} {Δ σ σ'}, {{ Γ ⊢s σ ≈ σ' : Δ }} -> {{ ⊢ Γ }} /\ {{ ⊢ Δ }}.
-Proof with mautosolve.
-  induction 1; split; destruct_pairs; mauto 3.
-Qed.
-
-Corollary presup_sub_eq_ctx_left {P : PtsSig} : forall {Γ : ctx P} {Δ σ σ'}, {{ Γ ⊢s σ ≈ σ' : Δ }} -> {{ ⊢ Γ }}.
-Proof with easy.
-  intros * ?%presup_sub_eq_ctx...
-Qed.
-
-Corollary presup_sub_eq_ctx_right {P : PtsSig} : forall {Γ : ctx P} {Δ σ σ'}, {{ Γ ⊢s σ ≈ σ' : Δ }} -> {{ ⊢ Δ }}.
-Proof with easy.
-  intros * ?%presup_sub_eq_ctx...
-Qed.
-
-#[export]
-Hint Resolve presup_sub_eq_ctx presup_sub_eq_ctx_left presup_sub_eq_ctx_right : mcpts.
-
-Lemma presup_exp_eq_ctx {P : PtsSig} : forall {Γ : ctx P} {M M' A}, {{ Γ ⊢ M ≈ M' : A }} -> {{ ⊢ Γ }}.
-Proof with mautosolve 2.
-  induction 1...
-Qed.
-
-#[export]
-Hint Resolve presup_exp_eq_ctx : mcpts.
-  
-Lemma presup_typ_eq_ctx {P : PtsSig} : forall {Γ : ctx P} {A A'}, {{ Γ ⊢ A ≈ A' }} -> {{ ⊢ Γ }}.
-Proof with mautosolve 2.
-  induction 1...
-Qed.
-
-#[export]
-Hint Resolve presup_exp_eq_ctx : mcpts.
-
-
-Lemma presup_subtyp_ctx {P} : forall {Γ : ctx P} {A A'}, {{ Γ ⊢ A ⊆ A' }} -> {{ ⊢ Γ }}.
-Proof with mautosolve 2.
-  induction 1...
-Qed.
-
-#[export]
-Hint Resolve presup_subtyp_ctx : mcpts.
+Hint Resolve presup_wf_ctx : mcpts.
  
-Lemma presup_wf_ctx_sub {P} : forall {Γ Δ : ctx P},
-    {{ ⊢ Γ ⊆ Δ }} -> {{ ⊢ Γ }} /\ {{ ⊢ Δ }}.
-Proof with mautosolve 2.  
-  induction 1; split; destruct_conjs; mauto 2.
+(** For equality of local contexts *)
+Lemma presup_wf_ctx_eq {P : PtsSig} : forall {Δ : gctx P} {Γ Γ' : ctx P}, {{ Δ ⊢ Γ ≈ Γ' }} -> {{ ⊢ Δ }} /\ {{ Δ ⊢ Γ }} /\ {{ Δ ⊢ Γ' }}.
+Proof with mautosolve.
+  induction 1; destruct_pairs...
 Qed.
 
-Lemma presup_wf_ctx_sub_left {P} : forall {Γ Δ : ctx P},
-    {{ ⊢ Γ ⊆ Δ }} -> {{ ⊢ Γ }}.
+Corollary presup_wf_ctx_eq_gctx {P : PtsSig} : forall {Δ : gctx P} {Γ Γ' : ctx P}, {{ Δ ⊢ Γ ≈ Γ' }} -> {{ ⊢ Δ }}.
+Proof with easy.
+  intros * ?%presup_wf_ctx_eq...
+Qed.
+
+Corollary presup_wf_ctx_eq_left {P : PtsSig} : forall {Δ : gctx P} {Γ Γ' : ctx P}, {{ Δ ⊢ Γ ≈ Γ' }} -> {{ Δ ⊢ Γ }}.
+Proof with easy.
+  intros * ?%presup_wf_ctx_eq...
+Qed.
+
+Corollary presup_wf_ctx_eq_right {P : PtsSig} : forall {Δ : gctx P} {Γ Γ' : ctx P}, {{ Δ ⊢ Γ ≈ Γ' }} -> {{ Δ ⊢ Γ' }}.
+Proof with easy.
+  intros * ?%presup_wf_ctx_eq...
+Qed.
+
+#[export]
+Hint Resolve presup_wf_ctx_eq presup_wf_ctx_eq_gctx presup_wf_ctx_eq_left presup_wf_ctx_eq_right : mcpts.
+
+(** For subtyping of local contexts *)
+Lemma presup_ctx_subtyp {P} : forall {Δ : gctx P} {Γ Γ' : ctx P}, {{ Δ ⊢ Γ ⊆ Γ' }} -> {{ ⊢ Δ }} /\ {{ Δ ⊢ Γ }} /\ {{ Δ ⊢ Γ' }}.
 Proof with mautosolve.
-  intros * []%presup_wf_ctx_sub...
+  induction 1; destruct_pairs...
+Qed.
+
+Corollary presup_ctx_subtyp_gctx {P} : forall {Δ : gctx P} {Γ Γ' : ctx P}, {{ Δ ⊢ Γ ⊆ Γ' }} -> {{ ⊢ Δ }}.
+Proof with easy.
+  intros * ?%presup_ctx_subtyp...
+Qed.
+
+Corollary presup_ctx_subtyp_left {P} : forall {Δ : gctx P} {Γ Γ' : ctx P}, {{ Δ ⊢ Γ ⊆ Γ' }} -> {{ Δ ⊢ Γ }}.
+Proof with easy.
+  intros * ?%presup_ctx_subtyp...
+Qed.
+
+Corollary presup_ctx_subtyp_right {P} : forall {Δ : gctx P} {Γ Γ' : ctx P}, {{ Δ ⊢ Γ ⊆ Γ' }} -> {{ Δ ⊢ Γ' }}.
+Proof with easy.
+  intros * ?%presup_ctx_subtyp...
+Qed.
+
+#[export]
+Hint Resolve presup_ctx_subtyp presup_ctx_subtyp_gctx presup_ctx_subtyp_left presup_ctx_subtyp_right : mcpts.
+
+
+
+(** For subtyping of types *)
+Lemma presup_typ_subtyp_right {P} : forall {Δ : gctx P} {Γ : ctx P} {A B}, {{ Δ ; Γ ⊢ A ⊆ B }} -> {{ Δ ; Γ ⊢ B }}.
+Proof with mautosolve.
+  induction 1...
+Qed.
+
+#[export]
+Hint Resolve presup_typ_subtyp_right : mcpts.
+
+
+(** ** Context Presuppositions *)
+
+(** For well-formedness of substitutions *)
+Lemma presup_sub {P : PtsSig} : forall {Δ : gctx P} {Γ Γ' σ}, {{ Δ ; Γ ⊢s σ : Γ' }} -> {{ ⊢ Δ }} /\ {{ Δ ⊢ Γ }} /\ {{ Δ ⊢ Γ' }}.
+Proof with mautosolve.
+  induction 1; destruct_pairs...
+Qed.
+
+Corollary presup_sub_gctx {P : PtsSig} : forall {Δ : gctx P} {Γ Γ' σ}, {{ Δ ; Γ ⊢s σ : Γ' }} -> {{ ⊢ Δ }}.
+Proof with easy.
+  intros * ?%presup_sub...
 Qed.
   
-Lemma presup_wf_ctx_sub_right {P} : forall {Γ Δ : ctx P},
-    {{ ⊢ Γ ⊆ Δ }} -> {{ ⊢ Δ }}.
+Corollary presup_sub_left {P : PtsSig} : forall {Δ : gctx P} {Γ Γ' σ}, {{ Δ ; Γ ⊢s σ : Γ' }} -> {{ Δ ⊢ Γ }}.
+Proof with easy.
+  intros * ?%presup_sub...
+Qed.
+
+Corollary presup_sub_right {P : PtsSig} : forall {Δ : gctx P} {Γ Γ' σ}, {{ Δ ; Γ ⊢s σ : Γ' }} -> {{ Δ ⊢ Γ' }}.
+Proof with easy.
+  intros * ?%presup_sub...
+Qed.
+
+#[export]
+Hint Resolve presup_sub presup_sub_gctx presup_sub_left presup_sub_right : mcpts.
+
+
+(** For well-formedness of expressions *)
+Lemma presup_exp_gctx_ctx {P : PtsSig} : forall {Δ : gctx P} {Γ M A}, {{ Δ ; Γ ⊢ M : A }} -> {{ ⊢ Δ }} /\ {{ Δ ⊢ Γ }}.
 Proof with mautosolve.
-  intros * []%presup_wf_ctx_sub...
+  induction 1...
 Qed.
 
+Corollary presup_exp_gctx {P : PtsSig} : forall {Δ : gctx P} {Γ M A}, {{ Δ ; Γ ⊢ M : A }} -> {{ ⊢ Δ }}.
+Proof with easy.
+  intros * ?%presup_exp_gctx_ctx...
+Qed.
 
-(** *** Immediate Results of Context Presuppositions *)
-Lemma wf_ctx_sub_refl {P} : forall (Γ Δ : ctx P),
-    {{ ⊢ Γ ≈ Δ }} ->
-    {{ ⊢ Γ ⊆ Δ }}.
-Proof. induction 1; mauto. Qed.
-
-#[export]
-Hint Resolve wf_ctx_sub_refl : mcpts.
-
-
-(** Equality-based conversions *)
-Lemma wf_conv_sorted {P} : forall (Γ : ctx P) M A s A',
-    {{ Γ ⊢ M : A }} ->
-    (** The next two arguments will be removed in SystemOpt *)
-    {{ Γ ⊢ A : Sort@s }} -> 
-    {{ Γ ⊢ A' : Sort@s }} ->
-    {{ Γ ⊢ A ≈ A' : Sort@s }} ->
-    {{ Γ ⊢ M : A' }}.
-Proof.
-  intros.
-  assert {{ Γ ⊢ A }} by mauto 2.
-  assert {{ Γ ⊢ A' }} by mauto 2.
-  mauto.
+Corollary presup_exp_ctx {P : PtsSig} : forall {Δ : gctx P} {Γ M A}, {{ Δ ; Γ ⊢ M : A }} -> {{ Δ ⊢ Γ }}.
+Proof with easy.
+  intros * ?%presup_exp_gctx_ctx...
 Qed.
 
 #[export]
-Hint Resolve wf_conv_sorted : mcpts.
+Hint Resolve presup_exp_gctx_ctx presup_exp_gctx presup_exp_ctx : mcpts.
 
-Lemma wf_conv {P} : forall (Γ : ctx P) M A A',
-    {{ Γ ⊢ M : A }} ->
-    (** The next two arguments will be removed in SystemOpt *)
-    {{ Γ ⊢ A }} ->
-    {{ Γ ⊢ A' }} ->
-    {{ Γ ⊢ A ≈ A'  }} ->
-    {{ Γ ⊢ M : A' }}.
-Proof. mauto. Qed.
+(** For well-formedness of types *)
+Lemma presup_typ {P} : forall {Δ : gctx P} {Γ A}, {{ Δ ; Γ ⊢ A }} -> {{ ⊢ Δ }} /\ {{ Δ ⊢ Γ }}.
+Proof with mautosolve.
+  induction 1...
+Qed.
 
-#[export]
-Hint Resolve wf_conv : mcpts.
+Corollary presup_typ_gctx {P} : forall {Δ : gctx P} {Γ A}, {{ Δ ; Γ ⊢ A }} -> {{ ⊢ Δ }}.
+Proof with easy.
+  intros * ?%presup_typ...
+Qed.
 
-
-Lemma wf_sub_conv_eq {P : PtsSig} : forall (Γ : ctx P) σ Δ Δ',
-  {{ Γ ⊢s σ : Δ }} ->
-  {{ ⊢ Δ ≈ Δ' }} ->
-  {{ Γ ⊢s σ : Δ' }}.
-Proof.
-  intros.
-  assert {{ ⊢ Δ' }} by (eapply presup_ctx_eq; eassumption).
-  eapply wf_sub_conv; mauto.
+Corollary presup_typ_ctx {P} : forall {Δ : gctx P} {Γ A}, {{ Δ ; Γ ⊢ A }} -> {{ Δ ⊢ Γ }}.
+Proof with easy.
+  intros * ?%presup_typ...
 Qed.
 
 #[export]
-Hint Resolve wf_sub_conv_eq : mcpts.
+Hint Resolve presup_typ presup_typ_gctx presup_typ_ctx : mcpts.
 
-Lemma wf_exp_eq_sort_subtyp {P} : forall {Γ : ctx P} {A B s},
-    {{ Γ ⊢ A ≈ B : Sort@s }} ->
-    {{ Γ ⊢ B }} ->
-    {{ Γ ⊢ A ⊆ B }}.
-Proof.
-  intros.
-  assert {{ Γ ⊢ A ≈ B }} by mauto 2.
-  mauto 2.
+
+(** For equality of substitutions *)
+Lemma presup_sub_eq_gctx_ctx {P : PtsSig} : forall {Δ : gctx P} {Γ Γ' σ σ'}, {{ Δ ; Γ ⊢s σ ≈ σ' : Γ' }} -> {{ ⊢ Δ }} /\ {{ Δ ⊢ Γ }} /\ {{ Δ ⊢ Γ' }}.
+Proof with mautosolve.
+  induction 1; destruct_pairs...
+Qed.
+
+Corollary presup_sub_eq_gctx {P : PtsSig} : forall {Δ : gctx P} {Γ Γ' σ σ'}, {{ Δ ; Γ ⊢s σ ≈ σ' : Γ' }} -> {{ ⊢ Δ }}.
+Proof with easy.
+  intros * ?%presup_sub_eq_gctx_ctx...
+Qed.
+
+Corollary presup_sub_eq_ctx_left {P : PtsSig} : forall {Δ : gctx P} {Γ Γ' σ σ'}, {{ Δ ; Γ ⊢s σ ≈ σ' : Γ' }} -> {{ Δ ⊢ Γ }}.
+Proof with easy.
+  intros * ?%presup_sub_eq_gctx_ctx...
+Qed.
+
+Corollary presup_sub_eq_ctx_right {P : PtsSig} : forall {Δ : gctx P} {Γ Γ' σ σ'}, {{ Δ ; Γ ⊢s σ ≈ σ' : Γ' }} -> {{ Δ ⊢ Γ' }}.
+Proof with easy.
+  intros * ?%presup_sub_eq_gctx_ctx...
 Qed.
 
 #[export]
-Hint Resolve wf_exp_eq_sort_subtyp : mcpts.
+Hint Resolve presup_sub_eq_gctx_ctx presup_sub_eq_gctx presup_sub_eq_ctx_left presup_sub_eq_ctx_right : mcpts.
 
-Lemma wf_eq_conv_sorted {P} : forall (Γ : ctx P) M M' A s A',
-    {{ Γ ⊢ M ≈ M' : A }} ->
-    (** The next two arguments will be removed in SystemOpt *)
-    {{ Γ ⊢ A : Sort@s }} -> 
-    {{ Γ ⊢ A' : Sort@s }} ->
-    {{ Γ ⊢ A ≈ A' : Sort@s }} ->
-    {{ Γ ⊢ M ≈ M' : A' }}.
-Proof. mauto. Qed. 
-
-#[export]
-Hint Resolve wf_eq_conv_sorted : mcpts.
-
-Lemma wf_eq_conv {P} : forall (Γ : ctx P) M M' A A',
-    {{ Γ ⊢ M ≈ M' : A }} ->
-    (** The next two arguments will be removed in SystemOpt *)
-    {{ Γ ⊢ A }} -> 
-    {{ Γ ⊢ A' }} ->
-    {{ Γ ⊢ A ≈ A' }} ->
-    {{ Γ ⊢ M ≈ M' : A' }}.
-Proof. mauto. Qed. 
-
-#[export]
-Hint Resolve wf_eq_conv : mcpts.
-
-
-Lemma wf_sub_eq_conv_eq {P : PtsSig} : forall (Γ : ctx P) σ σ' Δ Δ',
-    {{ Γ ⊢s σ ≈ σ' : Δ }} ->
-    {{ ⊢ Δ ≈ Δ' }} ->
-    {{ Γ ⊢s σ ≈ σ' : Δ' }}.
-Proof. mauto. Qed.
-
-#[export]
-Hint Resolve wf_sub_eq_conv_eq : mcpts.
-
-Add Parametric Morphism {P : PtsSig} (Γ : ctx P) : (wf_sub_eq Γ)
-    with signature wf_ctx_eq ==> eq ==> eq ==> iff as wf_sub_eq_morphism_iff3.
-Proof.
-  intros Δ Δ' H **; split; [| symmetry in H]; mauto.
+(** For equality of expressions *)
+Lemma presup_exp_eq_gctx_ctx {P : PtsSig} : forall {Δ : gctx P} {Γ M M' A}, {{ Δ ; Γ ⊢ M ≈ M' : A }} -> {{ ⊢ Δ }} /\ {{ Δ ⊢ Γ }}.
+Proof with mautosolve 2.
+  induction 1; destruct_pairs; split...
 Qed.
 
-(** We can prove some additional lemmas for type presuppositions as well. *)
+Corollary presup_exp_eq_gctx {P : PtsSig} : forall {Δ : gctx P} {Γ M M' A}, {{ Δ ; Γ ⊢ M ≈ M' : A }} -> {{ ⊢ Δ }}.
+Proof with easy.
+  intros * ?%presup_exp_eq_gctx_ctx...
+Qed.
 
-
-(** *** Additional Lemmas for Syntactic PERs *)
-
-Lemma exp_eq_refl {P : PtsSig} : forall {Γ : ctx P} {M A},
-    {{ Γ ⊢ M : A }} ->
-    {{ Γ ⊢ M ≈ M : A }}.
-Proof. mauto. Qed.
-
-#[export]
-Hint Resolve exp_eq_refl : mcpts.
-
-Lemma sub_eq_refl {P : PtsSig} : forall {Γ : ctx P} {σ Δ},
-    {{ Γ ⊢s σ : Δ }} ->
-    {{ Γ ⊢s σ ≈ σ : Δ }}.
-Proof. mauto. Qed.
-
-#[export]
-Hint Resolve sub_eq_refl : mcpts.
-
-Lemma ctx_eq_refl {P : PtsSig} : forall {Γ : ctx P},
-    {{ ⊢ Γ }} ->
-    {{ ⊢ Γ ≈ Γ }}.
-Proof.
-  induction 1; mauto 2.
-  econstructor; mauto 3.
+Corollary presup_exp_eq_ctx {P : PtsSig} : forall {Δ : gctx P} {Γ M M' A}, {{ Δ ; Γ ⊢ M ≈ M' : A }} -> {{ Δ ⊢ Γ }}.
+Proof with easy.
+  intros * ?%presup_exp_eq_gctx_ctx...
 Qed.
 
 #[export]
-Hint Resolve ctx_eq_refl : mcpts.
+Hint Resolve presup_exp_eq_gctx_ctx presup_exp_eq_gctx presup_exp_eq_ctx : mcpts.
 
-(** *** Lemmas for [exp] of [{{{ Sort@s }}}] *)
-Lemma wf_exp_sort_sub {P} : forall {Γ Γ' : ctx P} {A σ s},
-    {{ Γ ⊢s σ : Γ' }} ->
-    {{ Γ' ⊢ A : Sort@s }} ->
-    {{ Γ ⊢ A[σ] : Sort@s }}.
-Proof.
-  intros.
-  assert {{ Γ ⊢ A[σ] : Sort@s[σ] }} by mauto 4.
-  assert {{ ⊢ Γ }} by mauto 2.
-  assert {{ Γ ⊢ Sort@s[σ] ≈ Sort@s }} by mauto 3.
-  assert {{ Γ ⊢ Sort@s[σ] ⊆ Sort@s }} by mauto 3.
-  econstructor; mauto 3.
-  solve [econstructor; mauto 3].
+(** For equality of types *)
+Lemma presup_typ_eq_gctx_ctx {P : PtsSig} : forall {Δ : gctx P} {Γ A A'}, {{ Δ ; Γ ⊢ A ≈ A' }} -> {{ ⊢ Δ }} /\ {{ Δ ⊢ Γ }}.
+Proof with mautosolve 2.
+  induction 1; destruct_pairs; split...
+Qed.
+
+Corollary presup_typ_eq_gctx {P : PtsSig} : forall {Δ : gctx P} {Γ A A'}, {{ Δ ; Γ ⊢ A ≈ A' }} -> {{ ⊢ Δ }}.
+Proof with easy.
+  intros * ?%presup_typ_eq_gctx_ctx...
+Qed.
+
+Corollary presup_typ_eq_ctx {P : PtsSig} : forall {Δ : gctx P} {Γ A A'}, {{ Δ ; Γ ⊢ A ≈ A' }} -> {{ Δ ⊢ Γ }}.
+Proof with easy.
+  intros * ?%presup_typ_eq_gctx_ctx...
 Qed.
 
 #[export]
-Hint Resolve wf_exp_sort_sub : mcpts.
+Hint Resolve presup_exp_eq_gctx_ctx presup_exp_eq_gctx presup_exp_eq_ctx : mcpts.
 
+(** For subtyping of types *)
+Lemma presup_typ_subtyp_gctx_ctx {P} : forall {Δ : gctx P} {Γ A A'}, {{ Δ ; Γ ⊢ A ⊆ A' }} -> {{ ⊢ Δ }} /\ {{ Δ ⊢ Γ }}.
+Proof with mautosolve 2.
+  induction 1; destruct_pairs; mauto 2.
+  split; mauto 2.
+Qed.
 
-Lemma exp_eq_sub_compose_typ_sort {P} : forall {Γ Γ' Γ'' : ctx P} {A A' σ τ s},
-    {{ Γ'' ⊢ A' : Sort@s }} ->
-    {{ Γ'' ⊢ A ≈ A' : Sort@s }} ->
-    {{ Γ' ⊢s σ : Γ'' }} ->
-    {{ Γ ⊢s τ : Γ' }} ->
-    {{ Γ ⊢ A[σ∘τ] ≈ A'[σ][τ] : Sort@s }}.
-Proof.
-  intros.
-  assert {{ Γ ⊢ Sort@s[σ∘τ] ≈ Sort@s }} by mauto.
-  assert {{ Γ ⊢ Sort@s[σ∘τ] ⊆ Sort@s }} by mauto.
-  assert {{ Γ ⊢ A'[σ∘τ] ≈ A'[σ][τ] : Sort@s[σ∘τ] }} by mauto 4.    
-  transitivity {{{ A'[σ∘τ] }}}; mauto 4.
-  assert {{ Γ ⊢s σ∘τ ≈ σ∘τ : Γ'' }} by mauto.
-  assert {{ Γ ⊢ A[σ∘τ] ≈ A'[σ∘τ] : Sort@s[σ∘τ] }} by mauto 4.
-  mauto.                              
+Corollary presup_typ_subtyp_gctx {P} : forall {Δ : gctx P} {Γ A A'}, {{ Δ ; Γ ⊢ A ⊆ A' }} -> {{ ⊢ Δ }}.
+Proof with easy.
+  intros * ?%presup_typ_subtyp_gctx_ctx...
+Qed.
+
+Corollary presup_typ_subtyp_ctx {P} : forall {Δ : gctx P} {Γ A A'}, {{ Δ ; Γ ⊢ A ⊆ A' }} -> {{ Δ ⊢ Γ }}.
+Proof with easy.
+  intros * ?%presup_typ_subtyp_gctx_ctx...
 Qed.
 
 #[export]
-  Hint Resolve exp_eq_sub_compose_typ_sort : mcpts.
+Hint Resolve presup_typ_subtyp_gctx_ctx presup_typ_subtyp_gctx presup_typ_subtyp_ctx : mcpts.
 
-Lemma presup_ctx_lookup_typ {P : PtsSig} : forall {Γ : ctx P} {A x},
-    {{ ⊢ Γ }} ->
+(** Presupposition for context lookups *)    
+Lemma presup_ctx_lookup_typ {P : PtsSig} : forall {Δ : gctx P} {Γ A x},
+    {{ Δ ⊢ Γ }} ->
     {{ #x : A ∈ Γ }} ->
-    {{ Γ ⊢ A }}.
+    {{ Δ ; Γ ⊢ A }}.
 Proof with mautosolve 4.
   intros * HΓ.
   induction 1; inversion_clear HΓ.
-  - assert {{ Γ, A ⊢s Wk : Γ }} by mauto 3.
+  - assert {{ Δ ; Γ, A ⊢s Wk : Γ }} by mauto 3.
     eapply wf_typ_sub_sort; mauto 2.
-  - assert {{ Γ, B ⊢s Wk : Γ }} by mauto 3.
-    assert {{ Γ ⊢ A  }} by (eapply IHctx_lookup; eauto).
+  - assert {{ Δ ; Γ, B ⊢s Wk : Γ }} by mauto 3.
+    assert {{ Δ ; Γ ⊢ A  }} by mauto 2.
     eapply wf_typ_sub_sort; mauto 2.
 Qed.
 
 #[export]
 Hint Resolve presup_ctx_lookup_typ : mcpts.
 
-(** This removes the extra premise {{ Γ ⊢ A : Sort@s }} in wf_vlookup, which we use in soundness *)
-Corollary wf_vlookup' {P} : forall {Γ : ctx P} {x A},
-    {{ ⊢ Γ }} ->
-    {{ #x : A ∈ Γ }} ->
-    {{ Γ ⊢ #x : A }}.
+Lemma gctx_lookup_var_not_eq_fresh_var {P : PtsSig} : forall {Δ : gctx P} {x x' A},
+    {{ `#x : A ∈ Δ }} ->
+    {{ `#x' ∉ Δ }} ->
+    x <> x'.
 Proof.
-  intros.
-  assert {{ Γ ⊢ A }} by mauto 2.
-  econstructor; mauto 2.
+  induction 1; inversion_clear 1; intuition.
 Qed.
 
 #[export]
-Hint Resolve wf_vlookup' : mcpts.
+Hint Resolve gctx_lookup_var_not_eq_fresh_var : mcpts.
+
+Lemma gctx_weakening {P : PtsSig} :
+  (forall (Δ : gctx P), {{ ⊢ Δ }} -> forall x B, {{ ⊢ Δ, x:B }} -> {{ ⊢ Δ, x:B }}) /\
+    (forall (Δ : gctx P) Γ, {{ Δ ⊢ Γ }} -> forall x B, {{ ⊢ Δ, x:B }} -> {{ Δ, x:B ⊢ Γ }}) /\
+    (forall (Δ : gctx P) Γ Γ', {{ Δ ⊢ Γ ⊆ Γ' }} -> forall x B, {{ ⊢ Δ, x:B }} -> {{ Δ, x:B ⊢ Γ ⊆ Γ' }}) /\
+    (forall (Δ : gctx P) Γ A M, {{ Δ ; Γ ⊢ M : A }} -> forall x B, {{ ⊢ Δ, x:B }} -> {{ Δ, x:B ; Γ ⊢ M : A }}) /\
+    (forall (Δ : gctx P) Γ A M M', {{ Δ ; Γ ⊢ M ≈ M' : A }} -> forall x B, {{ ⊢ Δ, x:B }} -> {{ Δ, x:B ; Γ ⊢ M ≈ M' : A }}) /\
+    (forall (Δ : gctx P) Γ A, {{ Δ ; Γ ⊢ A }} -> forall x B, {{ ⊢ Δ, x:B }} -> {{ Δ, x:B ; Γ ⊢ A }}) /\
+    (forall (Δ : gctx P) Γ A A', {{ Δ ; Γ ⊢ A ≈ A' }} -> forall x B, {{ ⊢ Δ, x:B }} -> {{ Δ, x:B ; Γ ⊢ A ≈ A' }}) /\
+    (forall (Δ : gctx P) Γ A A', {{ Δ ; Γ ⊢ A ⊆ A' }} -> forall x B, {{ ⊢ Δ, x:B }} -> {{ Δ, x:B ; Γ ⊢ A ⊆ A' }}) /\
+    (forall (Δ : gctx P) Γ Γ' σ, {{ Δ ; Γ ⊢s σ : Γ' }} -> forall x B, {{ ⊢ Δ, x:B }} -> {{ Δ, x:B ; Γ ⊢s σ : Γ' }}) /\
+    (forall (Δ : gctx P) Γ Γ' σ σ', {{ Δ ; Γ ⊢s σ ≈ σ' : Γ' }} -> forall x B, {{ ⊢ Δ, x:B }} -> {{ Δ, x:B ; Γ ⊢s σ ≈ σ' : Γ' }}).
+Proof.
+  apply syntactic_wf_mut_ind;
+    intros;
+    try mauto 2;
+    try solve [econstructor; mauto 3].
+
+  - inversion_clear H0.
+    econstructor; mauto 3.
+  - mautosolve.
+  - inversion_clear H0.
+    econstructor; mauto 3.
+  - inversion_clear H0.
+    econstructor; mauto 3.
+Qed.      
+
+Corollary wf_ctx_gctx_weakening {P : PtsSig} : forall {Δ : gctx P} {Γ},
+    {{ Δ ⊢ Γ }} -> forall x B, {{ ⊢ Δ, x:B }} -> {{ Δ, x:B ⊢ Γ }}.
+Proof. intros; eapply gctx_weakening; mauto 2. Qed.
+
+Corollary wf_ctx_subtyp_gctx_weakening {P : PtsSig} : forall {Δ : gctx P} {Γ Γ'}, {{ Δ ⊢ Γ ⊆ Γ' }} -> forall x B, {{ ⊢ Δ, x:B }} -> {{ Δ, x:B ⊢ Γ ⊆ Γ' }}.
+Proof. intros; eapply gctx_weakening; mauto 2. Qed.
+
+Corollary wf_exp_gctx_weakening {P : PtsSig} : forall {Δ : gctx P} {Γ A M}, {{ Δ ; Γ ⊢ M : A }} -> forall x B, {{ ⊢ Δ, x:B }} -> {{ Δ, x:B ; Γ ⊢ M : A }}.
+Proof. intros; eapply gctx_weakening; mauto 2. Qed.
+
+Corollary wf_exp_eq_gctx_weakening {P : PtsSig} : forall {Δ : gctx P} {Γ A M M'}, {{ Δ ; Γ ⊢ M ≈ M' : A }} -> forall x B, {{ ⊢ Δ, x:B }} -> {{ Δ, x:B ; Γ ⊢ M ≈ M' : A }}.
+Proof. intros; eapply gctx_weakening; mauto 2. Qed.
+
+Corollary wf_typ_gctx_weakening {P : PtsSig} : forall {Δ : gctx P} {Γ A}, {{ Δ ; Γ ⊢ A }} -> forall x B, {{ ⊢ Δ, x:B }} -> {{ Δ, x:B ; Γ ⊢ A }}.
+Proof. intros; eapply gctx_weakening; mauto 2. Qed.
+  
+Corollary wf_typ_eq_gctx_weakening {P : PtsSig} : forall {Δ : gctx P} {Γ A A'}, {{ Δ ; Γ ⊢ A ≈ A' }} -> forall x B, {{ ⊢ Δ, x:B }} -> {{ Δ, x:B ; Γ ⊢ A ≈ A' }}.
+Proof. intros; eapply gctx_weakening; mauto 2. Qed.
+
+Corollary wf_typ_subtyp_gctx_weakening {P : PtsSig} :  forall {Δ : gctx P} {Γ A A'}, {{ Δ ; Γ ⊢ A ⊆ A' }} -> forall x B, {{ ⊢ Δ, x:B }} -> {{ Δ, x:B ; Γ ⊢ A ⊆ A' }}.
+Proof. intros; eapply gctx_weakening; mauto 2. Qed.
+
+Corollary wf_sub_gctx_weakening {P : PtsSig} : forall {Δ : gctx P} {Γ Γ' σ}, {{ Δ ; Γ ⊢s σ : Γ' }} -> forall x B, {{ ⊢ Δ, x:B }} -> {{ Δ, x:B ; Γ ⊢s σ : Γ' }}.
+Proof. intros; eapply gctx_weakening; mauto 2. Qed.
+
+Corollary wf_sub_eq_gctx_weakening {P : PtsSig} : forall {Δ : gctx P} {Γ Γ' σ σ'}, {{ Δ ; Γ ⊢s σ ≈ σ' : Γ' }} -> forall x B, {{ ⊢ Δ, x:B }} -> {{ Δ, x:B ; Γ ⊢s σ ≈ σ' : Γ' }}.
+Proof. intros; eapply gctx_weakening; mauto 2. Qed.
+
+#[export]  
+Hint Resolve wf_ctx_gctx_weakening wf_ctx_subtyp_gctx_weakening wf_exp_gctx_weakening wf_exp_eq_gctx_weakening wf_typ_gctx_weakening wf_typ_eq_gctx_weakening wf_typ_subtyp_gctx_weakening wf_sub_gctx_weakening wf_sub_eq_gctx_weakening : mcpts.
+  
+Lemma presup_gctx_lookup_typ {P : PtsSig} : forall {Δ : gctx P} {A x},
+    {{ ⊢ Δ }} ->
+    {{ `#x : A ∈ Δ }} ->
+    {{ Δ ; ⋅ ⊢ A }}.
+Proof with mautosolve 4.
+  intros * HΔ.
+  induction 1; inversion_clear HΔ; mauto 4.
+Qed.
+
 #[export]
-Remove Hints wf_vlookup : mcpts.
+Hint Resolve presup_gctx_lookup_typ : mcpts.
+ 
+(** ** Immediate Results of Context Presuppositions *)
+Lemma wf_gctx_sub_refl {P} : forall (Δ Δ' : gctx P),
+    {{ ⊢ Δ ≈ Δ' }} ->
+    {{ ⊢ Δ ⊆ Δ' }}.
+Proof. induction 1; mauto. Qed.
+
+#[export]
+Hint Resolve wf_gctx_sub_refl : mcpts.
+
+Lemma wf_ctx_sub_refl {P} : forall (Δ : gctx P) Γ Γ',
+    {{ Δ ⊢ Γ ≈ Γ' }} ->
+    {{ Δ ⊢ Γ ⊆ Γ' }}.
+Proof. induction 1; mauto. Qed.
+
+#[export]
+Hint Resolve wf_ctx_sub_refl : mcpts.
 
 
-Lemma exp_eq_sub_cong_typ1_sorted {P : PtsSig} : forall {Δ : ctx P} {Γ A A' σ s},
-    {{ Δ ⊢ A ≈ A' : Sort@s }} ->
-    {{ Γ ⊢s σ : Δ }} ->
-    {{ Γ ⊢ A[σ] ≈ A'[σ] : Sort@s }}.
-Proof with mautosolve 3.
+(** *** Equality-based conversions *)
+(** For well-formedness of expressions *)
+Lemma wf_exp_conv_exp_eq {P} : forall (Δ : gctx P) Γ M A s A',
+    {{ Δ ; Γ ⊢ M : A }} ->
+    (** The next two arguments will be removed in SystemOpt *)
+    {{ Δ ; Γ ⊢ A : Sort@s }} -> 
+    {{ Δ ; Γ ⊢ A' : Sort@s }} ->
+    {{ Δ ; Γ ⊢ A ≈ A' : Sort@s }} ->
+    {{ Δ ; Γ ⊢ M : A' }}.
+Proof.
   intros.
-  assert {{ Γ ⊢ Sort@s }} by mauto 3.
-  assert {{ Γ ⊢s σ ≈ σ : Δ }} by mauto 2.
-  assert {{ Γ ⊢ A[σ] ≈ A'[σ] : Sort@s[σ] }} by mauto 4.
+  assert {{ Δ ; Γ ⊢ A }} by mauto 2.
+  assert {{ Δ ; Γ ⊢ A' }} by mauto 2.
+  mauto.
+Qed.
+
+#[export]
+Hint Resolve wf_exp_conv_exp_eq : mcpts.
+  
+Lemma wf_exp_conv_typ_eq {P} : forall (Δ : gctx P) Γ M A A',
+    {{ Δ ; Γ ⊢ M : A }} ->
+    (** The next two arguments will be removed in SystemOpt *)
+    {{ Δ ; Γ ⊢ A }} ->
+    {{ Δ ; Γ ⊢ A' }} ->
+    {{ Δ ; Γ ⊢ A ≈ A'  }} ->
+    {{ Δ ; Γ ⊢ M : A' }}.
+Proof. mauto. Qed.
+
+#[export]
+Hint Resolve wf_exp_conv_typ_eq : mcpts.
+
+(** For well-formedness of substitutions *)
+Lemma wf_sub_conv_eq {P : PtsSig} : forall (Δ : gctx P) σ Γ Γ' Γ'',
+  {{ Δ ; Γ ⊢s σ : Γ' }} ->
+  {{ Δ ⊢ Γ' ≈ Γ'' }} ->
+  {{ Δ ; Γ ⊢s σ : Γ'' }}.
+Proof.
+  intros.
+  assert {{ Δ ⊢ Γ'' }} by mauto 2.
+  eapply wf_sub_conv; mauto.
+Qed.
+
+#[export]
+Hint Resolve wf_sub_conv_eq : mcpts.
+
+Add Parametric Morphism {P : PtsSig} (Δ : gctx P) (Γ : ctx P) : (wf_sub Δ Γ)
+    with signature wf_ctx_eq Δ ==> eq ==> iff as wf_sub_morphism_iff1.
+Proof.
+  intros Γ' Γ'' H **; split; [| symmetry in H]; mauto.
+Qed.
+
+(** For equality of expressions *)
+Lemma wf_exp_eq_conv_exp_eq {P} : forall (Δ : gctx P) Γ M M' A A' s,
+    {{ Δ ; Γ ⊢ M ≈ M' : A }} ->
+    (** The next two arguments will be removed in SystemOpt *)
+    {{ Δ ; Γ ⊢ A : Sort@s }} -> 
+    {{ Δ ; Γ ⊢ A' : Sort@s }} ->
+    {{ Δ ; Γ ⊢ A ≈ A' : Sort@s }} ->
+    {{ Δ ; Γ ⊢ M ≈ M' : A' }}.
+Proof. mauto. Qed. 
+
+#[export]
+Hint Resolve wf_exp_eq_conv_exp_eq : mcpts.
+
+Lemma wf_exp_eq_conv_typ_eq {P} : forall (Δ : gctx P) Γ M M' A A',
+    {{ Δ ; Γ ⊢ M ≈ M' : A }} ->
+    (** The next two arguments will be removed in SystemOpt *)
+    {{ Δ ; Γ ⊢ A }} -> 
+    {{ Δ ; Γ ⊢ A' }} ->
+    {{ Δ ; Γ ⊢ A ≈ A' }} ->
+    {{ Δ ; Γ ⊢ M ≈ M' : A' }}.
+Proof. mauto. Qed.
+
+#[export]
+Hint Resolve wf_exp_eq_conv_typ_eq : mcpts.
+
+(** For equality of substitutions *)
+Lemma wf_sub_eq_conv_eq {P : PtsSig} : forall (Δ : gctx P) σ σ' Γ Γ' Γ'',
+    {{ Δ ; Γ ⊢s σ ≈ σ' : Γ' }} ->
+    {{ Δ ⊢ Γ' ≈ Γ'' }} ->
+    {{ Δ ; Γ ⊢s σ ≈ σ' : Γ'' }}.
+Proof. mauto. Qed.
+
+#[export]
+Hint Resolve wf_sub_eq_conv_eq : mcpts.
+
+Add Parametric Morphism {P : PtsSig} (Δ : gctx P) (Γ : ctx P) : (wf_sub_eq Δ Γ)
+    with signature wf_ctx_eq Δ ==> eq ==> eq ==> iff as wf_sub_eq_morphism_iff3.
+Proof.
+  intros Γ' Γ'' H **; split; [| symmetry in H]; mauto.
+Qed.
+
+(** Other admissible rules following context presupposition *)
+Lemma wf_typ_eq_sub_id {P : PtsSig} : forall {Δ : gctx P} {Γ A},
+    {{ Δ ; Γ ⊢ A }} ->
+    {{ Δ ; Γ ⊢ A[Id] ≈ A }}.
+Proof.
+  induction 1; mauto 3.
+  transitivity {{{ A[σ∘Id] }}}; mauto 4.
+  symmetry.
+  mauto 4.
+Qed.
+
+#[export]
+Hint Resolve wf_typ_eq_sub_id : mcpts.
+
+
+(** ** Lemmas for [exp] of [{{{ Sort@s }}}] *)
+Lemma wf_typ_subtyp_sort_sub_left {P} : forall {Δ : gctx P} { Γ Γ' σ s},
+    {{ Δ ; Γ ⊢s σ : Γ' }} ->
+    {{ Δ ; Γ ⊢ Sort@s[σ] ⊆ Sort@s }}.
+Proof.
+  intros.
   econstructor; mauto 3.
 Qed.
 
-Lemma exp_eq_sub_cong_typ2_sorted {P} : forall {Δ : ctx P} {Γ A σ τ s},
-    {{ Δ ⊢ A : Sort@s }} ->
-    {{ Γ ⊢s σ : Δ }} ->
-    {{ Γ ⊢s σ ≈ τ : Δ }} ->
-    {{ Γ ⊢ A[σ] ≈ A[τ] : Sort@s }}.
-Proof with mautosolve 3.
+Lemma wf_typ_subtyp_sort_sub_right {P} : forall {Δ : gctx P} {Γ Γ' σ s},
+    {{ Δ ; Γ ⊢s σ : Γ' }} ->
+    {{ Δ ; Γ ⊢ Sort@s ⊆ Sort@s[σ] }}.
+Proof.
   intros.
-  assert {{ Γ ⊢ Sort@s }} by mauto 3.
-  assert {{ Δ ⊢ A ≈ A : Sort@s }} by mauto 3.
   econstructor; mauto 4.
 Qed.
 
+#[export]
+Hint Resolve wf_typ_subtyp_sort_sub_left wf_typ_subtyp_sort_sub_right : mcpts.
+ 
+Lemma wf_exp_sub_sorted {P} : forall {Δ : gctx P} {Γ Γ' A σ s},
+    {{ Δ ; Γ ⊢s σ : Γ' }} ->
+    {{ Δ ; Γ' ⊢ A : Sort@s }} ->
+    {{ Δ ; Γ ⊢ A[σ] : Sort@s }}.
+Proof.
+  intros.
+  assert {{ Δ ; Γ ⊢ A[σ] : Sort@s[σ] }} by mauto 4.
+  assert {{ Δ ⊢ Γ }} by mauto 2.
+  assert {{ Δ ; Γ ⊢ Sort@s[σ] ⊆ Sort@s }} by mauto 3.
+  econstructor; mauto 3.
+Qed.
 
-Lemma exp_eq_sub_compose_typ_sorted {P : PtsSig} : forall {Ψ : ctx P} {Δ Γ A σ τ s},
-    {{ Ψ ⊢ A : Sort@s }} ->
-    {{ Δ ⊢s σ : Ψ }} ->
-    {{ Γ ⊢s τ : Δ }} ->
-    {{ Γ ⊢ A[σ][τ] ≈ A[σ∘τ] : Sort@s }}.
+#[export]
+Hint Resolve wf_exp_sub_sorted : mcpts.
+
+Lemma wf_exp_eq_sub_cong_sorted1 {P : PtsSig} : forall {Δ : gctx P} {Γ Γ' A A' σ s},
+    {{ Δ ; Γ' ⊢ A ≈ A' : Sort@s }} ->
+    {{ Δ ; Γ ⊢s σ : Γ' }} ->
+    {{ Δ ; Γ ⊢ A[σ] ≈ A'[σ] : Sort@s }}.
+Proof with mautosolve 3.
+  intros.
+  assert {{ Δ ; Γ ⊢ Sort@s }} by mauto 3.
+  assert {{ Δ ; Γ ⊢s σ ≈ σ : Γ' }} by mauto 2.
+  assert {{ Δ ; Γ ⊢ A[σ] ≈ A'[σ] : Sort@s[σ] }} by mauto 4.
+  econstructor; mauto 3.
+Qed.
+             
+Lemma wf_exp_eq_sub_cong_sorted2 {P} : forall {Δ : gctx P} {Γ Γ' A σ τ s},
+    {{ Δ ; Γ' ⊢ A : Sort@s }} ->
+    {{ Δ ; Γ ⊢s σ : Γ' }} ->
+    {{ Δ ; Γ ⊢s σ ≈ τ : Γ' }} ->
+    {{ Δ ; Γ ⊢ A[σ] ≈ A[τ] : Sort@s }}.
+Proof with mautosolve 3.
+  intros.
+  assert {{ Δ ; Γ ⊢ Sort@s }} by mauto 3.
+  assert {{ Δ ; Γ' ⊢ A ≈ A : Sort@s }} by mauto 3.
+  econstructor; mauto 4.
+Qed.
+
+#[export]
+Hint Resolve wf_exp_eq_sub_cong_sorted1 wf_exp_eq_sub_cong_sorted2 : mcpts.
+ 
+  
+Lemma wf_exp_eq_sub_compose_sorted1 {P} : forall {Δ : gctx P} {Γ Γ' Γ'' A A' σ τ s},
+    {{ Δ ; Γ'' ⊢ A' : Sort@s }} ->
+    {{ Δ ; Γ'' ⊢ A ≈ A' : Sort@s }} ->
+    {{ Δ ; Γ' ⊢s σ : Γ'' }} ->
+    {{ Δ ; Γ ⊢s τ : Γ' }} ->
+    {{ Δ ; Γ ⊢ A[σ∘τ] ≈ A'[σ][τ] : Sort@s }}.
+Proof.
+  intros.
+  assert {{ Δ ; Γ ⊢ Sort@s[σ∘τ] ≈ Sort@s }} by mauto.
+  assert {{ Δ ; Γ ⊢ Sort@s[σ∘τ] ⊆ Sort@s }} by mauto.
+  assert {{ Δ ; Γ ⊢ A'[σ∘τ] ≈ A'[σ][τ] : Sort@s[σ∘τ] }} by mauto 4.
+  transitivity {{{ A'[σ∘τ] }}}; mauto 3.
+Qed.
+
+#[export]
+Hint Resolve wf_exp_eq_sub_compose_sorted1 : mcpts.
+
+Lemma wf_exp_eq_sub_compose_sorted2 {P : PtsSig} : forall {Δ : gctx P} {Γ Γ' Γ'' A σ τ s},
+    {{ Δ ; Γ'' ⊢ A : Sort@s }} ->
+    {{ Δ ; Γ' ⊢s σ : Γ'' }} ->
+    {{ Δ ; Γ ⊢s τ : Γ' }} ->
+    {{ Δ ; Γ ⊢ A[σ][τ] ≈ A[σ∘τ] : Sort@s }}.
 Proof with mautosolve 3.
   intros.
   econstructor...
 Qed.
 
 #[export]
-Hint Resolve exp_eq_sub_cong_typ1_sorted exp_eq_sub_cong_typ2_sorted exp_eq_sub_compose_typ_sorted : mcpts.
+Hint Resolve wf_exp_eq_sub_compose_sorted2 : mcpts.
 
-Lemma exp_eq_sub_compose_weaken_extend_typ {P : PtsSig} : forall {Γ : ctx P} {s σ Δ A B M},
-    {{ Γ ⊢s σ : Δ }} ->
-    {{ Δ ⊢ A : Sort@s }} ->
-    {{ Δ ⊢ B }} ->
-    {{ Γ ⊢ M : B[σ] }} ->
-    {{ Γ ⊢ A[Wk][σ,,M] ≈ A[σ] : Sort@s }}.
+Lemma wf_exp_eq_sub_compose_weaken_extend_sorted {P : PtsSig} : forall {Δ : gctx P} {Γ Γ' s σ A B M},
+    {{ Δ ; Γ ⊢s σ : Γ' }} ->
+    {{ Δ ; Γ' ⊢ A : Sort@s }} ->
+    {{ Δ ; Γ' ⊢ B }} ->
+    {{ Δ ; Γ ⊢ M : B[σ] }} ->
+    {{ Δ ; Γ ⊢ A[Wk][σ,,M] ≈ A[σ] : Sort@s }}.
 Proof with mautosolve 3.
   intros.
-  assert {{ Δ, B ⊢s Wk : Δ }} by mauto 4.
-  transitivity {{{ A[Wk∘(σ,,M)] }}}; [mautosolve 4 |].
-  eapply exp_eq_sub_cong_typ2_sorted...
+  assert {{ Δ ; Γ', B ⊢s Wk : Γ' }} by mauto 4.
+  assert {{ Δ ; Γ ⊢s Wk∘(σ,,M) ≈ σ : Γ' }} by mauto 3.
+  transitivity {{{ A[Wk∘(σ,,M)] }}}; mauto 4.
 Qed.
 
 #[export]
-Hint Resolve exp_eq_sub_compose_weaken_extend_typ : mcpts.
+Hint Resolve wf_exp_eq_sub_compose_weaken_extend_sorted : mcpts.
 
-Lemma exp_eq_sub_compose_weaken_id_extend_typ {P : PtsSig} : forall {Γ : ctx P} {s A B M},
-    {{ Γ ⊢ A : Sort@s }} ->
-    {{ Γ ⊢ B }} ->
-    {{ Γ ⊢ M : B }} ->
-    {{ Γ ⊢ A[Wk][Id,,M] ≈ A : Sort@s }}.
+
+Lemma exp_eq_sub_compose_weaken_id_extend_typ {P : PtsSig} : forall {Δ : gctx P} {Γ s A B M},
+    {{ Δ ; Γ ⊢ A : Sort@s }} ->
+    {{ Δ ; Γ ⊢ B }} ->
+    {{ Δ ; Γ ⊢ M : B }} ->
+    {{ Δ ; Γ ⊢ A[Wk][Id,,M] ≈ A : Sort@s }}.
 Proof with mautosolve 3.
   intros.
-  assert {{ ⊢ Γ }} by mauto 2.
-  assert {{ Γ ⊢ B[Id] }} by mauto 3.
-  assert {{ Γ ⊢ B ≈ B[Id] }} by mauto 3.
-  assert {{ Γ ⊢ M : B[Id] }} by mauto 2.
+  assert {{ Δ ⊢ Γ }} by mauto 2.
+  assert {{ Δ ; Γ ⊢ B[Id] }} by mauto 3.
+  assert {{ Δ ; Γ ⊢ B ≈ B[Id] }} by mauto 3.
+  assert {{ Δ ; Γ ⊢ M : B[Id] }} by mauto 2.
   transitivity {{{ A[Id] }}}...
 Qed.
 
 #[export]
 Hint Resolve exp_eq_sub_compose_weaken_id_extend_typ : mcpts.
 
-Lemma exp_eq_sub_compose_double_weaken_double_extend_typ {P : PtsSig} : forall {Γ : ctx P} {s σ Δ A B M C N},
-    {{ Γ ⊢s σ : Δ }} ->
-    {{ Δ ⊢ A : Sort@s }} ->
-    {{ Δ ⊢ B }} ->
-    {{ Γ ⊢ M : B[σ] }} ->
-    {{ Δ, B ⊢ C }} ->
-    {{ Γ ⊢ N : C[σ,,M] }} ->
-    {{ Γ ⊢ A[Wk∘Wk][σ,,M,,N] ≈ A[σ] : Sort@s }}.
+Lemma wf_exp_eq_sub_compose_double_weaken_double_extend_sorted {P : PtsSig} : forall {Δ : gctx P} {Γ Γ' s σ A B M C N},
+    {{ Δ ; Γ ⊢s σ : Γ' }} ->
+    {{ Δ ; Γ' ⊢ A : Sort@s }} ->
+    {{ Δ ; Γ' ⊢ B }} ->
+    {{ Δ ; Γ ⊢ M : B[σ] }} ->
+    {{ Δ; Γ', B ⊢ C }} ->
+    {{ Δ ; Γ ⊢ N : C[σ,,M] }} ->
+    {{ Δ ; Γ ⊢ A[Wk∘Wk][σ,,M,,N] ≈ A[σ] : Sort@s }}.
 Proof with mautosolve 3.
   intros.
-  assert {{ ⊢ Γ }} by mauto 2.
-  assert {{ ⊢ Δ }} by mauto 2.
-  assert {{ Δ, B ⊢s Wk : Δ }} by mauto 3.
-  assert {{ Δ, B, C ⊢s Wk : Δ, B }} by mauto 4.
-  assert {{ Δ, B ⊢ Sort@s }} by mauto 3.
-  assert {{ Δ, B ⊢ A[Wk] : Sort@s }} by mauto 3.
-  transitivity {{{ A[Wk][Wk][σ,,M,,N] }}}; [eapply exp_eq_sub_cong_typ1_sorted; mautosolve 3 |].
+  assert {{ Δ ⊢ Γ }} by mauto 2.
+  assert {{ Δ ⊢ Γ' }} by mauto 2.
+  assert {{ Δ; Γ', B ⊢s Wk : Γ' }} by mauto 3.
+  assert {{ Δ; Γ', B, C ⊢s Wk : Γ', B }} by mauto 4.
+  assert {{ Δ; Γ', B ⊢ Sort@s }} by mauto 3.
+  assert {{ Δ; Γ', B ⊢ A[Wk] : Sort@s }} by mauto 3.
+  transitivity {{{ A[Wk][Wk][σ,,M,,N] }}}; [eapply wf_exp_eq_sub_cong_sorted1; mautosolve 3 |].
   transitivity {{{ A[Wk][σ,,M] }}}...
 Qed.
 
 #[export]
-Hint Resolve exp_eq_sub_compose_double_weaken_double_extend_typ : mcpts.
+Hint Resolve wf_exp_eq_sub_compose_double_weaken_double_extend_sorted : mcpts.
 
-Lemma exp_eq_sub_compose_double_weaken_id_double_extend_typ {P : PtsSig} : forall {Γ : ctx P} {s A B M C N},
-    {{ Γ ⊢ A : Sort@s }} ->
-    {{ Γ ⊢ B }} ->
-    {{ Γ ⊢ M : B }} ->
-    {{ Γ, B ⊢ C }} ->
-    {{ Γ ⊢ N : C[Id,,M] }} ->
-    {{ Γ ⊢ A[Wk∘Wk][Id,,M,,N] ≈ A : Sort@s }}.
+Lemma wf_exp_eq_sub_compose_double_weaken_id_double_extend_sorted {P : PtsSig} : forall {Δ : gctx P} {Γ s A B M C N},
+    {{ Δ ; Γ ⊢ A : Sort@s }} ->
+    {{ Δ ; Γ ⊢ B }} ->
+    {{ Δ ; Γ ⊢ M : B }} ->
+    {{ Δ ; Γ, B ⊢ C }} ->
+    {{ Δ ; Γ ⊢ N : C[Id,,M] }} ->
+    {{ Δ ; Γ ⊢ A[Wk∘Wk][Id,,M,,N] ≈ A : Sort@s }}.
 Proof with mautosolve 3.
   intros.
-  assert {{ ⊢ Γ }} by mauto 2.
-  assert {{ Γ ⊢ B[Id] }} by mauto 3.
-  assert {{ Γ ⊢ B ≈ B[Id]  }} by mauto 3.
-  assert {{ Γ ⊢ M : B[Id] }} by mauto 3.
+  assert {{ Δ ⊢ Γ }} by mauto 2.
+  assert {{ Δ ; Γ ⊢ B[Id] }} by mauto 3.
+  assert {{ Δ ; Γ ⊢ B ≈ B[Id]  }} by mauto 3.
+  assert {{ Δ ; Γ ⊢ M : B[Id] }} by mauto 3.
   transitivity {{{ A[Id] }}}...
 Qed.
 
 #[export]
-Hint Resolve exp_eq_sub_compose_double_weaken_id_double_extend_typ : mcpts.
+Hint Resolve wf_exp_eq_sub_compose_double_weaken_id_double_extend_sorted : mcpts.
 
-Lemma exp_eq_typ_sub_sub {P : PtsSig} : forall {Γ : ctx P} {Δ Ψ σ τ s1 s2},
-    {{ Ψ ⊢ Sort@s1 : Sort@s2 }} ->
-    {{ Γ ⊢ Sort@s1 : Sort@s2 }} ->
-    {{ Δ ⊢s σ : Ψ }} ->
-    {{ Γ ⊢s τ : Δ }} ->
-    {{ Γ ⊢ Sort@s1[σ][τ] ≈ Sort@s1 : Sort@s2 }}.
+Lemma wf_exp_eq_sort_sub_sub {P : PtsSig} : forall {Δ : gctx P} {Γ Γ' Γ'' σ τ s1 s2},
+    {{ Δ ; Γ'' ⊢ Sort@s1 : Sort@s2 }} ->
+    {{ Δ ; Γ ⊢ Sort@s1 : Sort@s2 }} ->
+    {{ Δ ; Γ' ⊢s σ : Γ'' }} ->
+    {{ Δ ; Γ ⊢s τ : Γ' }} ->
+    {{ Δ ; Γ ⊢ Sort@s1[σ][τ] ≈ Sort@s1 : Sort@s2 }}.
 Proof.
   intros.
   transitivity {{{ Sort@s1[σ∘τ] }}}; [symmetry |]; mauto 3.  
 Qed.
 
 #[export]
-Hint Resolve exp_eq_typ_sub_sub : mcpts.
+Hint Resolve wf_exp_eq_sort_sub_sub : mcpts.
 #[export]
-Hint Rewrite -> @exp_eq_typ_sub_sub using mauto 4 : mcpts.
+Hint Rewrite -> @wf_exp_eq_sort_sub_sub using mauto 4 : mcpts.
 
-Lemma wf_exp_sort_sort_implies_axiom {P} : forall {Γ : ctx P} {s1 K},
-    {{ Γ ⊢ Sort@s1 : K }} ->
-    exists s2,
-      Ax_typ P s1 s2 /\
-        {{ Γ ⊢ Sort@s2 ⊆ K }}.
-Proof.
-  intros * H.
-  dependent induction H.
-  - eexists; split; mauto 2.
-  - specialize (IHwf_exp s1 A ltac:(reflexivity) ltac:(reflexivity)) as [s2 []].
-    eexists; mauto.
+Lemma vlookup_0_typ {P : PtsSig} : forall {Δ : gctx P} {Γ s},
+    {{ Δ ⊢ Γ }} ->
+    {{ Δ ; Γ, Sort@s ⊢ #0 : Sort@s }}.
+Proof with mautosolve 4.
+  intros.
+  assert {{ Δ ; Γ, Sort@s ⊢s Wk : Γ }} by mauto 4.
+  eapply wf_exp_conv_typ_eq with (A := {{{ Sort@s[Wk] }}}); mauto 3. 
 Qed.
 
-#[export]
-Hint Resolve wf_exp_sort_sort_implies_axiom : mcpts.
-
-(** *** Lemmas for [exp] of [{{{ ℕ }}}] *)
-
-Lemma wf_exp_subtyp_nat_sub {P} : forall {Γ : ctx P} {Δ σ s} {r : Ru_nat P s},
-    {{ Γ ⊢s σ : Δ }} ->
-    {{ Γ ⊢ ℕ[σ] ⊆ ℕ }}.
-Proof.
-  intros.
-  econstructor; mauto 3.
-  econstructor; mauto 3.
-Qed. 
-
-#[export]
-Hint Resolve wf_exp_subtyp_nat_sub : mcpts.
- 
-Lemma exp_sub_nat {P} : forall {Γ : ctx P} {Δ M σ s} {r : Ru_nat P s},
-    {{ Δ ⊢ M : ℕ }} ->
-    {{ Γ ⊢s σ : Δ }} ->
-    {{ Γ ⊢ M[σ] : ℕ }}.
+Lemma vlookup_1_typ {P : PtsSig} : forall {Δ : gctx P} {Γ s A},
+    {{ Δ ; Γ, Sort@s ⊢ A }} ->
+    {{ Δ ; Γ, Sort@s, A ⊢ #1 : Sort@s }}.
 Proof with mautosolve 3.
   intros.
-  assert {{ ⊢ Δ }} by mauto 2.
-  assert {{ Δ ⊢ ℕ }} by mauto 3.
-  assert {{ Γ ⊢ ℕ }} by mauto 3.
-  assert {{ Γ ⊢ M[σ] : ℕ[σ] }} by mauto 3.  
-  econstructor; mauto 2.
-Qed.
-
-#[export]
-Hint Resolve exp_sub_nat : mcpts.
-
-Lemma exp_eq_sub_cong_nat1 {P} : forall {Γ : ctx P} {Δ M M' σ s} {r : Ru_nat P s},
-    {{ Δ ⊢ M ≈ M' : ℕ }} ->
-    {{ Γ ⊢s σ : Δ }} ->
-    {{ Γ ⊢ M[σ] ≈ M'[σ] : ℕ }}.
-Proof with mautosolve 4.
-  intros.
-  assert {{ ⊢ Δ }} by mauto 2.
-  assert {{ Δ ⊢ ℕ }} by mauto 3.
-  assert {{ Γ ⊢ ℕ }} by mauto 3.  
-  econstructor; mauto.
-Qed.
-
-Lemma exp_eq_sub_cong_nat2 {P} : forall {Γ : ctx P} {Δ M σ τ s} {r : Ru_nat P s},
-    {{ Δ ⊢ M : ℕ }} ->
-    {{ Γ ⊢s σ : Δ }} ->
-    {{ Γ ⊢s σ ≈ τ : Δ }} ->
-    {{ Γ ⊢ M[σ] ≈ M[τ] : ℕ }}.
-Proof with mautosolve 4.
-  intros.
-  assert {{ ⊢ Δ }} by mauto 2.
-  assert {{ Δ ⊢ ℕ }} by mauto 3.
-  assert {{ Γ ⊢ ℕ }} by mauto 3.
-  econstructor; mauto.
-Qed.
-
-
-Lemma exp_eq_sub_compose_nat {P} : forall {Γ : ctx P} {Ψ Δ M σ τ s} {r : Ru_nat P s},
-    {{ Ψ ⊢ M : ℕ }} ->
-    {{ Δ ⊢s σ : Ψ }} ->
-    {{ Γ ⊢s τ : Δ }} ->
-    {{ Γ ⊢ M[σ][τ] ≈ M[σ∘τ] : ℕ }}.
-Proof with mautosolve 4.
-  intros.
-  assert {{ ⊢ Ψ }} by mauto 2.
-  assert {{ ⊢ Δ }} by mauto 2.
-  assert {{ Ψ ⊢ ℕ }} by mauto 3.
-  assert {{ Δ ⊢ ℕ }} by mauto 3.
-  assert {{ Γ ⊢ ℕ }} by mauto 3.
-  assert {{ Γ ⊢ M[σ∘τ] ≈ M[σ][τ] : ℕ[σ∘τ] }} by mauto 3.
-  econstructor; mauto 3.
-Qed.
-
-
-#[export]
-Hint Resolve exp_sub_nat exp_eq_sub_cong_nat1 exp_eq_sub_cong_nat2 exp_eq_sub_compose_nat : mcpts.
-
-Lemma exp_eq_nat_sub_sub {P} : forall {Γ : ctx P} {Δ Ψ σ τ s} {r : Ru_nat P s},
-    {{ Δ ⊢s σ : Ψ }} ->
-    {{ Γ ⊢s τ : Δ }} ->
-    {{ Γ ⊢ ℕ[σ][τ] ≈ ℕ : Sort@s }}.
-Proof. mauto. Qed.
-
-#[export]
-Hint Resolve exp_eq_nat_sub_sub : mcpts.
-
-Lemma exp_eq_nat_sub_sub_to_nat_sub {P} : forall {Γ : ctx P} {Δ Ψ Ψ' σ τ σ' s} {r : Ru_nat P s},
-    {{ Δ ⊢s σ : Ψ }} ->
-    {{ Γ ⊢s τ : Δ }} ->
-    {{ Γ ⊢s σ' : Ψ' }} ->
-    {{ Γ ⊢ ℕ[σ][τ] ≈ ℕ[σ'] : Sort@s}}.
-Proof. mauto. Qed.
-
-#[export]
-Hint Resolve exp_eq_nat_sub_sub_to_nat_sub : mcpts.
-
-Lemma exp_eq_sub_compose_weaken_extend_nat {P} : forall {Γ : ctx P} {σ Δ M B N s} {r : Ru_nat P s},
-    {{ Γ ⊢s σ : Δ }} ->
-    {{ Δ ⊢ M : ℕ }} ->
-    {{ Δ ⊢ B }} ->
-    {{ Γ ⊢ N : B[σ] }} ->
-    {{ Γ ⊢ M[Wk][σ,,N] ≈ M[σ] : ℕ }}.
-Proof with mautosolve 4.
-  intros.
-  assert {{ ⊢ Δ }} by mauto 2.
-  assert {{ Δ, B ⊢s Wk : Δ }} by mauto 3.
-  assert {{ Γ ⊢s σ,,N : Δ, B }} by mauto 2.
-  transitivity {{{ M[Wk∘(σ,,N)] }}}...
-Qed.
-
-#[export]
-Hint Resolve exp_eq_sub_compose_weaken_extend_nat : mcpts.
-
-Lemma exp_eq_sub_compose_weaken_id_extend_nat {P} : forall {Γ : ctx P} {M B N s} {r : Ru_nat P s},
-    {{ Γ ⊢ M : ℕ }} ->
-    {{ Γ ⊢ B }} ->
-    {{ Γ ⊢ N : B }} ->
-    {{ Γ ⊢ M[Wk][Id,,N] ≈ M : ℕ }}.
-Proof with mautosolve 3.
-  intros.
-  assert {{ ⊢ Γ }} by mauto 2.
-  assert {{ Γ ⊢ B[Id] }} by mauto 3.
-  assert {{ Γ ⊢ B ≈ B[Id] }} by mauto 4.
-  assert {{ Γ ⊢ N : B[Id] }} by mauto 4.
-  transitivity {{{ M[Id] }}}...
-Qed.
-
-#[export]
-Hint Resolve exp_eq_sub_compose_weaken_id_extend_nat : mcpts.
-
-Lemma exp_eq_sub_compose_double_weaken_double_extend_nat {P} : forall {Γ : ctx P} {σ Δ M B N C L s} {r : Ru_nat P s},
-    {{ Γ ⊢s σ : Δ }} ->
-    {{ Δ ⊢ M : ℕ }} ->
-    {{ Δ ⊢ B  }} ->
-    {{ Γ ⊢ N : B[σ] }} ->
-    {{ Δ, B ⊢ C }} ->
-    {{ Γ ⊢ L : C[σ,,N] }} ->
-    {{ Γ ⊢ M[Wk∘Wk][σ,,N,,L] ≈ M[σ] : ℕ }}.
-Proof with mautosolve 3.
-  intros.
-  assert {{ ⊢ Δ }} by mauto 2.
-  assert {{ Δ, B ⊢s Wk : Δ }} by mauto 3.
-  assert {{ Δ, B, C ⊢s Wk : Δ, B }} by mauto 4.
-  assert {{ Γ ⊢s σ,,N : Δ, B }} by mauto 2.
-  assert {{ Γ ⊢s σ,,N,,L : Δ, B, C }} by mauto 2.
-  transitivity {{{ M[Wk][Wk][σ,,N,,L] }}}; [econstructor; mautosolve 3|].
-  transitivity {{{ M[Wk][σ,,N] }}}...
-Qed.
-
-#[export]
-Hint Resolve exp_eq_sub_compose_double_weaken_double_extend_nat : mcpts.
-
-Lemma exp_eq_sub_compose_double_weaken_id_double_extend_nat {P} : forall {Γ : ctx P} {M B N C L s } {r : Ru_nat P s},
-    {{ Γ ⊢ M : ℕ }} ->
-    {{ Γ ⊢ B }} ->
-    {{ Γ ⊢ N : B }} ->
-    {{ Γ, B ⊢ C }} ->
-    {{ Γ ⊢ L : C[Id,,N] }} ->
-    {{ Γ ⊢ M[Wk∘Wk][Id,,N,,L] ≈ M : ℕ }}.
-Proof with mautosolve 3.
-  intros.
-  assert {{ ⊢ Γ }} by mauto 2.
-  assert {{ Γ ⊢ B[Id] }} by mauto 3.
-  assert {{ Γ ⊢ B ≈ B[Id] }} by mauto 4.
-  assert {{ Γ ⊢ N : B[Id] }} by mauto 4.
-  transitivity {{{ M[Id] }}}...
-Qed.
-
-#[export]
-Hint Resolve exp_eq_sub_compose_double_weaken_id_double_extend_nat : mcpts.
-
-Lemma vlookup_0_nat {P} : forall {Γ : ctx P} {s} {r : Ru_nat P s},
-    {{ ⊢ Γ }} ->
-    {{ Γ, ℕ ⊢ #0 : ℕ }}.
-Proof with mautosolve 3.
-  intros.
-  assert {{ Γ ⊢ ℕ }} by mauto 3.
-  assert {{ Γ, ℕ ⊢s Wk : Γ }} by mauto 3.
-  eapply wf_exp_conv...
-Qed.
-
-Lemma vlookup_1_nat {P} : forall {Γ : ctx P} {A s} {r : Ru_nat P s},
-    {{ Γ, ℕ ⊢ A }} ->
-    {{ Γ, ℕ, A ⊢ #1 : ℕ }}.
-Proof with mautosolve 3.
-  intros.
-  assert {{ ⊢ Γ }} by mauto 3.
-  assert {{ Γ ⊢ ℕ : Sort@s }} by mauto 2.
-  assert {{ Γ, ℕ ⊢s Wk : Γ }} by mauto 4.
-  assert {{ Γ, ℕ, A ⊢s Wk : Γ, ℕ }} by mauto 5.
-  assert {{ Γ, ℕ, A ⊢ #1 : ℕ[Wk][Wk] }} by mauto 4.
-  eapply wf_conv; mauto 4.
-Qed.
-
-#[export]
-Hint Resolve vlookup_0_nat vlookup_1_nat : mcpts.
-
-Lemma exp_sub_nat_helper {P} : forall {Γ : ctx P} {σ Δ M s} {r : Ru_nat P s},
-    {{ Γ ⊢s σ : Δ }} ->
-    {{ Γ ⊢ M : ℕ }} ->
-    {{ Γ ⊢ M : ℕ[σ] }}.
-Proof.
-  intros.
-  assert {{ ⊢ Δ }} by mauto 2.
-  assert {{ Δ ⊢ ℕ }} by mauto 3.
-  assert {{ Γ ⊢ ℕ }} by mauto 3.
-  assert {{ Γ ⊢ ℕ[σ] }} by mauto 3.
-  assert {{ Γ ⊢ ℕ ≈ ℕ[σ] }} by (symmetry; mauto 3).
-  assert {{ Γ ⊢ ℕ ⊆ ℕ[σ] }} by mauto 2.
-  eapply wf_exp_conv; mauto 2.
-Qed.
-
-#[export]
-Hint Resolve exp_sub_nat_helper : mcpts.
-
-Lemma exp_eq_var_0_sub_nat {P} : forall {Γ : ctx P} {σ Δ M s} {r : Ru_nat P s},
-    {{ Γ ⊢s σ : Δ }} ->
-    {{ Γ ⊢ M : ℕ }} ->
-    {{ Γ ⊢ #0[σ,,M] ≈ M : ℕ }}.
-Proof with mautosolve 3.
-  intros.
-  assert {{ ⊢ Δ }} by mauto 2.
-  assert {{ Δ ⊢ ℕ }} by mauto 3.
-  eapply wf_exp_eq_conv...
-Qed.
-
-Lemma exp_eq_var_1_sub_nat {P} : forall {Γ : ctx P} {σ Δ A M s} {r : Ru_nat P s},
-    {{ Γ ⊢s σ : Δ }} ->
-    {{ Δ ⊢ A }} ->
-    {{ Γ ⊢ M : A[σ] }} ->
-    {{ #0 : ℕ[Wk] ∈ Δ }} ->
-    {{ Γ ⊢ #1[σ,,M] ≈ #0[σ] : ℕ }}.
-Proof with mautosolve 4.
-  inversion 5 as [? Δ'|]; subst.
-  assert {{ Γ ⊢ #1[σ,,M] ≈ #0[σ] : ℕ[Wk][σ] }} by mauto 3.
-  eapply wf_exp_eq_conv; mauto 3.
-  econstructor; mauto.
-Qed.
-
-#[export]
-Hint Resolve exp_eq_var_0_sub_nat exp_eq_var_1_sub_nat : mcpts.
-
-Lemma exp_eq_var_0_weaken_nat {P} : forall {Γ : ctx P} {A s} {r : Ru_nat P s},
-    {{ ⊢ Γ, A }} ->
-    {{ #0 : ℕ[Wk] ∈ Γ }} ->
-    {{ Γ, A ⊢ #0[Wk] ≈ #1 : ℕ }}.
-Proof with mautosolve 4.
-  inversion 2; subst.
-  inversion 1; subst.
-  assert {{ Γ0, ℕ, A ⊢ #0[Wk] ≈ #1 : ℕ[Wk][Wk] }} by mauto 3.
-  eapply wf_exp_eq_conv; mauto 3.
-  econstructor; mauto.
-Qed.
-
-#[export]
-Hint Resolve exp_eq_var_0_weaken_nat : mcpts.
-
-Lemma sub_extend_nat {P} : forall {Γ : ctx P} {σ Δ M s} {r : Ru_nat P s},
-    {{ Γ ⊢s σ : Δ }} ->
-    {{ Γ ⊢ M : ℕ }} ->
-    {{ Γ ⊢s σ,,M : Δ, ℕ }}.
-Proof with mautosolve 4.
-  intros.
-  econstructor...
-Qed.
-
-#[export]
-Hint Resolve sub_extend_nat : mcpts.
-
-Lemma sub_eq_extend_cong_nat {P} : forall {Γ : ctx P} {σ σ' Δ M M' s} {r : Ru_nat P s},
-    {{ Γ ⊢s σ : Δ }} ->
-    {{ Γ ⊢s σ ≈ σ' : Δ }} ->
-    {{ Γ ⊢ M ≈ M' : ℕ }} ->
-    {{ Γ ⊢s σ,,M ≈ σ',,M' : Δ, ℕ }}.
-Proof with mautosolve 4.
-  intros.
-  econstructor; mauto 4.
-  assert {{ ⊢ Γ }} by mauto 2.
-  assert {{ Γ ⊢ ℕ ≈ ℕ[σ] : Sort@s }} by mauto 3.
-  assert {{ Δ ⊢ ℕ : Sort@s }} by mauto 3.
-  assert {{ Γ ⊢ ℕ[σ] : Sort@s }} by mauto 3.
-  assert {{ Γ ⊢ ℕ ⊆ ℕ[σ] }} by mauto 4.
-  eapply wf_exp_eq_conv; mauto 3.
-Qed.
-
-Lemma sub_eq_extend_compose_nat {P} : forall {Γ : ctx P} {τ Γ' σ Γ'' M s} {r : Ru_nat P s},
-    {{ Γ' ⊢s σ : Γ'' }} ->
-    {{ Γ' ⊢ M : ℕ }} ->
-    {{ Γ ⊢s τ : Γ' }} ->
-    {{ Γ ⊢s (σ,,M)∘τ ≈ (σ∘τ),,M[τ] : Γ'', ℕ }}.
-Proof with mautosolve 4.
-  intros.
-  econstructor...
-Qed.
-
-Lemma sub_eq_p_extend_nat {P} : forall {Γ : ctx P} {σ Γ' M s} {r : Ru_nat P s},
-    {{ Γ' ⊢s σ : Γ }} ->
-    {{ Γ' ⊢ M : ℕ }} ->
-    {{ Γ' ⊢s Wk∘(σ,,M) ≈ σ : Γ }}.
-Proof with mautosolve.
-  intros.
-  assert {{ Γ ⊢ ℕ : Sort@s }} by (econstructor; mauto 3).
-  econstructor...
-Qed.
-
-#[export]
-Hint Resolve sub_eq_extend_cong_nat sub_eq_extend_compose_nat sub_eq_p_extend_nat : mcpts.
-
-Lemma exp_eq_sub_sub_compose_cong_nat {P} : forall {Γ : ctx P} {Δ Δ' Ψ σ τ σ' τ' M s} {r : Ru_nat P s},
-    {{ Ψ ⊢ M : ℕ }} ->
-    {{ Δ ⊢s σ : Ψ }} ->
-    {{ Δ' ⊢s σ' : Ψ }} ->
-    {{ Γ ⊢s τ : Δ }} ->
-    {{ Γ ⊢s τ' : Δ' }} ->
-    {{ Γ ⊢s σ∘τ ≈ σ'∘τ' : Ψ }} ->
-    {{ Γ ⊢ M[σ][τ] ≈ M[σ'][τ'] : ℕ }}.
-Proof with mautosolve 4.
-  intros.
-  assert {{ Γ ⊢ M[σ][τ] ≈ M[σ∘τ] : ℕ }} by mauto.
-  assert {{ Γ ⊢ M[σ∘τ] ≈ M[σ'∘τ'] : ℕ }} by mauto.
-  enough {{ Γ ⊢ M[σ'∘τ'] ≈ M[σ'][τ'] : ℕ }}...
-Qed.
-
-#[export]
-Hint Resolve exp_eq_sub_sub_compose_cong_nat : mcpts.
-
-(** Lemmas about variables *)
-
-Lemma vlookup_0_typ {P : PtsSig} : forall {Γ : ctx P} {s},
-    {{ ⊢ Γ }} ->
-    {{ Γ, Sort@s ⊢ #0 : Sort@s }}.
-Proof with mautosolve 4.
-  intros.
-  assert {{ Γ, Sort@s ⊢s Wk : Γ }} by (econstructor; mauto 3).
-  eapply wf_exp_conv with (A := {{{ Sort@s[Wk] }}}); mauto 3.
-  econstructor...
-Qed.
-
-Lemma vlookup_1_typ {P : PtsSig} : forall {Γ : ctx P} {s A},
-    {{ Γ, Sort@s ⊢ A }} ->
-    {{ Γ, Sort@s, A ⊢ #1 : Sort@s }}.
-Proof with mautosolve 3.
-  intros.
-  assert {{ Γ, Sort@s ⊢s Wk : Γ }} by mauto 4.
-  assert {{ Γ, Sort@s, A ⊢s Wk : Γ, Sort@s }} by (econstructor; mauto 4).
-  assert {{ ⊢ Γ, Sort@s, A }} by mauto 3.
-  assert {{ ⊢ Γ }} by mauto 2.
-  assert {{ Γ, Sort@s ⊢ Sort@s[Wk] }} by mauto 3.
-  assert {{ Γ, Sort@s, A ⊢ Sort@s[Wk][Wk] }} by mauto 3.
+  assert {{ Δ ; Γ, Sort@s ⊢s Wk : Γ }} by mauto 4.
+  assert {{ Δ ; Γ, Sort@s, A ⊢s Wk : Γ, Sort@s }} by (econstructor; mauto 4).
+  assert {{ Δ ⊢ Γ, Sort@s, A }} by mauto 3.
+  assert {{ Δ ⊢ Γ }} by mauto 2.
+  assert {{ Δ ; Γ, Sort@s ⊢ Sort@s[Wk] }} by mauto 3.
+  assert {{ Δ ; Γ, Sort@s, A ⊢ Sort@s[Wk][Wk] }} by mauto 3.
   eapply wf_exp_conv with (A := {{{ Sort@s[Wk][Wk] }}}); mauto 3.
   econstructor; mauto 3.
   transitivity {{{ Sort@s[Wk] }}}; mauto 4.
@@ -881,915 +778,1463 @@ Qed.
 #[export]
 Hint Resolve vlookup_0_typ vlookup_1_typ : mcpts.
 
-Lemma exp_sub_typ_helper {P : PtsSig} : forall {Γ : ctx P} {σ Δ M s},
-    {{ Γ ⊢s σ : Δ }} ->
-    {{ Γ ⊢ M : Sort@s }} ->
-    {{ Γ ⊢ M : Sort@s[σ] }}.
+Lemma wf_exp_sub_typ_helper {P : PtsSig} : forall {Δ : gctx P} {Γ Γ' σ M s},
+    {{ Δ ; Γ ⊢s σ : Γ' }} ->
+    {{ Δ ; Γ ⊢ M : Sort@s }} ->
+    {{ Δ ; Γ ⊢ M : Sort@s[σ] }}.
 Proof.
   intros.
   do 3 (econstructor; mauto 4).
 Qed.
 
 #[export]
-Hint Resolve exp_sub_typ_helper : mcpts.
+Hint Resolve wf_exp_sub_typ_helper : mcpts.
 
-Lemma exp_eq_var_0_sub_typ {P : PtsSig} : forall {Γ : ctx P} {σ Δ M s},
-    {{ Γ ⊢s σ : Δ }} ->
-    {{ Γ ⊢ M : Sort@s }} ->
-    {{ Γ ⊢ #0[σ,,M] ≈ M : Sort@s }}.
+Lemma wf_exp_eq_var_0_sub_typ {P : PtsSig} : forall {Δ : gctx P} {Γ Γ' σ M s},
+    {{ Δ ; Γ ⊢s σ : Γ' }} ->
+    {{ Δ ; Γ ⊢ M : Sort@s }} ->
+    {{ Δ ; Γ ⊢ #0[σ,,M] ≈ M : Sort@s }}.
 Proof with mautosolve 3.
   intros.
-  assert {{ ⊢ Δ }} by mauto 2.
-  assert {{ Γ ⊢ Sort@s [σ] ⊆ Sort@s  }} by mauto 5.
+  assert {{ Δ ⊢ Γ' }} by mauto 2.
+  assert {{ Δ ; Γ ⊢ Sort@s[σ] ⊆ Sort@s  }} by mauto 5.
   eapply wf_exp_eq_conv; mauto 4.
 Qed.
 
-Lemma exp_eq_var_1_sub_typ {P : PtsSig} : forall {Γ : ctx P} {σ Δ A M s},
-    {{ Γ ⊢s σ : Δ }} ->
-    {{ Δ ⊢ A }} ->
-    {{ Γ ⊢ M : A[σ] }} ->
-    {{ #0 : Sort@s[Wk] ∈ Δ }} ->
-    {{ Γ ⊢ #1[σ,,M] ≈ #0[σ] : Sort@s }}.
+Lemma wf_exp_eq_var_1_sub_typ {P : PtsSig} : forall {Δ : gctx P} {Γ Γ' σ A M s},
+    {{ Δ ; Γ ⊢s σ : Γ' }} ->
+    {{ Δ ; Γ' ⊢ A }} ->
+    {{ Δ ; Γ ⊢ M : A[σ] }} ->
+    {{ #0 : Sort@s[Wk] ∈ Γ' }} ->
+    {{ Δ ; Γ ⊢ #1[σ,,M] ≈ #0[σ] : Sort@s }}.
 Proof with mautosolve 3.
   intros.
   inversion H2; subst.
-  assert {{ ⊢ Γ0 }} by mauto 3.
-  assert {{ Γ0, Sort@s ⊢s Wk : Γ0 }} by mauto 3.
+  assert {{ Δ ⊢ Γ0 }} by mauto 3.
+  assert {{ Δ ; Γ0, Sort@s ⊢s Wk : Γ0 }} by mauto 3.
   eapply wf_exp_eq_conv; mauto 3.
   econstructor; mauto 3.
   transitivity {{{ Sort@s[σ] }}}; mauto 4.
 Qed.
 
 #[export]
-Hint Resolve exp_eq_var_0_sub_typ exp_eq_var_1_sub_typ : mcpts.
+Hint Resolve wf_exp_eq_var_0_sub_typ wf_exp_eq_var_1_sub_typ : mcpts.
 #[export]
-Hint Rewrite -> @exp_eq_var_0_sub_typ @exp_eq_var_1_sub_typ : mcpts.
+Hint Rewrite -> @wf_exp_eq_var_0_sub_typ @wf_exp_eq_var_1_sub_typ : mcpts.
 
-Lemma exp_eq_var_0_weaken_typ {P : PtsSig} : forall {Γ : ctx P} {A s},
-    {{ ⊢ Γ, A }} ->
+Lemma wf_exp_eq_var_0_weaken_typ {P : PtsSig} : forall {Δ : gctx P} {Γ A s},
+    {{ Δ ⊢ Γ, A }} ->
     {{ #0 : Sort@s[Wk] ∈ Γ }} ->
-    {{ Γ, A ⊢ #0[Wk] ≈ #1 : Sort@s }}.
+    {{ Δ ; Γ, A ⊢ #0[Wk] ≈ #1 : Sort@s }}.
 Proof with mautosolve 3.
   inversion_clear 1.
   inversion 1 as [? Γ'|]; subst.
-  assert {{ ⊢ Γ' }} by mauto 2.
-  assert {{ Γ', Sort@s ⊢s Wk : Γ' }} by mauto 4.
-  assert {{ Γ', Sort@s, A ⊢s Wk : Γ', Sort@s }} by mauto 4.
+  assert {{ Δ ⊢ Γ' }} by mauto 2.
+  assert {{ Δ ; Γ', Sort@s ⊢s Wk : Γ' }} by mauto 4.
+  assert {{ Δ ; Γ', Sort@s, A ⊢s Wk : Γ', Sort@s }} by mauto 4.
   eapply wf_exp_eq_conv; mauto 3.
   econstructor; mauto 3.
   transitivity {{{ Sort@s[Wk] }}}; mauto 4.
 Qed.
 
 #[export]
-Hint Resolve exp_eq_var_0_weaken_typ : mcpts.
+Hint Resolve wf_exp_eq_var_0_weaken_typ : mcpts.
 
-Lemma sub_extend_typ {P : PtsSig} : forall {Γ : ctx P} {σ Δ M s},
-    {{ Γ ⊢s σ : Δ }} ->
-    {{ Γ ⊢ M : Sort@s }} ->
-    {{ Γ ⊢s σ,,M : Δ, Sort@s }}.
+
+(** Substitution cases *)
+Lemma wf_sub_extend_typ {P : PtsSig} : forall {Δ : gctx P} {Γ Γ' σ M s},
+    {{ Δ ; Γ ⊢s σ : Γ' }} ->
+    {{ Δ ; Γ ⊢ M : Sort@s }} ->
+    {{ Δ ; Γ ⊢s σ,,M : Γ', Sort@s }}.
 Proof with mautosolve 3.
   intros.
   econstructor...
 Qed.
 
 #[export]
-Hint Resolve sub_extend_typ : mcpts.
+Hint Resolve wf_sub_extend_typ : mcpts.
 
-Lemma sub_eq_extend_cong_typ {P : PtsSig} : forall {Γ : ctx P} {σ σ' Δ M M' s},
-    {{ Γ ⊢s σ : Δ }} ->
-    {{ Γ ⊢s σ ≈ σ' : Δ }} ->
-    {{ Γ ⊢ M ≈ M' : Sort@s }} ->
-    {{ Γ ⊢s σ,,M ≈ σ',,M' : Δ, Sort@s }}.
+Lemma wf_sub_eq_extend_cong_typ {P : PtsSig} : forall {Δ : gctx P} {Γ Γ' σ σ' M M' s},
+    {{ Δ ; Γ ⊢s σ : Γ' }} ->
+    {{ Δ ; Γ ⊢s σ ≈ σ' : Γ' }} ->
+    {{ Δ ; Γ ⊢ M ≈ M' : Sort@s }} ->
+    {{ Δ ; Γ ⊢s σ,,M ≈ σ',,M' : Γ', Sort@s }}.
 Proof with mautosolve 3.
   intros.
-  assert {{ ⊢ Δ }} by mauto 2.
+  assert {{ Δ ⊢ Γ' }} by mauto 2.
   econstructor; mauto 2.
   eapply wf_exp_eq_conv; mauto 3.
+Qed.
+
+Lemma wf_sub_eq_extend_compose_typ {P : PtsSig} : forall {Δ : gctx P} {Γ Γ' Γ'' τ σ A s M},
+    {{ Δ ; Γ' ⊢s σ : Γ'' }} ->
+    {{ Δ ; Γ'' ⊢ A }} ->
+    {{ Δ ; Γ' ⊢ M : Sort@s }} ->
+    {{ Δ ; Γ ⊢s τ : Γ' }} ->
+    {{ Δ ; Γ ⊢s (σ,,M)∘τ ≈ (σ∘τ),,M[τ] : Γ'', Sort@s }}.
+Proof with mautosolve 3.
+  intros.
+  econstructor...
+Qed.
+
+Lemma wf_sub_eq_p_extend_typ {P : PtsSig} : forall {Δ : gctx P} {Γ Γ' σ M s},
+    {{ Δ ; Γ' ⊢s σ : Γ }} ->
+    {{ Δ ; Γ' ⊢ M : Sort@s }} ->
+    {{ Δ ; Γ' ⊢s Wk∘(σ,,M) ≈ σ : Γ }}.
+Proof with mautosolve 3.
+  intros.
+  econstructor...
+Qed.
+
+#[export]
+Hint Resolve wf_sub_eq_extend_cong_typ wf_sub_eq_extend_compose_typ wf_sub_eq_p_extend_typ : mcpts.
+
+Lemma wf_exp_eq_sub_sub_compose_cong_typ {P : PtsSig} : forall {Δ : gctx P} {Γ Γ'1 Γ'2 Γ'' σ τ σ' τ' A s},
+    {{ Δ ; Γ'' ⊢ A : Sort@s }} ->
+    {{ Δ ; Γ'1 ⊢s σ : Γ'' }} ->
+    {{ Δ ; Γ'2 ⊢s σ' : Γ'' }} ->
+    {{ Δ ; Γ ⊢s τ : Γ'1 }} ->
+    {{ Δ ; Γ ⊢s τ' : Γ'2 }} ->
+    {{ Δ ; Γ ⊢s σ∘τ ≈ σ'∘τ' : Γ'' }} ->
+    {{ Δ ; Γ ⊢ A[σ][τ] ≈ A[σ'][τ'] : Sort@s }}.
+Proof with mautosolve 3.
+  intros.
+  assert {{ Δ ; Γ ⊢ A[σ][τ] ≈ A[σ∘τ] : Sort@s }} by mauto 2.
+  assert {{ Δ ; Γ ⊢ A[σ∘τ] ≈ A[σ'∘τ'] : Sort@s }} by mauto 3.
+  enough {{ Δ ; Γ ⊢ A[σ'∘τ'] ≈ A[σ'][τ'] : Sort@s }}...
+Qed.
+
+#[export]
+Hint Resolve wf_exp_eq_sub_sub_compose_cong_typ : mcpts.
+
+
+
+
+(** This removes the extra premise {{ Γ ⊢ A : Sort@s }} in wf_vlookup, which we use in soundness *)
+(* Corollary wf_vlookup' {P} : forall {Γ : ctx P} {x A}, *)
+(*     {{ ⊢ Γ }} -> *)
+(*     {{ #x : A ∈ Γ }} -> *)
+(*     {{ Γ ⊢ #x : A }}. *)
+(* Proof. *)
+(*   intros. *)
+(*   assert {{ Γ ⊢ A }} by mauto 2. *)
+(*   econstructor; mauto 2. *)
+(* Qed. *)
+
+(* #[export] *)
+(* Hint Resolve wf_vlookup' : mcpts. *)
+(* #[export] *)
+(* Remove Hints wf_vlookup : mcpts. *)
+
+
+
+(** ** Lemmas for [exp] of [{{{ ℕ }}}] *)
+Lemma wf_typ_subtyp_nat_sub_left {P} : forall {Δ : gctx P} {Γ Γ' σ s} {r : Ru_nat P s},
+    {{ Δ ; Γ ⊢s σ : Γ' }} ->
+    {{ Δ ; Γ ⊢ ℕ[σ] ⊆ ℕ }}.
+Proof.
+  intros.
+  econstructor; mauto 4.
+Qed. 
+
+Lemma wf_typ_subtyp_nat_sub_right {P} : forall {Δ : gctx P} {Γ Γ' σ s} {r : Ru_nat P s},
+    {{ Δ ; Γ ⊢s σ : Γ' }} ->
+    {{ Δ ; Γ ⊢ ℕ ⊆ ℕ[σ] }}.
+Proof.
+  intros.
+  assert {{ Δ ⊢ Γ' }} by mauto 2.
+  assert {{ Δ ; Γ' ⊢ ℕ }} by mauto 3.
+  assert {{ Δ ; Γ ⊢ ℕ[σ] }} by mauto 3.
+  enough {{ Δ ; Γ ⊢ ℕ ≈ ℕ[σ] }} by mauto 2.
+  symmetry; mauto 3.
+Qed. 
+
+#[export]
+Hint Resolve wf_typ_subtyp_nat_sub_left wf_typ_subtyp_nat_sub_right : mcpts.
+
+
+Lemma wf_exp_sub_nat {P} : forall {Δ : gctx P} {Γ Γ' M σ s} {r : Ru_nat P s},
+    {{ Δ ; Γ' ⊢ M : ℕ }} ->
+    {{ Δ ; Γ ⊢s σ : Γ' }} ->
+    {{ Δ ; Γ ⊢ M[σ] : ℕ }}.
+Proof with mautosolve 3.
+  intros.
+  assert {{ Δ ⊢ Γ' }} by mauto 2.
+  assert {{ Δ ; Γ' ⊢ ℕ }} by mauto 3.
+  assert {{ Δ ; Γ ⊢ ℕ }} by mauto 3.
+  assert {{ Δ ; Γ ⊢ M[σ] : ℕ[σ] }} by mauto 3.  
+  econstructor; mauto 2.
+Qed.
+
+#[export]
+Hint Resolve wf_exp_sub_nat : mcpts.
+
+Lemma wf_exp_eq_sub_cong_nat1 {P} : forall {Δ : gctx P} {Γ Γ' M M' σ s} {r : Ru_nat P s},
+    {{ Δ ; Γ' ⊢ M ≈ M' : ℕ }} ->
+    {{ Δ ; Γ ⊢s σ : Γ' }} ->
+    {{ Δ ; Γ ⊢ M[σ] ≈ M'[σ] : ℕ }}.
+Proof with mautosolve 4.
+  intros.
+  assert {{ Δ ⊢ Γ' }} by mauto 2.
+  assert {{ Δ ; Γ' ⊢ ℕ }} by mauto 3.
+  assert {{ Δ ; Γ ⊢ ℕ }} by mauto 3.
   econstructor; mauto 3.
 Qed.
 
-Lemma sub_eq_extend_compose_typ {P : PtsSig} : forall {Γ : ctx P} {τ Γ' σ Γ'' A s M},
-    {{ Γ' ⊢s σ : Γ'' }} ->
-    {{ Γ'' ⊢ A }} ->
-    {{ Γ' ⊢ M : Sort@s }} ->
-    {{ Γ ⊢s τ : Γ' }} ->
-    {{ Γ ⊢s (σ,,M)∘τ ≈ (σ∘τ),,M[τ] : Γ'', Sort@s }}.
-Proof with mautosolve 3.
-  intros.
-  econstructor...
-Qed.
-
-Lemma sub_eq_p_extend_typ {P : PtsSig} : forall {Γ : ctx P} {σ Γ' M s},
-    {{ Γ' ⊢s σ : Γ }} ->
-    {{ Γ' ⊢ M : Sort@s }} ->
-    {{ Γ' ⊢s Wk∘(σ,,M) ≈ σ : Γ }}.
-Proof with mautosolve 3.
-  intros.
-  econstructor...
-Qed.
-
-#[export]
-Hint Resolve sub_eq_extend_cong_typ sub_eq_extend_compose_typ sub_eq_p_extend_typ : mcpts.
-
-Lemma exp_eq_sub_sub_compose_cong_typ {P : PtsSig} : forall {Γ : ctx P} {Δ Δ' Ψ σ τ σ' τ' A s},
-    {{ Ψ ⊢ A : Sort@s }} ->
-    {{ Δ ⊢s σ : Ψ }} ->
-    {{ Δ' ⊢s σ' : Ψ }} ->
-    {{ Γ ⊢s τ : Δ }} ->
-    {{ Γ ⊢s τ' : Δ' }} ->
-    {{ Γ ⊢s σ∘τ ≈ σ'∘τ' : Ψ }} ->
-    {{ Γ ⊢ A[σ][τ] ≈ A[σ'][τ'] : Sort@s }}.
-Proof with mautosolve 3.
-  intros.
-  assert {{ Γ ⊢ A[σ][τ] ≈ A[σ∘τ] : Sort@s }} by mauto 2.
-  assert {{ Γ ⊢ A[σ∘τ] ≈ A[σ'∘τ'] : Sort@s }} by mauto 3.
-  enough {{ Γ ⊢ A[σ'∘τ'] ≈ A[σ'][τ'] : Sort@s }}...
-Qed.
-
-#[export]
-Hint Resolve exp_eq_sub_sub_compose_cong_typ : mcpts.
-
-Lemma typ_eq_sub_sub_compose_cong_typ {P : PtsSig} : forall {Γ : ctx P} {Δ Δ' Ψ σ τ σ' τ' A},
-    {{ Ψ ⊢ A }} ->
-    {{ Δ ⊢s σ : Ψ }} ->
-    {{ Δ' ⊢s σ' : Ψ }} ->
-    {{ Γ ⊢s τ : Δ }} ->
-    {{ Γ ⊢s τ' : Δ' }} ->
-    {{ Γ ⊢s σ∘τ ≈ σ'∘τ' : Ψ }} ->
-    {{ Γ ⊢ A[σ][τ] ≈ A[σ'][τ'] }}.
-Proof with mautosolve 3.
-  intros.
-  assert {{ Γ ⊢ A[σ][τ] ≈ A[σ∘τ] }} by mauto 3.
-  assert {{ Γ ⊢ A[σ∘τ] ≈ A[σ'∘τ'] }} by mauto 3.
-  enough {{ Γ ⊢ A[σ'∘τ'] ≈ A[σ'][τ'] }}...
-Qed.
-
-#[export]
-Hint Resolve typ_eq_sub_sub_compose_cong_typ : mcpts.
-
-
-(** *** Other Tedious Lemmas *)
-
-Lemma sub_eq_weaken_var0_id {P : PtsSig} : forall {Γ : ctx P} {A},
-    {{ Γ ⊢ A }} ->
-    {{ Γ, A ⊢s Wk,,#0 ≈ Id : Γ, A }}.
-Proof with mautosolve 4.
-  intros * ?.
-  assert {{ ⊢ Γ }} by mauto 2.
-  assert {{ Γ ⊢ A }} by mauto 2.
-  assert {{ ⊢ Γ, A }} by mauto 3.
-  assert {{ Γ, A ⊢s Wk : Γ }} by mauto 2.
-  assert {{ Γ, A ⊢s (Wk∘Id),,#0[Id] ≈ Id : Γ, A }} by mauto.
-  assert {{ Γ, A ⊢s Wk ≈ Wk∘Id : Γ }} by mauto.
-  assert {{ Γ, A ⊢s Wk,,#0 ≈ Wk∘Id,,#0[Id] : Γ, A }} by (eapply wf_sub_eq_extend_cong; mauto 4).
-  enough {{ Γ, A ⊢ #0 ≈ #0[Id] : A[Wk] }} by (etransitivity; mauto 3).
-  symmetry; econstructor; econstructor; mauto 2.
-Qed.
-
-#[export]
-Hint Resolve sub_eq_weaken_var0_id : mcpts.
-#[export]
-Hint Rewrite -> @sub_eq_weaken_var0_id using mauto 4 : mcpts.
-
-Lemma exp_eq_sub_sub_compose_cong_sorted {P : PtsSig} : forall {Γ : ctx P} {Δ Δ' Ψ σ τ σ' τ' M A s},
-    {{ Ψ ⊢ A : Sort@s }} ->
-    {{ Ψ ⊢ M : A }} ->
-    {{ Δ ⊢s σ : Ψ }} ->
-    {{ Δ' ⊢s σ' : Ψ }} ->
-    {{ Γ ⊢s τ : Δ }} ->
-    {{ Γ ⊢s τ' : Δ' }} ->
-    {{ Γ ⊢s σ∘τ ≈ σ'∘τ' : Ψ }} ->
-    {{ Γ ⊢ M[σ][τ] ≈ M[σ'][τ'] : A[σ∘τ] }}.
-Proof with mautosolve 3.
-  intros.
-  assert {{ Γ ⊢ A[σ∘τ] ≈ A[σ'∘τ'] }} by mauto.
-  assert {{ Γ ⊢ M[σ][τ] ≈ M[σ∘τ] : A[σ∘τ] }} by mauto 4.
-  assert {{ Γ ⊢ M[σ∘τ] ≈ M[σ'∘τ'] : A[σ∘τ] }} by mauto 4.
-  assert {{ Γ ⊢ M[σ'∘τ'] ≈ M[σ'][τ'] : A[σ'∘τ'] }} by mauto.
-  enough {{ Γ ⊢ M[σ'∘τ'] ≈ M[σ'][τ'] : A[σ∘τ] }} by mauto.
-  eapply wf_exp_eq_conv; mauto 4.
-  enough {{ Γ ⊢ A[σ'∘τ'] ≈ A[σ∘τ] }} by (econstructor; mauto 4).
-  mauto 4.
-Qed.
-
-#[export]
-Hint Resolve exp_eq_sub_sub_compose_cong_sorted : mcpts.
-
-Lemma exp_eq_sub_sub_compose_cong {P : PtsSig} : forall {Γ : ctx P} {Δ Δ' Ψ σ τ σ' τ' M A},
-    {{ Ψ ⊢ A }} ->
-    {{ Ψ ⊢ M : A }} ->
-    {{ Δ ⊢s σ : Ψ }} ->
-    {{ Δ' ⊢s σ' : Ψ }} ->
-    {{ Γ ⊢s τ : Δ }} ->
-    {{ Γ ⊢s τ' : Δ' }} ->
-    {{ Γ ⊢s σ∘τ ≈ σ'∘τ' : Ψ }} ->
-    {{ Γ ⊢ M[σ][τ] ≈ M[σ'][τ'] : A[σ∘τ] }}.
-Proof with mautosolve 3.
-  intros.
-  assert {{ Γ ⊢ A[σ∘τ] ≈ A[σ'∘τ'] }} by mauto.
-  assert {{ Γ ⊢ M[σ][τ] ≈ M[σ∘τ] : A[σ∘τ] }} by mauto.
-  assert {{ Γ ⊢ M[σ∘τ] ≈ M[σ'∘τ'] : A[σ∘τ] }} by mauto.
-  assert {{ Γ ⊢ M[σ'∘τ'] ≈ M[σ'][τ'] : A[σ'∘τ'] }} by mauto.
-  enough {{ Γ ⊢ M[σ'∘τ'] ≈ M[σ'][τ'] : A[σ∘τ] }} by mauto.
-  eapply wf_exp_eq_conv; mauto 4.
-  enough {{ Γ ⊢ A[σ'∘τ'] ≈ A[σ∘τ] }} by (econstructor; mauto 4).
-  mauto 4.
-Qed.
-
-#[export]
-Hint Resolve exp_eq_sub_sub_compose_cong : mcpts.
-
-Lemma ctxeq_ctx_lookup {P : PtsSig} : forall {Γ : ctx P} {Δ A x},
-    {{ ⊢ Γ ≈ Δ }} ->
-    {{ #x : A ∈ Γ }} ->
-    exists B,
-      {{ #x : B ∈ Δ }} /\
-        {{ Γ ⊢ A ≈ B }} /\
-        {{ Δ ⊢ A ≈ B }} /\
-        {{ Δ ⊢ A }}.
-Proof with (repeat eexists; mautosolve 3).
-  intros * HΓΔ Hx.
-  assert {{ ⊢ Γ }} by mauto 2.
-  assert {{ Γ ⊢ A }} by mauto 3.
-  gen Δ Hx.
-  induction 1 as [|* ? IHHx]; inversion_clear 1 as [|? ? ? ? HΓΔ'];
-    assert {{ ⊢ Δ0 }} by mauto 2.
-  - assert {{ Γ, A ⊢s Wk : Γ }} by mauto 2.
-    assert {{ Δ0, A' ⊢s Wk : Δ0 }} by mauto 3.
-    eexists.
-    do 3 (split; mauto 3).
-  - specialize (IHHx ltac:(mauto 2) ltac:(mauto 3) _ HΓΔ').
-    destruct_conjs.
-    assert {{ Γ, B ⊢s Wk : Γ }} by mauto 2.
-    assert {{ Δ0, A' ⊢s Wk : Δ0 }} by mauto 3.
-    eexists.
-    do 3 (split; mauto 3).
-Qed.
-
-#[export]
-Hint Resolve ctxeq_ctx_lookup : mcpts.
-
-Lemma sub_id_on_typ_sorted {P : PtsSig} : forall {Γ : ctx P} {M A s},
-    {{ Γ ⊢ A : Sort@s }} ->
-    {{ Γ ⊢ M : A }} ->
-    {{ Γ ⊢ M : A[Id] }}.
-Proof with mautosolve 3.
-  intros.
-  assert {{ ⊢ Γ }} by mauto 2.
-  eapply wf_conv; mauto 4.
-Qed.
-
-#[export]
-Hint Resolve sub_id_on_typ_sorted : mcpts.
-
-Lemma sub_id_on_typ {P : PtsSig} : forall {Γ : ctx P} {M A},
-    {{ Γ ⊢ A }} ->
-    {{ Γ ⊢ M : A }} ->
-    {{ Γ ⊢ M : A[Id] }}.
-Proof with mautosolve 3.
-  intros.
-  assert {{ ⊢ Γ }} by mauto 2.
-  eapply wf_conv; mauto 3.
-Qed.
-
-#[export]
-Hint Resolve sub_id_on_typ : mcpts.
-
-
-Lemma sub_id_extend {P : PtsSig} : forall {Γ : ctx P} {M A},
-    {{ Γ ⊢ A }} ->
-    {{ Γ ⊢ M : A }} ->
-    {{ Γ ⊢s Id,,M : Γ, A }}.
+Lemma wf_exp_eq_sub_cong_nat2 {P} : forall {Δ : gctx P} {Γ Γ' M σ τ s} {r : Ru_nat P s},
+    {{ Δ ; Γ' ⊢ M : ℕ }} ->
+    {{ Δ ; Γ ⊢s σ : Γ' }} ->
+    {{ Δ ; Γ ⊢s σ ≈ τ : Γ' }} ->
+    {{ Δ ; Γ ⊢ M[σ] ≈ M[τ] : ℕ }}.
 Proof with mautosolve 4.
   intros.
-  econstructor...
+  assert {{ Δ ⊢ Γ' }} by mauto 2.
+  assert {{ Δ ; Γ' ⊢ ℕ }} by mauto 3.
+  assert {{ Δ ; Γ ⊢ ℕ }} by mauto 3.
+  econstructor; mauto 3.
 Qed.
 
 #[export]
-Hint Resolve sub_id_extend : mcpts.
-
-Lemma sub_eq_id_on_typ_sorted {P : PtsSig} : forall {Γ : ctx P} {M M' A s},
-    {{ Γ ⊢ A : Sort@s }} ->
-    {{ Γ ⊢ M ≈ M' : A }} ->
-    {{ Γ ⊢ M ≈ M' : A[Id] }}.
+Hint Resolve wf_exp_eq_sub_cong_nat1 wf_exp_eq_sub_cong_nat2 : mcpts.
+  
+Lemma wf_exp_eq_sub_compose_nat {P} : forall {Δ : gctx P} {Γ Γ' Γ'' M σ τ s} {r : Ru_nat P s},
+    {{ Δ ; Γ'' ⊢ M : ℕ }} ->
+    {{ Δ ; Γ' ⊢s σ : Γ'' }} ->
+    {{ Δ ; Γ ⊢s τ : Γ'}} ->
+    {{ Δ ; Γ ⊢ M[σ][τ] ≈ M[σ∘τ] : ℕ }}.
 Proof with mautosolve 4.
   intros.
-  assert {{ ⊢ Γ }} by mauto 3.
-  eapply wf_eq_conv; mauto 3;
-    econstructor...
+  assert {{ Δ ⊢ Γ'' }} by mauto 2.
+  assert {{ Δ ⊢ Γ' }} by mauto 2.
+  assert {{ Δ ; Γ'' ⊢ ℕ }} by mauto 3.
+  assert {{ Δ ; Γ' ⊢ ℕ }} by mauto 3.
+  assert {{ Δ ; Γ ⊢ ℕ }} by mauto 3.
+  assert {{ Δ ; Γ ⊢ M[σ∘τ] ≈ M[σ][τ] : ℕ[σ∘τ] }} by mauto 3.
+  econstructor; mauto 3.
 Qed.
 
 #[export]
-Hint Resolve sub_eq_id_on_typ_sorted : mcpts.
+Hint Resolve wf_exp_eq_sub_compose_nat : mcpts.
 
-Lemma sub_eq_id_on_typ {P : PtsSig} : forall {Γ : ctx P} {M M' A},
-    {{ Γ ⊢ A }} ->
-    {{ Γ ⊢ M ≈ M' : A }} ->
-    {{ Γ ⊢ M ≈ M' : A[Id] }}.
+Lemma wf_exp_eq_nat_sub_sub {P} : forall {Δ : gctx P} {Γ Γ' Γ'' σ τ s} {r : Ru_nat P s},
+    {{ Δ ; Γ' ⊢s σ : Γ'' }} ->
+    {{ Δ ; Γ ⊢s τ : Γ' }} ->
+    {{ Δ ; Γ ⊢ ℕ[σ][τ] ≈ ℕ : Sort@s }}.
+Proof. mauto. Qed.
+
+#[export]
+Hint Resolve wf_exp_eq_nat_sub_sub : mcpts.
+
+Lemma wf_exp_eq_nat_sub_sub_to_nat_sub {P} : forall {Δ : gctx P} {Γ Γ' Γ''1 Γ''2 σ τ σ' s} {r : Ru_nat P s},
+    {{ Δ ; Γ' ⊢s σ : Γ''1 }} ->
+    {{ Δ ; Γ ⊢s τ : Γ' }} ->
+    {{ Δ ; Γ ⊢s σ' : Γ''2 }} ->
+    {{ Δ ; Γ ⊢ ℕ[σ][τ] ≈ ℕ[σ'] : Sort@s}}.
+Proof. mauto. Qed.
+
+#[export]
+Hint Resolve wf_exp_eq_nat_sub_sub_to_nat_sub : mcpts.
+
+Lemma wf_exp_eq_sub_compose_weaken_extend_nat {P} : forall {Δ : gctx P} {Γ Γ' σ M B N s} {r : Ru_nat P s},
+    {{ Δ ; Γ ⊢s σ : Γ' }} ->
+    {{ Δ ; Γ' ⊢ M : ℕ }} ->
+    {{ Δ ; Γ' ⊢ B }} ->
+    {{ Δ ; Γ ⊢ N : B[σ] }} ->
+    {{ Δ ; Γ ⊢ M[Wk][σ,,N] ≈ M[σ] : ℕ }}.
 Proof with mautosolve 4.
   intros.
-  assert {{ ⊢ Γ }} by mauto 3.
-  eapply wf_exp_eq_conv; mauto 3;
-    econstructor...
+  assert {{ Δ ⊢ Γ' }} by mauto 2.
+  assert {{ Δ; Γ', B ⊢s Wk : Γ' }} by mauto 3.
+  assert {{ Δ ; Γ ⊢s σ,,N : Γ', B }} by mauto 2.
+  transitivity {{{ M[Wk∘(σ,,N)] }}}...
 Qed.
 
 #[export]
-Hint Resolve sub_eq_id_on_typ : mcpts.
+Hint Resolve wf_exp_eq_sub_compose_weaken_extend_nat : mcpts.
 
-Lemma sub_eq_id_extend_cong_sorted {P : PtsSig} : forall {Γ : ctx P} {M M' A s},
-    {{ Γ ⊢ A : Sort@s }} ->
-    {{ Γ ⊢ M ≈ M' : A }} ->
-    {{ Γ ⊢s Id,,M ≈ Id,,M' : Γ, A }}.
+Lemma wf_exp_eq_sub_compose_weaken_id_extend_nat {P} : forall {Δ : gctx P} {Γ M B N s} {r : Ru_nat P s},
+    {{ Δ ; Γ ⊢ M : ℕ }} ->
+    {{ Δ ; Γ ⊢ B }} ->
+    {{ Δ ; Γ ⊢ N : B }} ->
+    {{ Δ ; Γ ⊢ M[Wk][Id,,N] ≈ M : ℕ }}.
 Proof with mautosolve 3.
+  intros.
+  assert {{ Δ ⊢ Γ }} by mauto 2.
+  assert {{ Δ ; Γ ⊢ B[Id] }} by mauto 3.
+  assert {{ Δ ; Γ ⊢ B ≈ B[Id] }} by mauto 4.
+  assert {{ Δ ; Γ ⊢ N : B[Id] }} by mauto 4.
+  transitivity {{{ M[Id] }}}...
+Qed.
+
+#[export]
+Hint Resolve wf_exp_eq_sub_compose_weaken_id_extend_nat : mcpts.
+
+Lemma wf_exp_eq_sub_compose_double_weaken_double_extend_nat {P} : forall {Δ : gctx P} {Γ Γ' σ M B N C L s} {r : Ru_nat P s},
+    {{ Δ ; Γ ⊢s σ : Γ' }} ->
+    {{ Δ ; Γ' ⊢ M : ℕ }} ->
+    {{ Δ ; Γ' ⊢ B  }} ->
+    {{ Δ ; Γ ⊢ N : B[σ] }} ->
+    {{ Δ ; Γ', B ⊢ C }} ->
+    {{ Δ ; Γ ⊢ L : C[σ,,N] }} ->
+    {{ Δ ;Γ ⊢ M[Wk∘Wk][σ,,N,,L] ≈ M[σ] : ℕ }}.
+Proof with mautosolve 3.
+  intros.
+  assert {{ Δ ⊢ Γ' }} by mauto 2.
+  assert {{ Δ ; Γ', B ⊢s Wk : Γ' }} by mauto 3.
+  assert {{ Δ ; Γ', B, C ⊢s Wk : Γ', B }} by mauto 4.
+  assert {{ Δ ; Γ ⊢s σ,,N : Γ', B }} by mauto 2.
+  assert {{ Δ ; Γ ⊢s σ,,N,,L : Γ', B, C }} by mauto 2.
+  transitivity {{{ M[Wk][Wk][σ,,N,,L] }}}; [econstructor; mautosolve 3|].
+  transitivity {{{ M[Wk][σ,,N] }}}...
+Qed.
+
+#[export]
+Hint Resolve wf_exp_eq_sub_compose_double_weaken_double_extend_nat : mcpts.
+
+Lemma wf_exp_eq_sub_compose_double_weaken_id_double_extend_nat {P} : forall {Δ : gctx P} {Γ M B N C L s } {r : Ru_nat P s},
+    {{ Δ ; Γ ⊢ M : ℕ }} ->
+    {{ Δ ; Γ ⊢ B }} ->
+    {{ Δ ; Γ ⊢ N : B }} ->
+    {{ Δ ; Γ, B ⊢ C }} ->
+    {{ Δ ; Γ ⊢ L : C[Id,,N] }} ->
+    {{ Δ ; Γ ⊢ M[Wk∘Wk][Id,,N,,L] ≈ M : ℕ }}.
+Proof with mautosolve 3.
+  intros.
+  assert {{ Δ ⊢ Γ }} by mauto 2.
+  assert {{ Δ ; Γ ⊢ B[Id] }} by mauto 3.
+  assert {{ Δ ; Γ ⊢ B ≈ B[Id] }} by mauto 4.
+  assert {{ Δ ; Γ ⊢ N : B[Id] }} by mauto 4.
+  transitivity {{{ M[Id] }}}...
+Qed.
+
+#[export]
+Hint Resolve wf_exp_eq_sub_compose_double_weaken_id_double_extend_nat : mcpts.
+
+Lemma vlookup_0_nat {P} : forall {Δ : gctx P} {Γ s} {r : Ru_nat P s},
+    {{ Δ ⊢ Γ }} ->
+    {{ Δ ; Γ, ℕ ⊢ #0 : ℕ }}.
+Proof with mautosolve 3.
+  intros.
+  assert {{ Δ ; Γ ⊢ ℕ }} by mauto 3.
+  assert {{ Δ ; Γ, ℕ ⊢s Wk : Γ }} by mauto 3.
+  eapply wf_exp_conv...
+Qed.
+
+Lemma vlookup_1_nat {P} : forall {Δ : gctx P} {Γ A s} {r : Ru_nat P s},
+    {{ Δ ; Γ, ℕ ⊢ A }} ->
+    {{ Δ ; Γ, ℕ, A ⊢ #1 : ℕ }}.
+Proof with mautosolve 3.
+  intros.
+  assert {{ Δ ⊢ Γ }} by mauto 3.
+  assert {{ Δ ; Γ ⊢ ℕ : Sort@s }} by mauto 2.
+  assert {{ Δ ; Γ, ℕ ⊢s Wk : Γ }} by mauto 4.
+  assert {{ Δ ; Γ, ℕ, A ⊢s Wk : Γ, ℕ }} by mauto 5.
+  assert {{ Δ ; Γ, ℕ, A ⊢ #1 : ℕ[Wk][Wk] }} by mauto 4.
+  eapply wf_exp_conv_exp_eq; mauto 3.
+Qed.
+
+#[export]
+Hint Resolve vlookup_0_nat vlookup_1_nat : mcpts.
+
+Lemma wf_exp_sub_nat_helper {P} : forall {Δ : gctx P} {Γ Γ' σ M s} {r : Ru_nat P s},
+    {{ Δ ; Γ ⊢s σ : Γ' }} ->
+    {{ Δ ; Γ ⊢ M : ℕ }} ->
+    {{ Δ ; Γ ⊢ M : ℕ[σ] }}.
+Proof.
+  intros.
+  assert {{ Δ ⊢ Γ' }} by mauto 2.
+  assert {{ Δ ; Γ' ⊢ ℕ }} by mauto 3.
+  assert {{ Δ ; Γ ⊢ ℕ }} by mauto 3.
+  assert {{ Δ ; Γ ⊢ ℕ ⊆ ℕ[σ] }} by mauto 2.
+  mauto 3.
+Qed.
+
+#[export]
+Hint Resolve wf_exp_sub_nat_helper : mcpts.
+
+Lemma wf_exp_eq_var_0_sub_nat {P} : forall {Δ : gctx P} {Γ Γ' σ M s} {r : Ru_nat P s},
+    {{ Δ ; Γ ⊢s σ : Γ' }} ->
+    {{ Δ ; Γ ⊢ M : ℕ }} ->
+    {{ Δ ; Γ ⊢ #0[σ,,M] ≈ M : ℕ }}.
+Proof with mautosolve 3.
+  intros.
+  assert {{ Δ ⊢ Γ' }} by mauto 2.
+  assert {{ Δ ; Γ' ⊢ ℕ }} by mauto 3.
+  eapply wf_exp_eq_conv...
+Qed.
+
+Lemma wf_exp_eq_var_1_sub_nat {P} : forall {Δ : gctx P} {Γ Γ' σ A M s} {r : Ru_nat P s},
+    {{ Δ ; Γ ⊢s σ : Γ' }} ->
+    {{ Δ ; Γ' ⊢ A }} ->
+    {{ Δ ; Γ ⊢ M : A[σ] }} ->
+    {{ #0 : ℕ[Wk] ∈ Γ' }} ->
+    {{ Δ ; Γ ⊢ #1[σ,,M] ≈ #0[σ] : ℕ }}.
+Proof with mautosolve 4.
+  inversion 5 as [? Γ''|]; subst.
+  assert {{ Δ ; Γ ⊢ #1[σ,,M] ≈ #0[σ] : ℕ[Wk][σ] }} by mauto 3.
+  eapply wf_exp_eq_conv; mauto 3.
+  econstructor; mauto.
+Qed.
+
+#[export]
+Hint Resolve wf_exp_eq_var_0_sub_nat wf_exp_eq_var_1_sub_nat : mcpts.
+
+Lemma wf_exp_eq_var_0_weaken_nat {P} : forall {Δ : gctx P} {Γ A s} {r : Ru_nat P s},
+    {{ Δ ⊢ Γ, A }} ->
+    {{ #0 : ℕ[Wk] ∈ Γ }} ->
+    {{ Δ ; Γ, A ⊢ #0[Wk] ≈ #1 : ℕ }}.
+Proof with mautosolve 4.
+  inversion 2; subst.
+  inversion 1; subst.
+  assert {{ Δ ; Γ0, ℕ, A ⊢ #0[Wk] ≈ #1 : ℕ[Wk][Wk] }} by mauto 3.
+  eapply wf_exp_eq_conv; mauto 3.
+  econstructor; mauto.
+Qed.
+
+#[export]
+Hint Resolve wf_exp_eq_var_0_weaken_nat : mcpts.
+
+(** *** Substitution cases *)
+Lemma wf_sub_extend_nat {P} : forall {Δ : gctx P} {Γ Γ' σ M s} {r : Ru_nat P s},
+    {{ Δ ; Γ ⊢s σ : Γ' }} ->
+    {{ Δ ; Γ ⊢ M : ℕ }} ->
+    {{ Δ ; Γ ⊢s σ,,M : Γ', ℕ }}.
+Proof with mautosolve 4.
   intros.
   econstructor...
 Qed.
 
 #[export]
-Hint Resolve sub_eq_id_extend_cong_sorted : mcpts.
+Hint Resolve wf_sub_extend_nat : mcpts.
 
-Lemma sub_eq_p_id_extend {P : PtsSig} : forall {Γ : ctx P} {M A},
-    {{ Γ ⊢ A }} ->
-    {{ Γ ⊢ M : A }} ->
-    {{ Γ ⊢s Wk∘(Id,,M) ≈ Id : Γ }}.
-Proof with mautosolve 3.
+Lemma wf_sub_eq_extend_cong_nat {P} : forall {Δ : gctx P} {Γ Γ' σ σ' M M' s} {r : Ru_nat P s},
+    {{ Δ ; Γ ⊢s σ : Γ' }} ->
+    {{ Δ ; Γ ⊢s σ ≈ σ' : Γ' }} ->
+    {{ Δ ; Γ ⊢ M ≈ M' : ℕ }} ->
+    {{ Δ ; Γ ⊢s σ,,M ≈ σ',,M' : Γ', ℕ }}.
+Proof with mautosolve 4.
+  intros.
+  econstructor; mauto 4.
+  assert {{ Δ ⊢ Γ }} by mauto 2.
+  assert {{ Δ ; Γ ⊢ ℕ ≈ ℕ[σ] : Sort@s }} by mauto 3.
+  assert {{ Δ ; Γ' ⊢ ℕ : Sort@s }} by mauto 3.
+  assert {{ Δ ; Γ ⊢ ℕ[σ] : Sort@s }} by mauto 3.
+  assert {{ Δ ; Γ ⊢ ℕ ⊆ ℕ[σ] }} by mauto 2.
+  eapply wf_exp_eq_conv; mauto 3.
+Qed.
+
+Lemma wf_sub_eq_extend_compose_nat {P} : forall {Δ : gctx P} {Γ Γ' Γ'' τ σ M s} {r : Ru_nat P s},
+    {{ Δ ; Γ' ⊢s σ : Γ'' }} ->
+    {{ Δ ; Γ' ⊢ M : ℕ }} ->
+    {{ Δ ; Γ ⊢s τ : Γ' }} ->
+    {{ Δ ; Γ ⊢s (σ,,M)∘τ ≈ (σ∘τ),,M[τ] : Γ'', ℕ }}.
+Proof with mautosolve 4.
   intros.
   econstructor...
 Qed.
 
-#[export]
-Hint Resolve sub_eq_p_id_extend : mcpts.
-#[export]
-Hint Rewrite -> @sub_eq_p_id_extend using mauto 4 : mcpts.
-
-Lemma sub_q {P : PtsSig} : forall {Γ : ctx P} {A σ Δ},
-    {{ Δ ⊢ A }} ->
-    {{ Γ ⊢s σ : Δ }} ->
-    {{ Γ, A[σ] ⊢s q σ : Δ, A }}.
-Proof with mautosolve 3.
-  intros.
-  assert {{ ⊢ Γ }} by mauto 2.
-  assert {{ Γ ⊢ A[σ] }} by mauto 3.
-  assert {{ Γ, A[σ] ⊢s Wk : Γ }} by mauto 3.
-  assert {{ Γ, A[σ] ⊢ #0 : A[σ][Wk] }} by mauto 3.
-  econstructor; mauto 2.
-  eapply wf_conv; mauto 3.
-Qed.
-
-Lemma sub_q_typ {P : PtsSig} : forall {Γ : ctx P} {σ Δ s},
-    {{ Γ ⊢s σ : Δ }} ->
-    {{ Γ, Sort@s ⊢s q σ : Δ, Sort@s }}.
-Proof with mautosolve 3.
-
-  intros.
-  assert {{ ⊢ Γ }} by mauto 3.
-  assert {{ Γ, Sort@s ⊢s Wk : Γ }} by mauto 4.
-  assert {{ Γ, Sort@s ⊢s σ∘Wk : Δ }} by mauto 4.
-  assert {{ Γ, Sort@s ⊢ Sort@s[Wk] ≈ Sort@s }} by mauto 4.
-  assert {{ Γ, Sort@s ⊢ #0 : Sort@s }} by mauto 3.
-  econstructor...
-Qed.
-
-#[export]
-Hint Resolve sub_q sub_q_typ : mcpts.
-
-Lemma sub_q_nat {P} : forall {Γ : ctx P} {σ Δ s} {r : Ru_nat P s},
-    {{ Γ ⊢s σ : Δ }} ->
-    {{ Γ, ℕ ⊢s q σ : Δ, ℕ }}.
-Proof with mautosolve 3.
-  intros.
-  assert {{ ⊢ Γ }} by mauto 3.
-  assert {{ Γ, ℕ ⊢s Wk : Γ }} by mauto 4.
-  assert {{ Γ, ℕ ⊢s σ∘Wk : Δ }} by mauto 4.
-  assert {{ Γ, ℕ ⊢ #0 : ℕ }}...
-Qed.
-
-#[export]
-Hint Resolve sub_q sub_q_typ sub_q_nat : mcpts.
-
-Lemma exp_eq_var_1_sub_q_sigma_nat {P} : forall {Γ : ctx P} {A σ Δ s} {r : Ru_nat P s},
-    {{ Δ, ℕ ⊢ A }} ->
-    {{ Γ ⊢s σ : Δ }} ->
-    {{ Γ, ℕ, A[q σ] ⊢ #1[q (q σ)] ≈ #1 : ℕ }}.
-Proof with mautosolve 3.
-  intros.
-  assert {{ Γ, ℕ ⊢s q σ : Δ, ℕ }} by mauto 3.
-  assert {{ Γ, ℕ ⊢ A[q σ] }} by mauto 4.
-  assert {{ ⊢ Γ, ℕ, A[q σ] }} by (econstructor; mauto 2).
-  assert {{ Δ, ℕ ⊢ #0 : ℕ }} by mauto 3.
-  assert {{ Γ, ℕ, A[q σ] ⊢ #0 : A[q σ][Wk] }} by mauto 3.
-  assert {{ Γ, ℕ, A[q σ] ⊢s q σ∘Wk : Δ, ℕ }} by mauto 3.
-  assert {{ Γ, ℕ, A[q σ] ⊢ A[q σ∘Wk] ≈ A[q σ][Wk]  }} by mauto 4.
-  assert {{ Γ, ℕ, A[q σ] ⊢ #0 : A[q σ∘Wk] }} by (eapply wf_conv; mauto 4).
-  assert {{ Γ, ℕ, A[q σ] ⊢s q σ∘Wk : Δ, ℕ }} by mauto 3.
-  assert {{ Γ, ℕ, A[q σ] ⊢ #1[q (q σ)] ≈ #0[q σ∘Wk] : ℕ }} by mauto 3.
-  assert {{ Γ, ℕ, A[q σ] ⊢ #0[q σ∘Wk] ≈ #0[q σ][Wk] : ℕ }} by mauto 4.
-  assert {{ Γ, ℕ ⊢s σ∘Wk : Δ }} by mauto 4.
-  assert {{ Γ, ℕ ⊢ #0 : ℕ }} by mauto 3.
-  assert {{ Γ, ℕ ⊢ #0 : ℕ[σ∘Wk] }} by mauto 3.
-  assert {{ Γ, ℕ ⊢ #0[q σ] ≈ #0 : ℕ }} by mauto 3.
-  assert {{ Γ, ℕ, A[q σ] ⊢ #0[q σ][Wk] ≈ #0[Wk] : ℕ }} by mauto 3.
-  etransitivity; [eassumption |].
-  etransitivity...
-Qed.
-
-#[export]
-Hint Resolve exp_eq_var_1_sub_q_sigma_nat : mcpts.
-
-Lemma sub_id_extend_zero {P} : forall {Γ : ctx P} {s} {r : Ru_nat P s},
-    {{ ⊢ Γ }} ->
-    {{ Γ ⊢s Id,,zero : Γ, ℕ }}.
-Proof. mauto 4. Qed.
-
-Lemma sub_weak_compose_weak_extend_succ_var_1 {P} : forall {Γ : ctx P} {A s} {r : Ru_nat P s},
-    {{ Γ, ℕ ⊢ A }} ->
-    {{ Γ, ℕ, A ⊢s Wk∘Wk,,succ #1 : Γ, ℕ }}.
-Proof with mautosolve 4.
-  intros.
-  assert {{ Γ, ℕ, A ⊢s Wk : Γ, ℕ  }} by mauto 4.
-  enough {{ Γ, ℕ, A ⊢s Wk∘Wk : Γ }}...
-Qed.
-
-Lemma sub_eq_id_extend_compose_sigma {P : PtsSig} : forall {Γ : ctx P} {M A σ Δ},
-    {{ Γ ⊢s σ : Δ }} ->
-    {{ Δ ⊢ A }} ->
-    {{ Δ ⊢ M : A }} ->
-    {{ Γ ⊢s (Id,,M)∘σ ≈ σ,,M[σ] : Δ, A }}.
-Proof with mautosolve 4.
-  intros.
-  assert {{ Δ ⊢s Id : Δ }} by mauto 3.
-  assert {{ Δ ⊢ M : A[Id] }} by mauto.
-  assert {{ Γ ⊢s (Id,,M)∘σ ≈ (Id∘σ),,M[σ] : Δ, A }} by mauto 3.
-  assert {{ Γ ⊢ M[σ] : A[Id][σ] }} by mauto.
-  assert {{ Γ ⊢ A[Id][σ] ≈ A[Id∘σ] }} by (symmetry; mauto 3).
-  assert {{ Γ ⊢ A[Id∘σ] }} by mauto 4.
-  assert {{ Γ ⊢ A[Id][σ] ⊆ A[Id∘σ] }} by mauto 4.
-  assert {{ Γ ⊢ M[σ] : A[Id∘σ] }} by (eapply wf_exp_conv; mauto 4).
-  enough {{ Γ ⊢ M[σ] ≈ M[σ] : A[Id∘σ] }}...
-Qed.
-
-#[export]
-Hint Resolve sub_eq_id_extend_compose_sigma : mcpts.
-
-Lemma sub_eq_sigma_compose_weak_id_extend {P : PtsSig} : forall {Γ : ctx P} {M A σ Δ},
-    {{ Γ ⊢ A }} ->
-    {{ Γ ⊢s σ : Δ }} ->
-    {{ Γ ⊢ M : A }} ->
-    {{ Γ ⊢s (σ∘Wk)∘(Id,,M) ≈ σ : Δ }}.
+Lemma wf_sub_eq_p_extend_nat {P} : forall {Δ : gctx P} {Γ Γ' σ M s} {r : Ru_nat P s},
+    {{ Δ ; Γ' ⊢s σ : Γ }} ->
+    {{ Δ ; Γ' ⊢ M : ℕ }} ->
+    {{ Δ ; Γ' ⊢s Wk∘(σ,,M) ≈ σ : Γ }}.
 Proof with mautosolve.
   intros.
-  assert {{ Γ ⊢s Id,,M : Γ, A }} by mauto.
-  assert {{ Γ ⊢s (σ∘Wk)∘(Id,,M) ≈ σ∘(Wk∘(Id,,M)) : Δ }} by mauto 4.
-  assert {{ Γ ⊢s Wk∘(Id,,M) ≈ Id : Γ }} by mauto.
-  enough {{ Γ ⊢s σ∘(Wk∘ (Id,,M)) ≈ σ∘Id : Δ }} by mauto.
+  assert {{ Δ ; Γ ⊢ ℕ : Sort@s }} by mauto 3.
   econstructor...
 Qed.
 
 #[export]
-Hint Resolve sub_eq_sigma_compose_weak_id_extend : mcpts.
+Hint Resolve wf_sub_eq_extend_cong_nat wf_sub_eq_extend_compose_nat wf_sub_eq_p_extend_nat : mcpts.
 
-Lemma sub_eq_q_sigma_id_extend {P : PtsSig} : forall {Γ : ctx P} {M A σ Δ},
-    {{ Δ ⊢ A }} ->
-    {{ Γ ⊢s σ : Δ }} ->
-    {{ Γ ⊢ M : A[σ] }} ->
-    {{ Γ ⊢s q σ∘(Id,,M) ≈ σ,,M : Δ, A }}.
+Lemma wf_exp_eq_sub_sub_compose_cong_nat {P} : forall {Δ : gctx P} {Γ Γ'1 Γ'2 Γ'' σ τ σ' τ' M s} {r : Ru_nat P s},
+    {{ Δ ; Γ'' ⊢ M : ℕ }} ->
+    {{ Δ ; Γ'1 ⊢s σ : Γ'' }} ->
+    {{ Δ ; Γ'2 ⊢s σ' : Γ'' }} ->
+    {{ Δ ; Γ ⊢s τ : Γ'1 }} ->
+    {{ Δ ; Γ ⊢s τ' : Γ'2 }} ->
+    {{ Δ ; Γ ⊢s σ∘τ ≈ σ'∘τ' : Γ'' }} ->
+    {{ Δ ; Γ ⊢ M[σ][τ] ≈ M[σ'][τ'] : ℕ }}.
 Proof with mautosolve 4.
   intros.
-  assert {{ ⊢ Γ }} by mauto 3.
-  assert {{ Γ ⊢ A[σ] }} by mauto 3.
-  assert {{ Γ ⊢ M : A[σ] }} by mauto.
-  assert {{ Γ ⊢s Id,,M : Γ, A[σ] }} by mauto.
-  assert {{ Γ, A[σ] ⊢s Wk : Γ }} by mauto 3.
-  assert {{ Γ ⊢ A[σ] }} by mauto 2.
-  assert {{ Γ, A[σ] ⊢ #0 : A[σ][Wk] }} by mauto 4.
-  assert {{ Γ, A[σ] ⊢ #0 : A[σ∘Wk] }} by (eapply wf_conv; mauto 3).
-  assert {{ Γ ⊢s q σ∘(Id,,M) ≈ ((σ∘Wk)∘(Id,,M)),,#0[Id,,M] : Δ, A }} by mauto.
-  assert {{ Γ ⊢s (σ∘Wk)∘(Id,,M) ≈ σ : Δ }} by mauto.
-  assert {{ Γ ⊢ M : A[σ][Id] }} by mauto 4.
-  assert {{ Γ ⊢ #0[Id,,M] ≈ M : A[σ][Id] }} by mauto 4.
-  assert {{ Γ ⊢ #0[Id,,M] ≈ M : A[σ] }} by mauto 4.
-  enough {{ Γ ⊢ #0[Id,,M] ≈ M : A[(σ∘Wk)∘(Id,,M)] }} by mauto.
-  assert {{ Γ ⊢s (σ∘Wk)∘(Id,,M) : Δ }} by mauto 3.
-  assert {{ Γ ⊢ A[(σ∘Wk)∘(Id,,M)] }} by mauto 3.
-  eapply wf_exp_eq_conv; mauto.
-Qed.
-
-
-#[export]
-Hint Resolve sub_eq_q_sigma_id_extend : mcpts.
-#[export]
-Hint Rewrite -> @sub_eq_q_sigma_id_extend using mauto 4 : mcpts.
-
-
-Lemma sub_eq_q_sigma_sigma0_extend {P} : forall {Γ1 Γ2 Γ3 : ctx P} {A σ σ0 M},
-    {{ Γ3 ⊢ A }} ->
-    {{ Γ2 ⊢s σ : Γ3 }} ->
-    {{ Γ1 ⊢s σ0 : Γ2 }} ->
-    {{ Γ1 ⊢ M : A[σ][σ0] }} ->
-    {{ Γ1 ⊢s (q σ)∘(σ0,,M) ≈ (σ∘σ0),,M : Γ3, A }}.
-Proof.
-  intros.
-  assert {{ Γ2, A[σ] ⊢s σ ∘ Wk : Γ3 }} by mauto.
-  assert {{ Γ2 ⊢ A[σ] }} by mauto 3.
-  assert {{ Γ2, A[σ] ⊢s Wk : Γ2 }} by mauto 3.
-  assert {{ Γ2, A[σ] ⊢ A[σ][Wk] }} by mauto 3.
-  assert {{ Γ2, A[σ] ⊢ #0 : A[σ][Wk] }} by mauto 4.
-  assert {{ Γ2, A[σ] ⊢ A[σ][Wk] ≈ A[σ∘Wk] }} by mauto.
-  assert {{ Γ2, A[σ] ⊢ #0 : A[σ∘Wk] }} by mauto 3.
-  assert {{ Γ1 ⊢s (q σ) ∘ (σ0,,M) ≈ ((σ∘Wk)∘(σ0,,M)),,#0[σ0,,M] : Γ3, A }} by mauto 3.
-  assert {{ Γ1 ⊢s (σ∘Wk)∘(σ0,,M) ≈ σ∘(Wk∘(σ0,,M)) : Γ3 }} by (econstructor; mauto 3).
-  assert {{ Γ1 ⊢s σ∘(Wk∘(σ0,,M)) ≈ σ∘σ0 : Γ3 }} by mauto 4.
-  assert {{ Γ1 ⊢s (σ ∘ Wk) ∘ (σ0,,M) ≈ σ∘σ0 : Γ3 }} by (etransitivity; mauto).
-  assert {{ Γ1 ⊢ #0[σ0,,M] ≈ M : A[σ][σ0] }} by mauto.
-  assert {{ Γ3 ⊢ A }} by mauto 2.
-  assert {{ Γ1 ⊢ A[σ][σ0] ≈ A[σ∘σ0] }} by mauto 3.
-  assert {{ Γ1 ⊢ A[σ][σ0] ≈ A[(σ∘Wk)∘(σ0,,M)] }} by (etransitivity; mauto 4).
-  assert {{ Γ1 ⊢s (σ∘Wk)∘(σ0,,M) : Γ3 }} by mauto 3.
-  assert {{ Γ1 ⊢ A[(σ∘Wk)∘(σ0,,M)] }} by mauto 2.
-  assert {{ Γ1 ⊢s (σ∘Wk)∘(σ0,,M),,#0[σ0,,M] ≈ σ∘σ0,,M : Γ3, A }} by (econstructor; mauto).
-  do 2 etransitivity; mauto.
+  assert {{ Δ ; Γ ⊢ M[σ][τ] ≈ M[σ∘τ] : ℕ }} by mauto.
+  assert {{ Δ ; Γ ⊢ M[σ∘τ] ≈ M[σ'∘τ'] : ℕ }} by mauto.
+  enough {{ Δ ; Γ ⊢ M[σ'∘τ'] ≈ M[σ'][τ'] : ℕ }}...
 Qed.
 
 #[export]
-Hint Resolve sub_eq_q_sigma_sigma0_extend : mcpts.
-#[export]
-Hint Rewrite -> @sub_eq_q_sigma_sigma0_extend using mauto 4 : mcpts.
+Hint Resolve wf_exp_eq_sub_sub_compose_cong_nat : mcpts.
 
-Lemma sub_eq_p_q_sigma {P : PtsSig} : forall {Γ : ctx P} {A σ Δ},
-    {{ Δ ⊢ A }} ->
-    {{ Γ ⊢s σ : Δ }} ->
-    {{ Γ, A[σ] ⊢s Wk∘q σ ≈ σ∘Wk : Δ }}.
+Lemma wf_typ_eq_sub_compose_cong {P : PtsSig} : forall {Δ : gctx P} {Γ Γ'1 Γ'2 Γ'' σ τ σ' τ' A},
+    {{ Δ ; Γ'' ⊢ A }} ->
+    {{ Δ ; Γ'1 ⊢s σ : Γ'' }} ->
+    {{ Δ ; Γ'2 ⊢s σ' : Γ'' }} ->
+    {{ Δ ; Γ ⊢s τ : Γ'1 }} ->
+    {{ Δ ; Γ ⊢s τ' : Γ'2 }} ->
+    {{ Δ ; Γ ⊢s σ∘τ ≈ σ'∘τ' : Γ'' }} ->
+    {{ Δ ; Γ ⊢ A[σ][τ] ≈ A[σ'][τ'] }}.
 Proof with mautosolve 3.
   intros.
-  assert {{ Γ, A[σ] ⊢s Wk : Γ }} by mauto 4.
-  assert {{ Γ ⊢ A[σ] }} by mauto 3.
-  assert {{ Γ, A[σ] ⊢ #0 : A[σ][Wk] }} by mauto 4.
-  enough {{ Γ, A[σ] ⊢ #0 : A[σ∘Wk] }} by mauto.
-  eapply wf_conv; mauto 3.
+  assert {{ Δ ; Γ ⊢ A[σ][τ] ≈ A[σ∘τ] }} by mauto 3.
+  assert {{ Δ ; Γ ⊢ A[σ∘τ] ≈ A[σ'∘τ'] }} by mauto 3.
+  enough {{ Δ ; Γ ⊢ A[σ'∘τ'] ≈ A[σ'][τ'] }}...
 Qed.
 
 #[export]
-Hint Resolve sub_eq_p_q_sigma : mcpts.
+Hint Resolve wf_typ_eq_sub_compose_cong : mcpts.
 
-Lemma sub_eq_p_q_sigma_nat {P} : forall {Γ : ctx P} {σ Δ s} {r : Ru_nat P s},
-    {{ Γ ⊢s σ : Δ }} ->
-    {{ Γ, ℕ ⊢s Wk∘q σ ≈ σ∘Wk : Δ }}.
-Proof with mautosolve 3.
-  intros.
-  assert {{ ⊢ Γ, ℕ }} by mauto 3.
-  assert {{ Γ, ℕ ⊢s Wk : Γ }} by mauto 2.
-  assert {{ Γ, ℕ ⊢ #0 : ℕ }}...
-Qed.
 
-#[export]
-Hint Resolve sub_eq_p_q_sigma_nat : mcpts.
-
-Lemma sub_eq_p_p_q_q_sigma_nat {P} : forall {Γ : ctx P} {A σ Δ s} {r : Ru_nat P s},
-    {{ Δ, ℕ ⊢ A  }} ->
-    {{ Γ ⊢s σ : Δ }} ->
-    {{ Γ, ℕ, A[q σ] ⊢s Wk∘(Wk∘q (q σ)) ≈ (σ∘Wk)∘Wk : Δ }}.
-Proof with mautosolve 3.
-  intros.
-  assert {{ Γ, ℕ ⊢ A[q σ] }} by mauto 4.
-  assert {{ ⊢ Γ, ℕ, A[q σ] }} by mauto 3.
-  assert {{ ⊢ Δ, ℕ }} by mauto 3.
-  assert {{ Γ, ℕ, A[q σ] ⊢s Wk∘q (q σ) ≈ q σ∘Wk : Δ, ℕ }} by mauto.
-  assert {{ Γ, ℕ, A[q σ] ⊢s Wk∘(Wk∘q (q σ)) ≈ Wk∘(q σ∘Wk) : Δ }} by mauto 3.
-  assert {{ Δ, ℕ ⊢s Wk : Δ }} by mauto.
-  assert {{ Γ, ℕ ⊢s q σ : Δ, ℕ }} by mauto.
-  assert {{ Γ, ℕ, A[q σ] ⊢s Wk∘(q σ∘Wk) ≈ (Wk∘q σ)∘Wk : Δ }} by mauto 4.
-  assert {{ Γ, ℕ ⊢s Wk∘q σ ≈ σ∘Wk : Δ }} by mauto.
-  enough {{ Γ, ℕ, A[q σ] ⊢s (Wk∘q σ)∘Wk ≈ (σ∘Wk)∘Wk : Δ }}...
-Qed.
-
-#[export]
-Hint Resolve sub_eq_p_p_q_q_sigma_nat : mcpts.
-
-Lemma sub_eq_q_sigma_compose_weak_weak_extend_succ_var_1 {P} : forall {Γ : ctx P} {A σ Δ s} {r : Ru_nat P s},
-    {{ Δ, ℕ ⊢ A }} ->
-    {{ Γ ⊢s σ : Δ }} ->
-    {{ Γ, ℕ, A[q σ] ⊢s q σ∘(Wk∘Wk,,succ #1) ≈ (Wk∘Wk,,succ #1)∘q (q σ) : Δ, ℕ }}.
-Proof with mautosolve 3.
-  intros.
-  assert {{ ⊢ Δ, ℕ, A }} by mauto 3.
-  assert {{ ⊢ Γ, ℕ }} by mauto 3.
-  assert {{ Γ, ℕ ⊢s Wk : Γ }} by mauto 3.
-  assert {{ Γ, ℕ ⊢s σ∘Wk : Δ }} by mauto 3.
-  assert {{ Γ, ℕ ⊢ A[q σ] }} by mauto 4.
-  set (Γ' := {{{ Γ, ℕ, A[q σ] }}}).
-  set (WkWksucc := {{{ (Wk∘Wk),,succ #1 }}}).
-  assert {{ ⊢ Γ' }} by mauto 2.
-  assert {{ Γ' ⊢s Wk∘Wk : Γ }} by mauto 3.
-  assert {{ Γ' ⊢s WkWksucc : Γ, ℕ }} by mauto 4.
-  assert {{ Γ, ℕ ⊢ #0 : ℕ}} by mauto 3.
-  assert {{ Γ' ⊢s q σ∘WkWksucc ≈ ((σ∘Wk)∘WkWksucc),,#0[WkWksucc] : Δ, ℕ }} by mautosolve 3.
-  assert {{ Γ' ⊢ #1 : ℕ[Wk][Wk] }} by mauto.
-  assert {{ Γ' ⊢ ℕ[Wk][Wk] ≈ ℕ : Sort@s }} by mauto 3.
-  assert {{ Γ' ⊢ #1 : ℕ }} by mauto 2.
-  assert {{ Γ' ⊢ succ #1 : ℕ }} by mauto.
-  assert {{ Γ' ⊢s Wk∘WkWksucc : Γ }} by mauto 4.
-  assert {{ Γ' ⊢s Wk∘WkWksucc ≈ Wk∘Wk : Γ }} by mauto 4.
-  assert {{ Γ ⊢s σ ≈ σ : Δ }} by mauto.
-  assert {{ Γ' ⊢s σ∘(Wk∘WkWksucc) ≈ σ∘(Wk∘Wk) : Δ }} by mauto 3.
-  assert {{ Γ' ⊢s (σ∘Wk)∘WkWksucc ≈ σ∘(Wk∘Wk) : Δ }} by mauto 3.
-  assert {{ Γ' ⊢s σ∘(Wk∘Wk) ≈ (σ∘Wk)∘Wk : Δ }} by mauto 4.
-  assert {{ Γ' ⊢s (σ∘Wk)∘Wk ≈ Wk∘(Wk∘q (q σ)) : Δ }} by mauto.
-  assert {{ Δ, ℕ ⊢s Wk : Δ }} by mauto 4.
-  assert {{ Δ, ℕ, A ⊢s Wk : Δ, ℕ }} by mauto 4.
-  assert {{ Δ, ℕ, A ⊢s Wk∘Wk : Δ }} by mauto 4.
-  assert {{ Γ' ⊢s q (q σ) : Δ, ℕ, A }} by mauto.
-  assert {{ Γ' ⊢s Wk∘(Wk∘q (q σ)) ≈ (Wk∘Wk)∘q (q σ) : Δ }} by mauto 3.
-  assert {{ Γ' ⊢s σ∘(Wk∘Wk) ≈ (Wk∘Wk)∘q (q σ) : Δ }} by mauto 3.
-  assert {{ Γ' ⊢ #0[WkWksucc] ≈ succ #1 : ℕ }} by mauto.
-  assert {{ Γ' ⊢ succ #1[q (q σ)] ≈ succ #1 : ℕ }} by mauto 3.
-  assert {{ Δ, ℕ, A ⊢ #1 : ℕ }} by mauto 2.
-  assert {{ Γ' ⊢ succ #1 ≈ (succ #1)[q (q σ)] : ℕ }} by mauto 4.
-  assert {{ Γ' ⊢ #0[WkWksucc] ≈ (succ #1)[q (q σ)] : ℕ }} by mauto 2.
-  assert {{ Γ' ⊢s (σ∘Wk)∘WkWksucc : Δ }} by mauto 3.
-  assert {{ Γ' ⊢s ((σ∘Wk)∘WkWksucc),,#0[WkWksucc] ≈ ((Wk∘Wk)∘q (q σ)),,(succ #1)[q (q σ)] : Δ, ℕ }} by mauto 3.
-  assert {{ Δ, ℕ, A ⊢ #1 : ℕ[Wk][Wk] }} by mauto 4.
-  assert {{ Δ, ℕ, A ⊢ ℕ[Wk][Wk] ≈ ℕ : Sort@s }} by mauto 3.
-  assert {{ Δ, ℕ, A ⊢ succ #1 : ℕ }} by mauto 4.
-  enough {{ Γ' ⊢s ((Wk∘Wk)∘q (q σ)),,(succ #1)[q (q σ)] ≈ WkWksucc∘q (q σ) : Δ, ℕ }}...
-Qed.
-
-#[export]
-Hint Resolve sub_eq_q_sigma_compose_weak_weak_extend_succ_var_1 : mcpts.
-
-(** *** Lemmas for [wf_subtyp] *)
-
-Fact wf_subtyp_refl_sorted {P} : forall {Γ : ctx P} {A s},
-    {{ Γ ⊢ A : Sort@s }} ->
-    {{ Γ ⊢ A ⊆ A }}.
+(** ** Lemmas for [typ] *)
+Lemma wf_typ_eq_refl_sort {P : PtsSig} : forall {Δ : gctx P} {Γ s},
+    {{ Δ ⊢ Γ }} ->
+    {{ Δ ; Γ ⊢ Sort@s ≈ Sort@s }}.
 Proof. mauto. Qed.
 
 #[export]
-Hint Resolve wf_subtyp_refl_sorted : mcpts.
+Hint Resolve wf_typ_eq_refl_sort : mcpts.
 
-Lemma wf_subtyp_sub {P} : forall {Δ : ctx P} {A A'},
-    {{ Δ ⊢ A ⊆ A' }} ->
-    forall Γ σ,
-      {{ Γ ⊢s σ : Δ }} ->
-      {{ Γ ⊢ A[σ] ⊆ A'[σ] }}.
-Proof.
-  induction 1; intros; mauto 4.
-  - assert {{ Γ0 ⊢ A[σ] ≈ B[σ] }} by mauto 3.
-    assert {{ Γ0 ⊢ B[σ] }} by mauto 3.
-    mauto 3.
-  - assert {{ ⊢ Γ0 }} by mauto 2.
-    assert {{ Γ ⊢ Sort@s1 ⊆ Sort@s2 }} by mauto.
-    assert {{ Γ ⊢ Sort@s1 }} by mauto.
-    assert {{ Γ0 ⊢ Sort@s1[σ] ≈ Sort@s1 }} by mauto.
-    assert {{ Γ0 ⊢ Sort@s2 ≈ Sort@s2[σ] }} by (symmetry; mauto).
-    transitivity {{{ Sort@s1 }}}; mauto 3.
-    transitivity {{{ Sort@s2 }}}; mauto 3.
-    mauto 4.
-  - assert {{ Γ0 ⊢ A[σ] : Sort@s1 }} by mauto 3.
-    assert {{ Γ0, A[σ] ⊢ B[q σ] : Sort@s2 }} by mauto 4.
-    assert {{ Γ0 ⊢ Π r A[σ] B[q σ] }} by mauto.
-    transitivity {{{ Π r (A[σ]) (B[q σ]) }}}; [econstructor; mauto 3|].
-    transitivity {{{ Π r (A'[σ]) (B'[q σ]) }}}; [ | econstructor; mauto 4].
-    eapply wf_subtyp_pi; mauto 4.
-Qed.
+Lemma wf_typ_eq_sub_cong1 {P : PtsSig} : forall {Δ : gctx P} {Γ Γ' A A' σ},
+    {{ Δ ; Γ' ⊢ A ≈ A' }} ->
+    {{ Δ ; Γ ⊢s σ : Γ' }} ->
+    {{ Δ ; Γ ⊢ A[σ] ≈ A'[σ] }}.
+Proof. mauto. Qed.
 
-
-#[export]
-Hint Resolve wf_subtyp_sub : mcpts.
-
-
-Lemma wf_subtyp_sort_weaken {P} : forall {Γ : ctx P} {s1 s2 A},
-    {{ Γ ⊢ Sort@s1 ⊆ Sort@s2 }} ->
-    {{ ⊢ Γ, A }} ->
-    {{ Γ, A ⊢ Sort@s1 ⊆ Sort@s2 }}.
-Proof.    
-  intros.
-  assert {{ Γ ⊢ Sort@s2  }} by mauto 2.
-  assert {{ Γ, A ⊢s Wk : Γ }} by mauto 2.
-  dependent induction H; mauto 2.
-  - assert {{ Γ, A ⊢ Sort@s1[Wk] ≈ Sort@s2[Wk] }} by mauto.
-    assert {{ Γ, A ⊢ Sort@s1[Wk] ≈ Sort@s1  }} by mauto.
-    assert {{ Γ, A ⊢ Sort@s2[Wk] ≈ Sort@s2  }} by mauto.
-    assert {{ Γ, A ⊢ Sort@s1 ≈ Sort@s2  }} by mauto.
-    mauto 3.
-  - assert {{ Γ ⊢ Sort@s1 ⊆ Sort@s2 }} by mauto 3.
-    assert {{ Γ, A ⊢ Sort@s1[Wk] ⊆ Sort@s2[Wk] }} by mauto 2.
-    assert {{ Γ, A ⊢ Sort@s1[Wk] }} by mauto 4.
-    assert {{ Γ, A ⊢ Sort@s1 ⊆ Sort@s1[Wk] }} by mauto 4.
-    transitivity {{{ Sort@s1[Wk] }}}; mauto.
-Qed.
-
-Lemma ctx_sub_ctx_lookup {P} : forall {Γ Δ : ctx P},
-    {{ ⊢ Δ ⊆ Γ }} ->
-    forall {A x},
-      {{ #x : A ∈ Γ }} ->
-      exists B,
-        {{ #x : B ∈ Δ }} /\
-          {{ Δ ⊢ B ⊆ A }}.
-Proof with (do 2 eexists; repeat split; mautosolve).
-  induction 1; intros * Hx; progressive_inversion.
-  dependent destruction Hx.
-  - eexists; split; mauto 3.
-    eapply wf_subtyp_sub; mauto 4.
-  - edestruct IHwf_ctx_sub as [? []]; try eassumption...
-Qed.
-
-#[export]
-Hint Resolve ctx_sub_ctx_lookup : mcpts.
-
-(** *** Lemmas for [wf_typ_eq] *)
-
-Fact wf_typ_eq_refl {P : PtsSig} : forall {Γ : ctx P} {A},
-    {{ Γ ⊢ A }} ->
-    {{ Γ ⊢ A ≈ A }}.
+Lemma wf_typ_eq_sub_cong2  {P} : forall {Δ : gctx P} {Γ Γ' A σ τ},
+    {{ Δ ; Γ' ⊢ A }} ->
+    {{ Δ ; Γ ⊢s σ : Γ' }} ->
+    {{ Δ ; Γ ⊢s σ ≈ τ : Γ' }} ->
+    {{ Δ ; Γ ⊢ A[σ] ≈ A[τ] }}.
 Proof. mauto. Qed.
 
 #[export]
-Hint Resolve wf_typ_eq_refl : mcpts.
-
-Lemma wf_typ_eq_sub_sorted {P : PtsSig} : forall {Δ : ctx P} {s A A'},
-    {{ Δ ⊢ A ≈ A' : Sort@s }} ->
-    forall Γ σ,
-    {{ Γ ⊢s σ : Δ }} ->
-    {{ Γ ⊢ A[σ] ≈ A'[σ] : Sort@s }}.
+Hint Resolve wf_typ_eq_sub_cong1 wf_typ_eq_sub_cong2 : mcpts.
+  
+Lemma wf_typ_eq_sub_compose_typ  {P : PtsSig} : forall {Δ : gctx P} {Γ Γ' Γ'' A σ τ},
+    {{ Δ ; Γ'' ⊢ A }} ->
+    {{ Δ ; Γ' ⊢s σ : Γ'' }} ->
+    {{ Δ ; Γ ⊢s τ : Γ' }} ->
+    {{ Δ ; Γ ⊢ A[σ][τ] ≈ A[σ∘τ] }}.
 Proof. mauto. Qed.
 
 #[export]
-Hint Resolve wf_typ_eq_sub_sorted : mcpts.
+Hint Resolve wf_typ_eq_sub_compose_typ : mcpts.
 
-Lemma wf_typ_sort_weaken {P : PtsSig} : forall {Γ : ctx P} {s A},
-    {{ Γ ⊢ Sort@s ≈ Sort@s }} ->
-    {{ ⊢ Γ, A }} ->
-    {{ Γ, A ⊢ Sort@s ≈ Sort@s }}.
-Proof. mauto. Qed.
-
-Lemma wf_typ_sort_sub {P} : forall {Γ Γ' : ctx P} {A σ},
-    {{ Γ ⊢s σ : Γ' }} ->
-    {{ Γ' ⊢ A }} ->
-    {{ Γ ⊢ A[σ] }}.
-Proof. mauto. Qed.
-
-#[export]
-Hint Resolve wf_typ_sort_sub : mcpts.
-
-Lemma wf_typ_eq_sub_unsorted {P : PtsSig} : forall {Δ : ctx P} {A A'},
-    {{ Δ ⊢ A ≈ A' }} ->
-    forall Γ σ,
-    {{ Γ ⊢s σ : Δ }} ->
-    {{ Γ ⊢ A[σ] ≈ A'[σ] }}.
-Proof. mauto. Qed.
-
-#[export]
-Hint Resolve wf_typ_eq_sub_unsorted : mcpts.
-
-Lemma typ_eq_sub_cong_typ1 {P : PtsSig} : forall {Δ : ctx P} {Γ A A' σ},
-    {{ Δ ⊢ A ≈ A' }} ->
-    {{ Γ ⊢s σ : Δ }} ->
-    {{ Γ ⊢ A[σ] ≈ A'[σ] }}.
-Proof. mauto. Qed.
-
-Lemma typ_eq_sub_cong_typ2  {P} : forall {Δ : ctx P} {Γ A σ τ},
-    {{ Δ ⊢ A }} ->
-    {{ Γ ⊢s σ : Δ }} ->
-    {{ Γ ⊢s σ ≈ τ : Δ }} ->
-    {{ Γ ⊢ A[σ] ≈ A[τ] }}.
-Proof. mauto. Qed.
-
-Lemma typ_eq_sub_compose_typ  {P : PtsSig} : forall {Ψ : ctx P} {Δ Γ A σ τ},
-    {{ Ψ ⊢ A  }} ->
-    {{ Δ ⊢s σ : Ψ }} ->
-    {{ Γ ⊢s τ : Δ }} ->
-    {{ Γ ⊢ A[σ][τ] ≈ A[σ∘τ] }}.
-Proof. mauto. Qed.
-
-#[export]
-Hint Resolve typ_eq_sub_cong_typ1 typ_eq_sub_cong_typ2 typ_eq_sub_compose_typ : mcpts.
-
-Lemma typ_eq_sub_compose_weaken_extend_typ {P : PtsSig} : forall {Γ : ctx P} {σ Δ A B M},
-    {{ Γ ⊢s σ : Δ }} ->
-    {{ Δ ⊢ A }} ->
-    {{ Δ ⊢ B }} ->
-    {{ Γ ⊢ M : B[σ] }} ->
-    {{ Γ ⊢ A[Wk][σ,,M] ≈ A[σ] }}.
+Lemma wf_typ_eq_sub_compose_weaken_extend {P : PtsSig} : forall {Δ : gctx P} {Γ Γ' σ A B M},
+    {{ Δ ; Γ ⊢s σ : Γ' }} ->
+    {{ Δ ; Γ' ⊢ A }} ->
+    {{ Δ ; Γ' ⊢ B }} ->
+    {{ Δ ; Γ ⊢ M : B[σ] }} ->
+    {{ Δ ; Γ ⊢ A[Wk][σ,,M] ≈ A[σ] }}.
 Proof with mautosolve 3.
   intros.  
-  assert {{ Δ, B ⊢s Wk : Δ }} by mauto 4.
+  assert {{ Δ ; Γ', B ⊢s Wk : Γ' }} by mauto 4.
   transitivity {{{ A[Wk∘(σ,,M)] }}}; [mautosolve 4 |].
-  eapply typ_eq_sub_cong_typ2...
+  eapply wf_typ_eq_sub_cong2...
 Qed.
 
 #[export]
-Hint Resolve typ_eq_sub_compose_weaken_extend_typ : mcpts.
+Hint Resolve wf_typ_eq_sub_compose_weaken_extend : mcpts.
 
-Lemma typ_eq_sub_compose_weaken_id_extend_typ {P : PtsSig} : forall {Γ : ctx P} {A B M},
-    {{ Γ ⊢ A }} ->
-    {{ Γ ⊢ B }} ->
-    {{ Γ ⊢ M : B }} ->
-    {{ Γ ⊢ A[Wk][Id,,M] ≈ A }}.
+Lemma wf_typ_eq_sub_compose_weaken_id_extend {P : PtsSig} : forall {Δ : gctx P} {Γ A B M},
+    {{ Δ ; Γ ⊢ A }} ->
+    {{ Δ ; Γ ⊢ B }} ->
+    {{ Δ ; Γ ⊢ M : B }} ->
+    {{ Δ ; Γ ⊢ A[Wk][Id,,M] ≈ A }}.
 Proof with mautosolve 3.
   intros.
-  assert {{ ⊢ Γ }} by mauto 2.
-  assert {{ Γ ⊢ B[Id] }} by mauto 3.
-  assert {{ Γ ⊢ B ≈ B[Id] }} by mauto 3.
-  assert {{ Γ ⊢ M : B[Id] }} by mauto 2.
+  assert {{ Δ ⊢ Γ }} by mauto 2.
+  assert {{ Δ ; Γ ⊢ B[Id] }} by mauto 3.
+  assert {{ Δ ; Γ ⊢ B ≈ B[Id] }} by mauto 3.
+  assert {{ Δ ; Γ ⊢ M : B[Id] }} by mauto 2.
   transitivity {{{ A[Id] }}}...
 Qed.
 
 #[export]
-Hint Resolve typ_eq_sub_compose_weaken_id_extend_typ : mcpts.
+Hint Resolve wf_typ_eq_sub_compose_weaken_id_extend : mcpts.
 
-Lemma typ_eq_sub_compose_double_weaken_double_extend_typ {P : PtsSig} : forall {Γ : ctx P} {σ Δ A B M C N},
-    {{ Γ ⊢s σ : Δ }} ->
-    {{ Δ ⊢ A }} ->
-    {{ Δ ⊢ B }} ->
-    {{ Γ ⊢ M : B[σ] }} ->
-    {{ Δ, B ⊢ C }} ->
-    {{ Γ ⊢ N : C[σ,,M] }} ->
-    {{ Γ ⊢ A[Wk∘Wk][σ,,M,,N] ≈ A[σ] }}.
+Lemma wf_typ_eq_sub_compose_double_weaken_double_extend {P : PtsSig} : forall {Δ : gctx P} {Γ Γ' σ A B M C N},
+    {{ Δ ; Γ ⊢s σ : Γ' }} ->
+    {{ Δ ; Γ' ⊢ A }} ->
+    {{ Δ ; Γ' ⊢ B }} ->
+    {{ Δ ; Γ ⊢ M : B[σ] }} ->
+    {{ Δ ; Γ', B ⊢ C }} ->
+    {{ Δ ; Γ ⊢ N : C[σ,,M] }} ->
+    {{ Δ ; Γ ⊢ A[Wk∘Wk][σ,,M,,N] ≈ A[σ] }}.
 Proof with mautosolve 3.
   intros.
-  assert {{ ⊢ Γ }} by mauto 2.
-  assert {{ ⊢ Δ }} by mauto 2.
-  assert {{ Δ, B ⊢s Wk : Δ }} by mauto 3.
-  assert {{ Δ, B, C ⊢s Wk : Δ, B }} by mauto 4.
-  assert {{ Δ, B ⊢ A[Wk] }} by mauto 3.
-  transitivity {{{ A[Wk][Wk][σ,,M,,N] }}}; [eapply typ_eq_sub_cong_typ1; mautosolve 3 |].
+  assert {{ Δ ⊢ Γ }} by mauto 2.
+  assert {{ Δ ⊢ Γ' }} by mauto 2.
+  assert {{ Δ ; Γ', B ⊢s Wk : Γ' }} by mauto 3.
+  assert {{ Δ ; Γ', B, C ⊢s Wk : Γ', B }} by mauto 4.
+  assert {{ Δ ; Γ', B ⊢ A[Wk] }} by mauto 3.
+  transitivity {{{ A[Wk][Wk][σ,,M,,N] }}}; [eapply wf_typ_eq_sub_cong1; mautosolve 3 |].
   transitivity {{{ A[Wk][σ,,M] }}}...
 Qed.
 
 #[export]
-Hint Resolve typ_eq_sub_compose_double_weaken_double_extend_typ : mcpts.
+Hint Resolve wf_typ_eq_sub_compose_double_weaken_double_extend : mcpts.
 
-Lemma typ_eq_sub_compose_double_weaken_id_double_extend_typ {P : PtsSig} : forall {Γ : ctx P} {A B M C N},
-    {{ Γ ⊢ A }} ->
-    {{ Γ ⊢ B }} ->
-    {{ Γ ⊢ M : B }} ->
-    {{ Γ, B ⊢ C }} ->
-    {{ Γ ⊢ N : C[Id,,M] }} ->
-    {{ Γ ⊢ A[Wk∘Wk][Id,,M,,N] ≈ A }}.
+Lemma wf_typ_eq_sub_compose_double_weaken_id_double_extend {P : PtsSig} : forall {Δ : gctx P} {Γ A B M C N},
+    {{ Δ ; Γ ⊢ A }} ->
+    {{ Δ ; Γ ⊢ B }} ->
+    {{ Δ ; Γ ⊢ M : B }} ->
+    {{ Δ ; Γ, B ⊢ C }} ->
+    {{ Δ ; Γ ⊢ N : C[Id,,M] }} ->
+    {{ Δ ; Γ ⊢ A[Wk∘Wk][Id,,M,,N] ≈ A }}.
 Proof with mautosolve 3.
   intros.
-  assert {{ ⊢ Γ }} by mauto 2.
-  assert {{ Γ ⊢ B[Id] }} by mauto 3.
-  assert {{ Γ ⊢ B ≈ B[Id] }} by mauto 3.
-  assert {{ Γ ⊢ M : B[Id] }} by mauto 3.
+  assert {{ Δ ⊢ Γ }} by mauto 2.
+  assert {{ Δ ; Γ ⊢ B[Id] }} by mauto 3.
+  assert {{ Δ ; Γ ⊢ B ≈ B[Id] }} by mauto 3.
+  assert {{ Δ ; Γ ⊢ M : B[Id] }} by mauto 3.
   transitivity {{{ A[Id] }}}...
 Qed.
 
 #[export]
-Hint Resolve typ_eq_sub_compose_double_weaken_id_double_extend_typ : mcpts.
+Hint Resolve wf_typ_eq_sub_compose_double_weaken_id_double_extend : mcpts.
 
-Lemma typ_eq_typ_sub_sub {P : PtsSig} : forall {Γ : ctx P} {Δ Ψ σ τ s1},
-    {{ Δ ⊢s σ : Ψ }} ->
-    {{ Γ ⊢s τ : Δ }} ->
-    {{ Γ ⊢ Sort@s1[σ][τ] ≈ Sort@s1 }}.
+Lemma wf_typ_eq_sort_sub_sub {P : PtsSig} : forall {Δ : gctx P} {Γ Γ' Γ'' σ τ s1},
+    {{ Δ ; Γ' ⊢s σ : Γ'' }} ->
+    {{ Δ ; Γ ⊢s τ : Γ' }} ->
+    {{ Δ ; Γ ⊢ Sort@s1[σ][τ] ≈ Sort@s1 }}.
 Proof.
   intros.
   transitivity {{{ Sort@s1[σ∘τ] }}}; mauto.
 Qed.
 
 #[export]
-Hint Resolve typ_eq_typ_sub_sub : mcpts.
+Hint Resolve wf_typ_eq_sort_sub_sub : mcpts.
 #[export]
-Hint Rewrite -> @typ_eq_typ_sub_sub using mauto 4 : mcpts.
+Hint Rewrite -> @wf_typ_eq_sort_sub_sub using mauto 4 : mcpts.
 
-Lemma var_compose_subs {P : PtsSig} : forall {Γ : ctx P} {τ Δ σ Ψ A x},
-    {{ Ψ ⊢ A }} ->
-    {{ Δ ⊢s σ : Ψ }} ->
-    {{ Γ ⊢s τ : Δ }} ->
-    {{ #x : A[σ][τ] ∈ Γ }} ->
-    {{ Γ ⊢ #x : A[σ∘τ] }}.
+(** *** Lemmas for [wf_subtyp] *)
+
+(* Fact wf_typ_subtyp_refl_sorted {P} : forall {Δ : gctx P} {Γ A s}, *)
+(*     {{ Δ ; Γ ⊢ A : Sort@s }} -> *)
+(*     {{ Δ ; Γ ⊢ A ⊆ A }}. *)
+(* Proof. mauto. Qed. *)
+
+(* #[export] *)
+(* Hint Resolve wf_typ_subtyp_refl_sorted : mcpts. *)
+
+(* Lemma wf_typ_subtyp_sub {P} : forall {Δ : gctx P} {Γ' A A'}, *)
+(*     {{ Δ ; Γ' ⊢ A ⊆ A' }} -> *)
+(*     forall Γ σ, *)
+(*       {{ Δ ; Γ ⊢s σ : Γ' }} -> *)
+(*       {{ Δ ; Γ ⊢ A[σ] ⊆ A'[σ] }}. *)
+(* Proof. *)
+(*   induction 1; intros; mauto 4. *)
+(*   (* - assert {{ Δ ; Γ0 ⊢ A[σ] ≈ B[σ] }} by mauto 3. *) *)
+(*   (*   assert {{ Γ0 ⊢ B[σ] }} by mauto 3. *) *)
+(*   (*   mauto 3. *) *)
+(*   - assert {{ Δ ⊢ Γ0 }} by mauto 2. *)
+(*     assert {{ Δ ; Γ ⊢ Sort@s1 ⊆ Sort@s2 }} by mauto. *)
+(*     assert {{ Δ ; Γ ⊢ Sort@s1 }} by mauto. *)
+(*     assert {{ Δ ; Γ0 ⊢ Sort@s1[σ] ≈ Sort@s1 }} by mauto. *)
+(*     assert {{ Δ ; Γ0 ⊢ Sort@s2 ≈ Sort@s2[σ] }} by (symmetry; mauto). *)
+(*     transitivity {{{ Sort@s1 }}}; mauto 3. *)
+(*     transitivity {{{ Sort@s2 }}}; mauto 3. *)
+(*     mauto 4. *)
+(*   - assert {{ Δ ; Γ0 ⊢ A[σ] : Sort@s1 }} by mauto 3. *)
+(*     assert {{ Δ ; Γ0, A[σ] ⊢ B[q σ] : Sort@s2 }} by mauto 4. *)
+(*     assert {{ Δ ; Γ0 ⊢ Π r A[σ] B[q σ] }} by mauto. *)
+(*     transitivity {{{ Π r (A[σ]) (B[q σ]) }}}; [econstructor; mauto 3|]. *)
+(*     transitivity {{{ Π r (A'[σ]) (B'[q σ]) }}}; [ | econstructor; mauto 4]. *)
+(*     eapply wf_subtyp_pi; mauto 4. *)
+(* Qed. *)
+
+
+(* #[export] *)
+(* Hint Resolve wf_subtyp_sub : mcpts. *)
+
+
+(* Lemma wf_subtyp_sort_weaken {P} : forall {Γ : ctx P} {s1 s2 A}, *)
+(*     {{ Γ ⊢ Sort@s1 ⊆ Sort@s2 }} -> *)
+(*     {{ ⊢ Γ, A }} -> *)
+(*     {{ Γ, A ⊢ Sort@s1 ⊆ Sort@s2 }}. *)
+(* Proof.     *)
+(*   intros. *)
+(*   assert {{ Γ ⊢ Sort@s2  }} by mauto 2. *)
+(*   assert {{ Γ, A ⊢s Wk : Γ }} by mauto 2. *)
+(*   dependent induction H; mauto 2. *)
+(*   - assert {{ Γ, A ⊢ Sort@s1[Wk] ≈ Sort@s2[Wk] }} by mauto. *)
+(*     assert {{ Γ, A ⊢ Sort@s1[Wk] ≈ Sort@s1  }} by mauto. *)
+(*     assert {{ Γ, A ⊢ Sort@s2[Wk] ≈ Sort@s2  }} by mauto. *)
+(*     assert {{ Γ, A ⊢ Sort@s1 ≈ Sort@s2  }} by mauto. *)
+(*     mauto 3. *)
+(*   - assert {{ Γ ⊢ Sort@s1 ⊆ Sort@s2 }} by mauto 3. *)
+(*     assert {{ Γ, A ⊢ Sort@s1[Wk] ⊆ Sort@s2[Wk] }} by mauto 2. *)
+(*     assert {{ Γ, A ⊢ Sort@s1[Wk] }} by mauto 4. *)
+(*     assert {{ Γ, A ⊢ Sort@s1 ⊆ Sort@s1[Wk] }} by mauto 4. *)
+(*     transitivity {{{ Sort@s1[Wk] }}}; mauto. *)
+(* Qed. *)
+
+(* Lemma ctx_sub_ctx_lookup {P} : forall {Γ Δ : ctx P}, *)
+(*     {{ ⊢ Δ ⊆ Γ }} -> *)
+(*     forall {A x}, *)
+(*       {{ #x : A ∈ Γ }} -> *)
+(*       exists B, *)
+(*         {{ #x : B ∈ Δ }} /\ *)
+(*           {{ Δ ⊢ B ⊆ A }}. *)
+(* Proof with (do 2 eexists; repeat split; mautosolve). *)
+(*   induction 1; intros * Hx; progressive_inversion. *)
+(*   dependent destruction Hx. *)
+(*   - eexists; split; mauto 3. *)
+(*     eapply wf_subtyp_sub; mauto 4. *)
+(*   - edestruct IHwf_ctx_sub as [? []]; try eassumption... *)
+(* Qed. *)
+
+(* #[export] *)
+(* Hint Resolve ctx_sub_ctx_lookup : mcpts. *)
+
+
+(** ** Lemmas about context lookups *)
+Lemma wf_gctx_eq_gctx_lookup {P : PtsSig} : forall {Δ : gctx P} {Δ' A x},
+    {{ ⊢ Δ ≈ Δ' }} ->
+    {{ `#x : A ∈ Δ }} ->
+    exists B,
+      {{ `#x : B ∈ Δ' }} /\
+        {{ Δ ; ⋅ ⊢ A ≈ B }} /\
+        {{ Δ' ; ⋅ ⊢ A ≈ B }} /\
+        {{ Δ' ; ⋅ ⊢ A }}.
+Proof.
+  intros * HΔΔ' Hx.
+  assert {{ ⊢ Δ }} by mauto 2.
+  assert {{ Δ ; ⋅ ⊢ A }} by mauto 2.
+  gen Δ' Hx.
+  induction 1 as [|* ? IHHx]; inversion_clear 1 as [| ? ? ? ? ? HΔΔ'0];
+    assert {{ ⊢ Δ'0 }} by mauto 2.
+  - eexists; repeat split; mauto 3.
+  - specialize (IHHx ltac:(mauto 2) ltac:(mauto 3) _ HΔΔ'0).
+    destruct_conjs.
+    eexists; repeat split; mauto 3.
+Qed.    
+
+#[export]
+Hint Resolve wf_gctx_eq_gctx_lookup : mcpts.
+ 
+Lemma wf_ctx_eq_ctx_lookup {P : PtsSig} : forall {Δ : gctx P} {Γ Γ' A x},
+    {{ Δ ⊢ Γ ≈ Γ' }} ->
+    {{ #x : A ∈ Γ }} ->
+    exists B,
+      {{ #x : B ∈ Γ' }} /\
+        {{ Δ ; Γ ⊢ A ≈ B }} /\
+        {{ Δ ; Γ' ⊢ A ≈ B }} /\
+        {{ Δ ; Γ' ⊢ A }}.
+Proof with (repeat eexists; mautosolve 3).
+  intros * HΓΓ' Hx.
+  assert {{ Δ ⊢ Γ }} by mauto 2.
+  assert {{ Δ ; Γ ⊢ A }} by mauto 3.
+  gen Γ' Hx.
+  induction 1 as [|* ? IHHx]; inversion_clear 1 as [|? ? ? ? ? HΓΓ'0];
+    assert {{ Δ ⊢ Γ'0 }} by mauto 2.
+  - assert {{ Δ ⊢ Γ, A }} by mauto 3.
+    assert {{ Δ ; Γ, A ⊢s Wk : Γ }} by mauto 2.
+    assert {{ Δ ; Γ'0, A' ⊢s Wk : Γ'0 }} by mauto 3.
+    eexists.
+    do 3 (split; mauto 3).
+  - specialize (IHHx ltac:(mauto 2) ltac:(mauto 3) _ HΓΓ'0).
+    destruct_conjs.
+    assert {{ Δ ; Γ, B ⊢s Wk : Γ }} by mauto 2.
+    assert {{ Δ ; Γ'0, A' ⊢s Wk : Γ'0 }} by mauto 3.
+    eexists.
+    do 3 (split; mauto 3).
+Qed.
+
+#[export]
+Hint Resolve wf_ctx_eq_ctx_lookup : mcpts.
+
+
+(** ** Other Tedious Lemmas *)
+Lemma wf_sub_eq_weaken_var0_id {P : PtsSig} : forall {Δ : gctx P} {Γ A},
+    {{ Δ ; Γ ⊢ A }} ->
+    {{ Δ ; Γ, A ⊢s Wk,,#0 ≈ Id : Γ, A }}.
+Proof with mautosolve 4.
+  intros * ?.
+  assert {{ Δ ⊢ Γ }} by mauto 2.
+  assert {{ Δ ; Γ ⊢ A }} by mauto 2.
+  assert {{ Δ ⊢ Γ, A }} by mauto 3.
+  assert {{ Δ ; Γ, A ⊢s Wk : Γ }} by mauto 2.
+  assert {{ Δ ; Γ, A ⊢s (Wk∘Id),,#0[Id] ≈ Id : Γ, A }} by mauto.
+  assert {{ Δ ; Γ, A ⊢s Wk ≈ Wk∘Id : Γ }} by mauto.
+  assert {{ Δ ; Γ, A ⊢s Wk,,#0 ≈ Wk∘Id,,#0[Id] : Γ, A }} by (eapply wf_sub_eq_extend_cong; mauto 4).
+  enough {{ Δ ; Γ, A ⊢ #0 ≈ #0[Id] : A[Wk] }} by (etransitivity; mauto 3).
+  symmetry; econstructor; econstructor; mauto 2.
+Qed.
+
+#[export]
+Hint Resolve wf_sub_eq_weaken_var0_id : mcpts.
+#[export]
+Hint Rewrite -> @wf_sub_eq_weaken_var0_id using mauto 4 : mcpts.
+
+Lemma wf_exp_eq_sub_sub_compose_cong {P : PtsSig} : forall {Δ : gctx P} {Γ Γ'1 Γ'2 Γ'' σ τ σ' τ' M A},
+    {{ Δ ; Γ'' ⊢ A }} ->
+    {{ Δ ; Γ'' ⊢ M : A }} ->
+    {{ Δ ; Γ'1 ⊢s σ : Γ'' }} ->
+    {{ Δ ; Γ'2 ⊢s σ' : Γ'' }} ->
+    {{ Δ ; Γ ⊢s τ : Γ'1 }} ->
+    {{ Δ ; Γ ⊢s τ' : Γ'2 }} ->
+    {{ Δ ; Γ ⊢s σ∘τ ≈ σ'∘τ' : Γ'' }} ->
+    {{ Δ ; Γ ⊢ M[σ][τ] ≈ M[σ'][τ'] : A[σ∘τ] }}.
+Proof with mautosolve 3.
+  intros.
+  assert {{ Δ ; Γ ⊢ A[σ∘τ] ≈ A[σ'∘τ'] }} by mauto.
+  assert {{ Δ ; Γ ⊢ M[σ][τ] ≈ M[σ∘τ] : A[σ∘τ] }} by mauto 4.
+  assert {{ Δ ; Γ ⊢ M[σ∘τ] ≈ M[σ'∘τ'] : A[σ∘τ] }} by mauto 4.
+  assert {{ Δ ; Γ ⊢ M[σ'∘τ'] ≈ M[σ'][τ'] : A[σ'∘τ'] }} by mauto.
+  enough {{ Δ ; Γ ⊢ M[σ'∘τ'] ≈ M[σ'][τ'] : A[σ∘τ] }} by mauto.
+  eapply wf_exp_eq_conv_typ_eq; mauto 3.
+Qed.
+
+#[export]
+Hint Resolve wf_exp_eq_sub_sub_compose_cong : mcpts.
+
+Lemma wf_exp_sub_id_on_typ {P : PtsSig} : forall {Δ : gctx P} {Γ M A},
+    {{ Δ ; Γ ⊢ A }} ->
+    {{ Δ ; Γ ⊢ M : A }} ->
+    {{ Δ ; Γ ⊢ M : A[Id] }}.
+Proof with mautosolve 3.
+  intros.
+  assert {{ Δ ⊢ Γ }} by mauto 2.
+  eapply wf_exp_conv_typ_eq; mauto 3.
+Qed.
+
+#[export]
+Hint Resolve wf_exp_sub_id_on_typ : mcpts.
+
+Lemma wf_exp_sub_id_on_typ_sorted {P : PtsSig} : forall {Δ : gctx P} {Γ M A s},
+    {{ Δ ; Γ ⊢ A : Sort@s }} ->
+    {{ Δ ; Γ ⊢ M : A }} ->
+    {{ Δ ; Γ ⊢ M : A[Id] }}.
+Proof. mauto 3. Qed.
+
+#[export]
+Hint Resolve wf_exp_sub_id_on_typ_sorted : mcpts.
+
+Lemma wf_sub_id_extend {P : PtsSig} : forall {Δ : gctx P} {Γ M A},
+    {{ Δ ; Γ ⊢ A }} ->
+    {{ Δ ; Γ ⊢ M : A }} ->
+    {{ Δ ; Γ ⊢s Id,,M : Γ, A }}.
+Proof with mautosolve 4.
+  intros.
+  econstructor...
+Qed.
+
+#[export]
+Hint Resolve wf_sub_id_extend : mcpts.
+
+Lemma wf_sub_id_extend_sorted {P : PtsSig} : forall {Δ : gctx P} {Γ M A s},
+    {{ Δ ; Γ ⊢ A : Sort@s }} ->
+    {{ Δ ; Γ ⊢ M : A }} ->
+    {{ Δ ; Γ ⊢s Id,,M : Γ, A }}.
+Proof. mauto 3. Qed.
+
+#[export]
+Hint Resolve wf_sub_id_extend_sorted : mcpts.
+
+Lemma wf_exp_eq_sub_id_on_typ {P : PtsSig} : forall {Δ : gctx P} {Γ M M' A},
+    {{ Δ ; Γ ⊢ A }} ->
+    {{ Δ ; Γ ⊢ M ≈ M' : A }} ->
+    {{ Δ ; Γ ⊢ M ≈ M' : A[Id] }}.
+Proof with mautosolve 4.
+  intros.
+  assert {{ Δ ⊢ Γ }} by mauto 3.
+  eapply wf_exp_eq_conv_typ_eq; mauto 3.
+Qed.
+
+#[export]
+Hint Resolve wf_exp_eq_sub_id_on_typ : mcpts.
+
+Lemma wf_exp_eq_sub_id_on_typ_sorted {P : PtsSig} : forall {Δ : gctx P} {Γ M M' A s},
+    {{ Δ ; Γ ⊢ A : Sort@s }} ->
+    {{ Δ ; Γ ⊢ M ≈ M' : A }} ->
+    {{ Δ ; Γ ⊢ M ≈ M' : A[Id] }}.
+Proof. mauto 3. Qed.
+  
+#[export]
+Hint Resolve wf_exp_eq_sub_id_on_typ_sorted : mcpts.
+
+Lemma wf_sub_eq_p_id_extend {P : PtsSig} : forall {Δ : gctx P} {Γ M A},
+    {{ Δ ; Γ ⊢ A }} ->
+    {{ Δ ; Γ ⊢ M : A }} ->
+    {{ Δ ; Γ ⊢s Wk∘(Id,,M) ≈ Id : Γ }}.
+Proof with mautosolve 3.
+  intros.
+  econstructor...
+Qed.
+
+#[export]
+Hint Resolve wf_sub_eq_p_id_extend : mcpts.
+#[export]
+Hint Rewrite -> @wf_sub_eq_p_id_extend using mauto 4 : mcpts.
+
+
+Lemma wf_sub_eq_p_id_extend_sorted {P : PtsSig} : forall {Δ : gctx P} {Γ M A s},
+    {{ Δ ; Γ ⊢ A : Sort@s }} ->
+    {{ Δ ; Γ ⊢ M : A }} ->
+    {{ Δ ; Γ ⊢s Wk∘(Id,,M) ≈ Id : Γ }}.
+Proof. mauto 3. Qed.
+
+#[export]
+Hint Resolve wf_sub_eq_p_id_extend_sorted : mcpts.
+#[export]
+Hint Rewrite -> @wf_sub_eq_p_id_extend_sorted using mauto 4 : mcpts.
+
+
+Lemma wf_sub_eq_id_extend_cong {P : PtsSig} : forall {Δ : gctx P} {Γ M M' A},
+    {{ Δ ; Γ ⊢ A }} ->
+    {{ Δ ; Γ ⊢ M ≈ M' : A }} ->
+    {{ Δ ; Γ ⊢s Id,,M ≈ Id,,M' : Γ, A }}.
+Proof with mautosolve 3.
+  intros.
+  econstructor...
+Qed.
+
+#[export]
+Hint Resolve wf_sub_eq_id_extend_cong : mcpts.
+
+
+Lemma wf_sub_eq_id_extend_cong_sorted {P : PtsSig} : forall {Δ : gctx P} {Γ M M' A s},
+    {{ Δ ; Γ ⊢ A : Sort@s }} ->
+    {{ Δ ; Γ ⊢ M ≈ M' : A }} ->
+    {{ Δ ; Γ ⊢s Id,,M ≈ Id,,M' : Γ, A }}.
+Proof. mauto 3. Qed.
+
+#[export]
+Hint Resolve wf_sub_eq_id_extend_cong_sorted : mcpts.
+
+
+Lemma wf_sub_q {P : PtsSig} : forall {Δ : gctx P} {Γ Γ' A σ},
+    {{ Δ ; Γ' ⊢ A }} ->
+    {{ Δ ; Γ ⊢s σ : Γ' }} ->
+    {{ Δ ; Γ, A[σ] ⊢s q σ : Γ', A }}.
+Proof with mautosolve 3.
+  intros.
+  assert {{ Δ ⊢ Γ }} by mauto 2.
+  assert {{ Δ ; Γ ⊢ A[σ] }} by mauto 3.
+  assert {{ Δ ; Γ, A[σ] ⊢s Wk : Γ }} by mauto 3.
+  assert {{ Δ ; Γ, A[σ] ⊢ #0 : A[σ][Wk] }} by mauto 3.
+  econstructor; mauto 2.
+  eapply wf_exp_conv_typ_eq; mauto 3.
+Qed.
+
+Lemma wf_sub_q_sort {P : PtsSig} : forall {Δ : gctx P} {Γ Γ' σ s},
+    {{ Δ ; Γ ⊢s σ : Γ' }} ->
+    {{ Δ ; Γ, Sort@s ⊢s q σ : Γ', Sort@s }}.
+Proof with mautosolve 3.
+  intros.
+  assert {{ Δ ⊢ Γ }} by mauto 2.
+  assert {{ Δ ; Γ, Sort@s ⊢s Wk : Γ }} by mauto 4.
+  assert {{ Δ ; Γ, Sort@s ⊢s σ∘Wk : Γ' }} by mauto 4.
+  assert {{ Δ ; Γ, Sort@s ⊢ Sort@s[Wk] ≈ Sort@s }} by mauto 4.
+  assert {{ Δ ; Γ, Sort@s ⊢ #0 : Sort@s }} by mauto 3.
+  econstructor...
+Qed.
+
+Lemma wf_sub_q_nat {P} : forall {Δ : gctx P} {Γ Γ' σ s} {r : Ru_nat P s},
+    {{ Δ ; Γ ⊢s σ : Γ' }} ->
+    {{ Δ ; Γ, ℕ ⊢s q σ : Γ', ℕ }}.
+Proof with mautosolve 3.
+  intros.
+  assert {{ Δ ⊢ Γ }} by mauto 2.
+  assert {{ Δ ; Γ, ℕ ⊢s Wk : Γ }} by mauto 4.
+  assert {{ Δ ; Γ, ℕ ⊢s σ∘Wk : Γ' }} by mauto 4.
+  assert {{ Δ ; Γ, ℕ ⊢ #0 : ℕ }}...
+Qed.
+
+#[export]
+Hint Resolve wf_sub_q wf_sub_q_sort wf_sub_q_nat : mcpts.
+
+Lemma wf_exp_eq_var_1_sub_q_q_sigma_nat {P} : forall {Δ : gctx P} {Γ Γ' A σ s} {r : Ru_nat P s},
+    {{ Δ ; Γ', ℕ ⊢ A }} ->
+    {{ Δ ; Γ ⊢s σ : Γ' }} ->
+    {{ Δ ; Γ, ℕ, A[q σ] ⊢ #1[q (q σ)] ≈ #1 : ℕ }}.
+Proof with mautosolve 3.
+  intros.
+  assert {{ Δ ; Γ, ℕ ⊢s q σ : Γ', ℕ }} by mauto 3.
+  assert {{ Δ ; Γ, ℕ ⊢ A[q σ] }} by mauto 4.
+  assert {{ Δ ⊢ Γ, ℕ, A[q σ] }} by (econstructor; mauto 2).
+  assert {{ Δ; Γ', ℕ ⊢ #0 : ℕ }} by mauto 3.
+  assert {{ Δ ; Γ, ℕ, A[q σ] ⊢ #0 : A[q σ][Wk] }} by mauto 3.
+  assert {{ Δ ; Γ, ℕ, A[q σ] ⊢s q σ∘Wk : Γ', ℕ }} by mauto 3.
+  assert {{ Δ ; Γ, ℕ, A[q σ] ⊢ A[q σ∘Wk] ≈ A[q σ][Wk]  }} by mauto 4.
+  assert {{ Δ ; Γ, ℕ, A[q σ] ⊢ #0 : A[q σ∘Wk] }} by (eapply wf_exp_conv_typ_eq; mauto 4).
+  assert {{ Δ ; Γ, ℕ, A[q σ] ⊢s q σ∘Wk : Γ', ℕ }} by mauto 3.
+  assert {{ Δ ; Γ, ℕ, A[q σ] ⊢ #1[q (q σ)] ≈ #0[q σ∘Wk] : ℕ }} by mauto 3.
+  assert {{ Δ ; Γ, ℕ, A[q σ] ⊢ #0[q σ∘Wk] ≈ #0[q σ][Wk] : ℕ }} by mauto 4.
+  assert {{ Δ ; Γ, ℕ ⊢s σ∘Wk : Γ' }} by mauto 4.
+  assert {{ Δ ; Γ, ℕ ⊢ #0 : ℕ }} by mauto 3.
+  assert {{ Δ ; Γ, ℕ ⊢ #0 : ℕ[σ∘Wk] }} by mauto 3.
+  assert {{ Δ ; Γ, ℕ ⊢ #0[q σ] ≈ #0 : ℕ }} by mauto 3.
+  assert {{ Δ ; Γ, ℕ, A[q σ] ⊢ #0[q σ][Wk] ≈ #0[Wk] : ℕ }} by mauto 3.
+  etransitivity; [eassumption |].
+  etransitivity...
+Qed.
+
+#[export]
+Hint Resolve wf_exp_eq_var_1_sub_q_q_sigma_nat : mcpts.
+
+Lemma wf_exp_eq_var_1_sub_q_q_sigma_nat_sorted {P} : forall {Δ : gctx P} {Γ Γ' A σ s s'} {r : Ru_nat P s},
+    {{ Δ ; Γ', ℕ ⊢ A : Sort@s' }} ->
+    {{ Δ ; Γ ⊢s σ : Γ' }} ->
+    {{ Δ ; Γ, ℕ, A[q σ] ⊢ #1[q (q σ)] ≈ #1 : ℕ }}.
+Proof. mauto 3. Qed.
+
+#[export]
+Hint Resolve wf_exp_eq_var_1_sub_q_q_sigma_nat_sorted : mcpts.
+
+Lemma wf_sub_id_extend_zero {P} : forall {Δ : gctx P} {Γ s} {r : Ru_nat P s},
+    {{ Δ ⊢ Γ }} ->
+    {{ Δ ; Γ ⊢s Id,,zero : Γ, ℕ }}.
+Proof. mauto 4. Qed.
+
+#[export]
+Hint Resolve wf_sub_id_extend_zero : mcpts.
+  
+Lemma wf_sub_weak_compose_weak_extend_succ_var1 {P} : forall {Δ : gctx P} {Γ A s} {r : Ru_nat P s},
+    {{ Δ ; Γ, ℕ ⊢ A }} ->
+    {{ Δ ; Γ, ℕ, A ⊢s Wk∘Wk,,succ #1 : Γ, ℕ }}.
+Proof with mautosolve 4.
+  intros.
+  assert {{ Δ ; Γ, ℕ, A ⊢s Wk : Γ, ℕ  }} by mauto 4.
+  enough {{ Δ ; Γ, ℕ, A ⊢s Wk∘Wk : Γ }}...
+Qed.
+
+#[export]
+Hint Resolve wf_sub_weak_compose_weak_extend_succ_var1 : mcpts.
+
+Lemma wf_sub_weak_compose_weak_extend_succ_var1_sorted {P} : forall {Δ : gctx P} {Γ A s s'} {r : Ru_nat P s},
+    {{ Δ ; Γ, ℕ ⊢ A : Sort@s' }} ->
+    {{ Δ ; Γ, ℕ, A ⊢s Wk∘Wk,,succ #1 : Γ, ℕ }}.
+Proof. mauto 3. Qed.
+
+#[export]
+Hint Resolve wf_sub_weak_compose_weak_extend_succ_var1_sorted : mcpts.
+
+Lemma wf_sub_eq_id_extend_compose {P : PtsSig} : forall {Δ : gctx P} {Γ Γ' M A σ},
+    {{ Δ ; Γ ⊢s σ : Γ' }} ->
+    {{ Δ ; Γ' ⊢ A }} ->
+    {{ Δ ; Γ' ⊢ M : A }} ->
+    {{ Δ ; Γ ⊢s (Id,,M)∘σ ≈ σ,,M[σ] : Γ', A }}.
+Proof with mautosolve 4.
+  intros.
+  assert {{ Δ ; Γ' ⊢s Id : Γ' }} by mauto 3.
+  assert {{ Δ ; Γ' ⊢ M : A[Id] }} by mauto.
+  assert {{ Δ ; Γ ⊢s (Id,,M)∘σ ≈ (Id∘σ),,M[σ] : Γ', A }} by mauto 3.
+  assert {{ Δ ; Γ ⊢ M[σ] : A[Id][σ] }} by mauto.
+  assert {{ Δ ; Γ ⊢ A[Id][σ] ≈ A[Id∘σ] }} by (symmetry; mauto 3).
+  assert {{ Δ ; Γ ⊢ A[Id∘σ] }} by mauto 3.
+  assert {{ Δ ; Γ ⊢ A[Id][σ] ⊆ A[Id∘σ] }} by mauto 4.
+  assert {{ Δ ; Γ ⊢ M[σ] : A[Id∘σ] }} by (eapply wf_exp_conv_typ_eq; mauto 3).
+  enough {{ Δ ; Γ ⊢ M[σ] ≈ M[σ] : A[Id∘σ] }}...
+Qed.
+
+#[export]
+Hint Resolve wf_sub_eq_id_extend_compose : mcpts.
+
+Lemma wf_sub_eq_id_extend_compose_sorted {P : PtsSig} : forall {Δ : gctx P} {Γ Γ' M A σ s},
+    {{ Δ ; Γ ⊢s σ : Γ' }} ->
+    {{ Δ ; Γ' ⊢ A : Sort@s }} ->
+    {{ Δ ; Γ' ⊢ M : A }} ->
+    {{ Δ ; Γ ⊢s (Id,,M)∘σ ≈ σ,,M[σ] : Γ', A }}.
+Proof. mauto 3. Qed.
+
+#[export]
+Hint Resolve wf_sub_eq_id_extend_compose_sorted : mcpts.
+
+Lemma wf_sub_eq_sigma_compose_weak_id_extend {P : PtsSig} : forall {Δ : gctx P} {Γ Γ' M A σ},
+    {{ Δ ; Γ ⊢ A }} ->
+    {{ Δ ; Γ ⊢s σ : Γ' }} ->
+    {{ Δ ; Γ ⊢ M : A }} ->
+    {{ Δ ; Γ ⊢s (σ∘Wk)∘(Id,,M) ≈ σ : Γ' }}.
+Proof with mautosolve.
+  intros.
+  assert {{ Δ ; Γ ⊢s Id,,M : Γ, A }} by mauto.
+  assert {{ Δ ; Γ ⊢s (σ∘Wk)∘(Id,,M) ≈ σ∘(Wk∘(Id,,M)) : Γ' }} by mauto 4.
+  assert {{ Δ ; Γ ⊢s Wk∘(Id,,M) ≈ Id : Γ }} by mauto.
+  enough {{ Δ ; Γ ⊢s σ∘(Wk∘ (Id,,M)) ≈ σ∘Id : Γ' }} by mauto 4.
+  econstructor...
+Qed.
+
+#[export]
+Hint Resolve wf_sub_eq_sigma_compose_weak_id_extend : mcpts.
+
+Lemma wf_sub_eq_sigma_compose_weak_id_extend_sorted {P : PtsSig} : forall {Δ : gctx P} {Γ Γ' M A σ s},
+    {{ Δ ; Γ ⊢ A : Sort@s }} ->
+    {{ Δ ; Γ ⊢s σ : Γ' }} ->
+    {{ Δ ; Γ ⊢ M : A }} ->
+    {{ Δ ; Γ ⊢s (σ∘Wk)∘(Id,,M) ≈ σ : Γ' }}.
+Proof. mauto 3. Qed.
+
+#[export]
+Hint Resolve wf_sub_eq_sigma_compose_weak_id_extend_sorted : mcpts.
+
+Lemma wf_sub_eq_q_sigma_id_extend {P : PtsSig} : forall {Δ : gctx P} {Γ Γ' M A σ},
+    {{ Δ ; Γ' ⊢ A }} ->
+    {{ Δ ; Γ ⊢s σ : Γ' }} ->
+    {{ Δ ; Γ ⊢ M : A[σ] }} ->
+    {{ Δ ; Γ ⊢s q σ∘(Id,,M) ≈ σ,,M : Γ', A }}.
+Proof with mautosolve 4.
+  intros.
+  assert {{ Δ ⊢ Γ }} by mauto 3.
+  assert {{ Δ ; Γ ⊢ A[σ] }} by mauto 3.
+  assert {{ Δ ; Γ ⊢ M : A[σ] }} by mauto.
+  assert {{ Δ ; Γ ⊢s Id,,M : Γ, A[σ] }} by mauto.
+  assert {{ Δ ; Γ, A[σ] ⊢s Wk : Γ }} by mauto 3.
+  assert {{ Δ ; Γ ⊢ A[σ] }} by mauto 2.
+  assert {{ Δ ; Γ, A[σ] ⊢ #0 : A[σ][Wk] }} by mauto 4.
+  assert {{ Δ ; Γ, A[σ] ⊢ #0 : A[σ∘Wk] }} by (eapply wf_exp_conv_typ_eq; mauto 3).
+  assert {{ Δ ; Γ ⊢s q σ∘(Id,,M) ≈ ((σ∘Wk)∘(Id,,M)),,#0[Id,,M] : Γ', A }} by mauto.
+  assert {{ Δ ; Γ ⊢s (σ∘Wk)∘(Id,,M) ≈ σ : Γ' }} by mauto.
+  assert {{ Δ ; Γ ⊢ M : A[σ][Id] }} by mauto 4.
+  assert {{ Δ ; Γ ⊢ #0[Id,,M] ≈ M : A[σ][Id] }} by mauto 4.
+  assert {{ Δ ; Γ ⊢ #0[Id,,M] ≈ M : A[σ] }} by mauto 4.
+  enough {{ Δ ; Γ ⊢ #0[Id,,M] ≈ M : A[(σ∘Wk)∘(Id,,M)] }} by mauto.
+  assert {{ Δ ; Γ ⊢s (σ∘Wk)∘(Id,,M) : Γ' }} by mauto 3.
+  assert {{ Δ ; Γ ⊢ A[(σ∘Wk)∘(Id,,M)] }} by mauto 3.
+  eapply wf_exp_eq_conv_typ_eq; mauto 3.
+Qed.
+
+#[export]
+Hint Resolve wf_sub_eq_q_sigma_id_extend : mcpts.
+#[export]
+Hint Rewrite -> @wf_sub_eq_q_sigma_id_extend using mauto 4 : mcpts.
+
+Lemma wf_sub_eq_q_sigma_id_extend_sorted {P : PtsSig} : forall {Δ : gctx P} {Γ Γ' M A σ s},
+    {{ Δ ; Γ' ⊢ A : Sort@s }} ->
+    {{ Δ ; Γ ⊢s σ : Γ' }} ->
+    {{ Δ ; Γ ⊢ M : A[σ] }} ->
+    {{ Δ ; Γ ⊢s q σ∘(Id,,M) ≈ σ,,M : Γ', A }}.
+Proof. mauto 3. Qed.
+
+#[export]
+Hint Resolve wf_sub_eq_q_sigma_id_extend_sorted : mcpts.
+#[export]
+Hint Rewrite -> @wf_sub_eq_q_sigma_id_extend_sorted using mauto 4 : mcpts.
+
+Lemma wf_sub_eq_q_sigma_extend_tau {P} : forall {Δ : gctx P } {Γ1 Γ2 Γ3 A σ τ M},
+    {{ Δ ; Γ3 ⊢ A }} ->
+    {{ Δ ; Γ2 ⊢s σ : Γ3 }} ->
+    {{ Δ ; Γ1 ⊢s τ : Γ2 }} ->
+    {{ Δ ; Γ1 ⊢ M : A[σ][τ] }} ->
+    {{ Δ ; Γ1 ⊢s (q σ)∘(τ,,M) ≈ (σ∘τ),,M : Γ3, A }}.
 Proof.
   intros.
-  assert {{ Δ ⊢ A[σ] }} by mauto 4.
-  assert {{ Γ ⊢ A[σ][τ] }} by mauto 3.
-  assert {{ Γ ⊢ A[σ∘τ] }} by mauto 3.
-  eapply wf_conv; mauto 3.
+  assert {{ Δ ; Γ2, A[σ] ⊢s σ ∘ Wk : Γ3 }} by mauto.
+  assert {{ Δ ; Γ2 ⊢ A[σ] }} by mauto 3.
+  assert {{ Δ ; Γ2, A[σ] ⊢s Wk : Γ2 }} by mauto 3.
+  assert {{ Δ ; Γ2, A[σ] ⊢ A[σ][Wk] }} by mauto 3.
+  assert {{ Δ ; Γ2, A[σ] ⊢ #0 : A[σ][Wk] }} by mauto 4.
+  assert {{ Δ ; Γ2, A[σ] ⊢ A[σ][Wk] ≈ A[σ∘Wk] }} by mauto.
+  assert {{ Δ ; Γ2, A[σ] ⊢ #0 : A[σ∘Wk] }} by mauto 3.
+  assert {{ Δ ; Γ1 ⊢s (q σ) ∘ (τ,,M) ≈ ((σ∘Wk)∘(τ,,M)),,#0[τ,,M] : Γ3, A }} by mauto 3.
+  assert {{ Δ ; Γ1 ⊢s (σ∘Wk)∘(τ,,M) ≈ σ∘(Wk∘(τ,,M)) : Γ3 }} by (econstructor; mauto 3).
+  assert {{ Δ ; Γ1 ⊢s σ∘(Wk∘(τ,,M)) ≈ σ∘τ : Γ3 }} by mauto 4.
+  assert {{ Δ ; Γ1 ⊢s (σ ∘ Wk) ∘ (τ,,M) ≈ σ∘τ : Γ3 }} by (etransitivity; mauto).
+  assert {{ Δ ; Γ1 ⊢ #0[τ,,M] ≈ M : A[σ][τ] }} by mauto.
+  assert {{ Δ ; Γ3 ⊢ A }} by mauto 2.
+  assert {{ Δ ; Γ1 ⊢ A[σ][τ] ≈ A[σ∘τ] }} by mauto 3.
+  assert {{ Δ ; Γ1 ⊢ A[σ][τ] ≈ A[(σ∘Wk)∘(τ,,M)] }} by (etransitivity; mauto 4).
+  assert {{ Δ ; Γ1 ⊢s (σ∘Wk)∘(τ,,M) : Γ3 }} by mauto 3.
+  assert {{ Δ ; Γ1 ⊢ A[(σ∘Wk)∘(τ,,M)] }} by mauto 2.
+  assert {{ Δ ; Γ1 ⊢s (σ∘Wk)∘(τ,,M),,#0[τ,,M] ≈ σ∘τ,,M : Γ3, A }} by (econstructor; mauto).
+  do 2 etransitivity; mauto.
+Qed.
+
+#[export]
+Hint Resolve wf_sub_eq_q_sigma_extend_tau : mcpts.
+#[export]
+Hint Rewrite -> @wf_sub_eq_q_sigma_extend_tau using mauto 4 : mcpts.
+
+Lemma wf_sub_eq_q_sigma_extend_tau_sorted {P} : forall {Δ : gctx P } {Γ1 Γ2 Γ3 A σ τ M s},
+    {{ Δ ; Γ3 ⊢ A : Sort@s }} ->
+    {{ Δ ; Γ2 ⊢s σ : Γ3 }} ->
+    {{ Δ ; Γ1 ⊢s τ : Γ2 }} ->
+    {{ Δ ; Γ1 ⊢ M : A[σ][τ] }} ->
+    {{ Δ ; Γ1 ⊢s (q σ)∘(τ,,M) ≈ (σ∘τ),,M : Γ3, A }}.
+Proof. mauto 3. Qed.
+
+#[export]
+Hint Resolve wf_sub_eq_q_sigma_extend_tau : mcpts.
+#[export]
+Hint Rewrite -> @wf_sub_eq_q_sigma_extend_tau using mauto 4 : mcpts.
+
+
+Lemma wf_sub_eq_p_q_sigma {P : PtsSig} : forall {Δ : gctx P} {Γ Γ' A σ},
+    {{ Δ ; Γ' ⊢ A }} ->
+    {{ Δ ; Γ ⊢s σ : Γ' }} ->
+    {{ Δ ; Γ, A[σ] ⊢s Wk∘q σ ≈ σ∘Wk : Γ' }}.
+Proof with mautosolve 3.
+  intros.
+  assert {{ Δ ; Γ, A[σ] ⊢s Wk : Γ }} by mauto 4.
+  assert {{ Δ ; Γ ⊢ A[σ] }} by mauto 3.
+  assert {{ Δ ; Γ, A[σ] ⊢ #0 : A[σ][Wk] }} by mauto 4.
+  enough {{ Δ ; Γ, A[σ] ⊢ #0 : A[σ∘Wk] }} by mauto.
+  eapply wf_exp_conv_typ_eq; mauto 3.
+Qed.
+
+#[export]
+Hint Resolve wf_sub_eq_p_q_sigma : mcpts.
+
+Lemma wf_sub_eq_p_q_sigma_sorted {P : PtsSig} : forall {Δ : gctx P} {Γ Γ' A σ s},
+    {{ Δ ; Γ' ⊢ A : Sort@s }} ->
+    {{ Δ ; Γ ⊢s σ : Γ' }} ->
+    {{ Δ ; Γ, A[σ] ⊢s Wk∘q σ ≈ σ∘Wk : Γ' }}.
+Proof. mauto 3. Qed.
+
+#[export]
+Hint Resolve wf_sub_eq_p_q_sigma_sorted : mcpts.
+
+Lemma wf_sub_eq_p_q_sigma_nat {P} : forall {Δ : gctx P} {Γ Γ' σ s} {r : Ru_nat P s},
+    {{ Δ ; Γ ⊢s σ : Γ' }} ->
+    {{ Δ ; Γ, ℕ ⊢s Wk∘q σ ≈ σ∘Wk : Γ' }}.
+Proof with mautosolve 3.
+  intros.
+  assert {{ Δ ⊢ Γ, ℕ }} by mauto 3.
+  assert {{ Δ ; Γ, ℕ ⊢s Wk : Γ }} by mauto 2.
+  assert {{ Δ ; Γ, ℕ ⊢ #0 : ℕ }}...
+Qed.
+
+#[export]
+Hint Resolve wf_sub_eq_p_q_sigma_nat : mcpts.
+
+Lemma wf_sub_eq_p_p_q_q_sigma_nat {P} : forall {Δ : gctx P} {Γ Γ' A σ s} {r : Ru_nat P s},
+    {{ Δ ; Γ', ℕ ⊢ A }} ->
+    {{ Δ ; Γ ⊢s σ : Γ' }} ->
+    {{ Δ ; Γ, ℕ, A[q σ] ⊢s Wk∘(Wk∘q (q σ)) ≈ (σ∘Wk)∘Wk : Γ' }}.
+Proof with mautosolve 3.
+  intros.
+  assert {{ Δ ; Γ, ℕ ⊢ A[q σ] }} by mauto 4.
+  assert {{ Δ ⊢ Γ, ℕ, A[q σ] }} by mauto 3.
+  assert {{ Δ ⊢ Γ', ℕ }} by mauto 3.
+  assert {{ Δ ; Γ, ℕ, A[q σ] ⊢s Wk∘q (q σ) ≈ q σ∘Wk : Γ', ℕ }} by mauto.
+  assert {{ Δ ; Γ, ℕ, A[q σ] ⊢s Wk∘(Wk∘q (q σ)) ≈ Wk∘(q σ∘Wk) : Γ' }} by mauto 3.
+  assert {{ Δ ; Γ', ℕ ⊢s Wk : Γ' }} by mauto.
+  assert {{ Δ ; Γ, ℕ ⊢s q σ : Γ', ℕ }} by mauto.
+  assert {{ Δ ; Γ, ℕ, A[q σ] ⊢s Wk∘(q σ∘Wk) ≈ (Wk∘q σ)∘Wk : Γ' }} by mauto 4.
+  assert {{ Δ ; Γ, ℕ ⊢s Wk∘q σ ≈ σ∘Wk : Γ' }} by mauto.
+  enough {{ Δ ; Γ, ℕ, A[q σ] ⊢s (Wk∘q σ)∘Wk ≈ (σ∘Wk)∘Wk : Γ' }}...
+Qed.
+
+#[export]
+Hint Resolve wf_sub_eq_p_p_q_q_sigma_nat : mcpts.
+
+Lemma wf_sub_eq_p_p_q_q_sigma_nat_sorted {P} : forall {Δ : gctx P} {Γ Γ' A σ s s'} {r : Ru_nat P s},
+    {{ Δ ; Γ', ℕ ⊢ A : Sort@s' }} ->
+    {{ Δ ; Γ ⊢s σ : Γ' }} ->
+    {{ Δ ; Γ, ℕ, A[q σ] ⊢s Wk∘(Wk∘q (q σ)) ≈ (σ∘Wk)∘Wk : Γ' }}.
+Proof. mauto 3. Qed.
+
+#[export]
+Hint Resolve wf_sub_eq_p_p_q_q_sigma_nat_sorted : mcpts.
+
+Lemma wf_sub_eq_q_sigma_compose_weak_weak_extend_succ_var1 {P} : forall {Δ : gctx P} {Γ Γ' A σ s} {r : Ru_nat P s},
+    {{ Δ ; Γ', ℕ ⊢ A }} ->
+    {{ Δ ; Γ ⊢s σ : Γ' }} ->
+    {{ Δ ; Γ, ℕ, A[q σ] ⊢s q σ∘(Wk∘Wk,,succ #1) ≈ (Wk∘Wk,,succ #1)∘q (q σ) : Γ', ℕ }}.
+Proof with mautosolve 3.
+  intros.
+  assert {{ Δ ⊢ Γ', ℕ, A }} by mauto 3.
+  assert {{ Δ ⊢ Γ, ℕ }} by mauto 3.
+  assert {{ Δ ; Γ, ℕ ⊢s Wk : Γ }} by mauto 3.
+  assert {{ Δ ; Γ, ℕ ⊢s σ∘Wk : Γ' }} by mauto 3.
+  assert {{ Δ ; Γ, ℕ ⊢ A[q σ] }} by mauto 4.
+  set (Γ'' := {{{ Γ, ℕ, A[q σ] }}}).
+  set (WkWksucc := {{{ (Wk∘Wk),,succ #1 }}}).
+  assert {{ Δ ⊢ Γ'' }} by mauto 2.
+  assert {{ Δ ; Γ'' ⊢s Wk∘Wk : Γ }} by mauto 3.
+  assert {{ Δ ; Γ'' ⊢s WkWksucc : Γ, ℕ }} by mauto 4.
+  assert {{ Δ ; Γ, ℕ ⊢ #0 : ℕ}} by mauto 3.
+  assert {{ Δ ; Γ'' ⊢s q σ∘WkWksucc ≈ ((σ∘Wk)∘WkWksucc),,#0[WkWksucc] : Γ', ℕ }} by mautosolve 3.
+  assert {{ Δ ; Γ'' ⊢ #1 : ℕ[Wk][Wk] }} by mauto.
+  assert {{ Δ ; Γ'' ⊢ ℕ[Wk][Wk] ≈ ℕ : Sort@s }} by mauto 3.
+  assert {{ Δ ; Γ'' ⊢ #1 : ℕ }} by mauto 2.
+  assert {{ Δ ; Γ'' ⊢ succ #1 : ℕ }} by mauto.
+  assert {{ Δ ; Γ'' ⊢s Wk∘WkWksucc : Γ }} by mauto 4.
+  assert {{ Δ ; Γ'' ⊢s Wk∘WkWksucc ≈ Wk∘Wk : Γ }} by mauto 4.
+  assert {{ Δ ; Γ ⊢s σ ≈ σ : Γ' }} by mauto.
+  assert {{ Δ ; Γ'' ⊢s σ∘(Wk∘WkWksucc) ≈ σ∘(Wk∘Wk) : Γ' }} by mauto 3.
+  assert {{ Δ ; Γ'' ⊢s (σ∘Wk)∘WkWksucc ≈ σ∘(Wk∘Wk) : Γ' }} by mauto 3.
+  assert {{ Δ ; Γ'' ⊢s σ∘(Wk∘Wk) ≈ (σ∘Wk)∘Wk : Γ' }} by mauto 4.
+  assert {{ Δ ; Γ'' ⊢s (σ∘Wk)∘Wk ≈ Wk∘(Wk∘q (q σ)) : Γ' }} by mauto.
+  assert {{ Δ ; Γ', ℕ ⊢s Wk : Γ' }} by mauto 4.
+  assert {{ Δ ; Γ', ℕ, A ⊢s Wk : Γ', ℕ }} by mauto 4.
+  assert {{ Δ ; Γ', ℕ, A ⊢s Wk∘Wk : Γ' }} by mauto 4.
+  assert {{ Δ ; Γ'' ⊢s q (q σ) : Γ', ℕ, A }} by mauto.
+  assert {{ Δ ; Γ'' ⊢s Wk∘(Wk∘q (q σ)) ≈ (Wk∘Wk)∘q (q σ) : Γ' }} by mauto 3.
+  assert {{ Δ ; Γ'' ⊢s σ∘(Wk∘Wk) ≈ (Wk∘Wk)∘q (q σ) : Γ' }} by mauto 3.
+  assert {{ Δ ; Γ'' ⊢ #0[WkWksucc] ≈ succ #1 : ℕ }} by mauto.
+  assert {{ Δ ; Γ'' ⊢ succ #1[q (q σ)] ≈ succ #1 : ℕ }} by mauto 3.
+  assert {{ Δ ; Γ', ℕ, A ⊢ #1 : ℕ }} by mauto 2.
+  assert {{ Δ ; Γ'' ⊢ succ #1 ≈ (succ #1)[q (q σ)] : ℕ }} by mauto 4.
+  assert {{ Δ ; Γ'' ⊢ #0[WkWksucc] ≈ (succ #1)[q (q σ)] : ℕ }} by mauto 2.
+  assert {{ Δ ; Γ'' ⊢s (σ∘Wk)∘WkWksucc : Γ' }} by mauto 3.
+  assert {{ Δ ; Γ'' ⊢s ((σ∘Wk)∘WkWksucc),,#0[WkWksucc] ≈ ((Wk∘Wk)∘q (q σ)),,(succ #1)[q (q σ)] : Γ', ℕ }} by mauto 3.
+  assert {{ Δ ; Γ', ℕ, A ⊢ #1 : ℕ[Wk][Wk] }} by mauto 4.
+  assert {{ Δ ; Γ', ℕ, A ⊢ ℕ[Wk][Wk] ≈ ℕ : Sort@s }} by mauto 3.
+  assert {{ Δ ; Γ', ℕ, A ⊢ succ #1 : ℕ }} by mauto 4.
+  enough {{ Δ ; Γ'' ⊢s ((Wk∘Wk)∘q (q σ)),,(succ #1)[q (q σ)] ≈ WkWksucc∘q (q σ) : Γ', ℕ }}...
+Qed.
+
+#[export]
+Hint Resolve wf_sub_eq_q_sigma_compose_weak_weak_extend_succ_var1 : mcpts.
+
+Lemma wf_sub_eq_q_sigma_compose_weak_weak_extend_succ_var1_unsorted {P} : forall {Δ : gctx P} {Γ Γ' A σ s s'} {r : Ru_nat P s},
+    {{ Δ ; Γ', ℕ ⊢ A : Sort@s' }} ->
+    {{ Δ ; Γ ⊢s σ : Γ' }} ->
+    {{ Δ ; Γ, ℕ, A[q σ] ⊢s q σ∘(Wk∘Wk,,succ #1) ≈ (Wk∘Wk,,succ #1)∘q (q σ) : Γ', ℕ }}.
+Proof. mauto 3. Qed.
+#[export]
+Hint Resolve wf_sub_eq_q_sigma_compose_weak_weak_extend_succ_var1_unsorted : mcpts.
+
+
+(** *** Lemmas for [wf_subtyp] *)
+
+Fact wf_typ_subtyp_refl_sorted {P} : forall {Δ : gctx P} {Γ A s},
+    {{ Δ ; Γ ⊢ A : Sort@s }} ->
+    {{ Δ ; Γ ⊢ A ⊆ A }}.
+Proof. mauto. Qed.
+
+#[export]
+Hint Resolve wf_typ_subtyp_refl_sorted : mcpts.
+
+Lemma wf_typ_subtyp_sub {P} : forall {Δ : gctx P} {Γ' A A'},
+    {{ Δ ; Γ' ⊢ A ⊆ A' }} ->
+    forall Γ σ,
+      {{ Δ ; Γ ⊢s σ : Γ' }} ->
+      {{ Δ ; Γ ⊢ A[σ] ⊆ A'[σ] }}.
+Proof.
+  induction 1; intros; mauto 4.
+  (* - assert {{ Γ0 ⊢ A[σ] ≈ B[σ] }} by mauto 3. *)
+  (*   assert {{ Γ0 ⊢ B[σ] }} by mauto 3. *)
+  (*   mauto 3. *)
+  - assert {{ Δ ⊢ Γ0 }} by mauto 2.
+    assert {{ Δ ; Γ ⊢ Sort@s1 ⊆ Sort@s2 }} by mauto.
+    assert {{ Δ ; Γ ⊢ Sort@s1 }} by mauto.
+    assert {{ Δ ; Γ0 ⊢ Sort@s1[σ] ≈ Sort@s1 }} by mauto.
+    assert {{ Δ ; Γ0 ⊢ Sort@s2 ≈ Sort@s2[σ] }} by (symmetry; mauto).
+    transitivity {{{ Sort@s1 }}}; mauto 3.
+    transitivity {{{ Sort@s2 }}}; mauto 3.
+  - assert {{ Δ ; Γ0 ⊢ A[σ] : Sort@s1 }} by mauto 3.
+    assert {{ Δ ; Γ0, A[σ] ⊢ B[q σ] : Sort@s2 }} by mauto 4.
+    assert {{ Δ ; Γ0 ⊢ Π r A[σ] B[q σ] }} by mauto 3.
+    transitivity {{{ Π r (A[σ]) (B[q σ]) }}}; [econstructor; mauto 3|].
+    transitivity {{{ Π r (A'[σ]) (B'[q σ]) }}}; [ | econstructor; mauto 4].
+    eapply wf_typ_subtyp_pi; mauto 4.
+Qed.
+
+#[export]
+Hint Resolve wf_typ_subtyp_sub : mcpts.
+
+Lemma wf_subtyp_sort_weaken {P} : forall {Δ : gctx P} {Γ s1 s2 A},
+    {{ Δ ; Γ ⊢ Sort@s1 ⊆ Sort@s2 }} ->
+    {{ Δ ⊢ Γ, A }} ->
+    {{ Δ ; Γ, A ⊢ Sort@s1 ⊆ Sort@s2 }}.
+Proof.    
+  intros.
+  assert {{ Δ ; Γ ⊢ Sort@s2  }} by mauto 2.
+  assert {{ Δ ; Γ, A ⊢s Wk : Γ }} by mauto 2.
+  transitivity {{{ Sort@s1[Wk] }}}; mauto 3.
+  transitivity {{{ Sort@s2[Wk] }}}; mauto 3.
+Qed.
+
+#[export]
+Hint Resolve wf_subtyp_sort_weaken : mcpts.
+
+Lemma wf_ctx_subtyp_ctx_lookup {P} : forall {Δ : gctx P} {Γ Γ'},
+    {{ Δ ⊢ Γ' ⊆ Γ }} ->
+    forall {A x},
+      {{ #x : A ∈ Γ }} ->
+      exists B,
+        {{ #x : B ∈ Γ' }} /\
+          {{ Δ ; Γ' ⊢ B ⊆ A }}.
+Proof with (do 2 eexists; repeat split; mautosolve).
+  induction 1; intros * Hx; progressive_inversion.
+  dependent destruction Hx.
+  - eexists; split; mauto 3.
+    eapply wf_typ_subtyp_sub; mauto 4.
+  - edestruct IHwf_ctx_subtyp as [? []]; try eassumption...
+Qed.
+
+#[export]
+Hint Resolve wf_ctx_subtyp_ctx_lookup : mcpts.
+
+Lemma wf_gctx_subtyp_gctx_lookup {P} : forall {Δ Δ' : gctx P},
+    {{ ⊢ Δ' ⊆ Δ }} ->
+    forall {A x},
+      {{ `#x : A ∈ Δ }} ->
+      exists B,
+        {{ `#x : B ∈ Δ' }} /\
+          {{ Δ' ; ⋅ ⊢ B ⊆ A }}.
+Proof with (do 2 eexists; repeat split; mautosolve).
+  induction 1; intros * Hx; progressive_inversion.
+  dependent destruction Hx.
+  - eexists; split; mauto 3.
+    eapply wf_typ_subtyp_gctx_weakening; mauto 3.
+  - edestruct IHwf_gctx_subtyp as [? []]; try eassumption...
+Qed.
+
+#[export]
+Hint Resolve wf_gctx_subtyp_gctx_lookup : mcpts.
+
+Lemma wf_exp_sort_implies_axiom {P} : forall {Δ : gctx P} {Γ s1 K},
+    {{ Δ ; Γ ⊢ Sort@s1 : K }} ->
+    exists s2,
+      Ax_typ P s1 s2 /\
+        {{ Δ ; Γ ⊢ Sort@s2 ⊆ K }}.
+Proof.
+  intros * H.
+  dependent induction H.
+  - eexists; split; mauto 2.
+  - specialize (IHwf_exp _ s1 A ltac:(reflexivity) ltac:(reflexivity) ltac:(reflexivity)) as [s2 []].
+    eexists; mauto.
+Qed.
+
+#[export]
+Hint Resolve wf_exp_sort_implies_axiom : mcpts.
+
+
+(** *** Lemmas about variables *)
+Lemma var_compose_subs {P : PtsSig} : forall {Δ : gctx P} {Γ Γ' Γ'' τ σ A x},
+    {{ Δ ; Γ'' ⊢ A }} ->
+    {{ Δ ; Γ' ⊢s σ : Γ'' }} ->
+    {{ Δ ; Γ ⊢s τ : Γ' }} ->
+    {{ #x : A[σ][τ] ∈ Γ }} ->
+    {{ Δ ; Γ ⊢ #x : A[σ∘τ] }}.
+Proof.
+  intros.
+  assert {{ Δ ; Γ' ⊢ A[σ] }} by mauto 4.
+  assert {{ Δ ; Γ ⊢ A[σ][τ] }} by mauto 3.
+  assert {{ Δ ; Γ ⊢ A[σ∘τ] }} by mauto 3.
+  eapply wf_exp_conv_typ_eq; mauto 3.
 Qed.
 
 #[export]
 Hint Resolve var_compose_subs : mcpts.
 
-Lemma sub_lookup_var0 {P : PtsSig} : forall (Δ : ctx P) Γ σ M1 M2 B,
-    {{ Δ ⊢s σ : Γ }} ->
-    {{ Γ ⊢ B }} ->
-    {{ Δ ⊢ M1 : B[σ] }} ->
-    {{ Δ ⊢ M2 : B[σ] }} ->
-    {{ Δ ⊢ #0[σ,,M1,,M2] ≈ M2 : B[σ] }}.
+Lemma sub_lookup_var0 {P : PtsSig} : forall (Δ : gctx P) Γ Γ' σ M1 M2 B,
+    {{ Δ ; Γ' ⊢s σ : Γ }} ->
+    {{ Δ ; Γ ⊢ B }} ->
+    {{ Δ ; Γ' ⊢ M1 : B[σ] }} ->
+    {{ Δ ; Γ' ⊢ M2 : B[σ] }} ->
+    {{ Δ ; Γ' ⊢ #0[σ,,M1,,M2] ≈ M2 : B[σ] }}.
 Proof.
   intros.
-  assert {{ Γ, B ⊢ B[Wk] }} by mauto 4.
-  assert {{ Δ ⊢s σ,,M1 : Γ, B }} by mauto 3.
-  assert {{ Δ ⊢ B[Wk][σ,,M1] }} by mauto 4.
-  assert {{ Δ ⊢ B[Wk][σ,,M1] ≈ B[σ] }} by mauto 3.
-  eapply wf_eq_conv; mauto 3.
+  assert {{ Δ ; Γ, B ⊢ B[Wk] }} by mauto 4.
+  assert {{ Δ ; Γ' ⊢s σ,,M1 : Γ, B }} by mauto 3.
+  assert {{ Δ ; Γ' ⊢ B[Wk][σ,,M1] }} by mauto 4.
+  assert {{ Δ ; Γ' ⊢ B[Wk][σ,,M1] ≈ B[σ] }} by mauto 3.
+  eapply wf_exp_eq_conv_typ_eq; mauto 3.
   eapply wf_exp_eq_var_0_sub with (A := {{{ B[Wk] }}}); [| | econstructor]; mauto.
 Qed.
 
-Lemma id_sub_lookup_var0 {P : PtsSig} : forall (Γ : ctx P) M1 M2 B,
-    {{ Γ ⊢ B }} ->
-    {{ Γ ⊢ M1 : B }} ->
-    {{ Γ ⊢ M2 : B }} ->
-    {{ Γ ⊢ #0[Id,,M1,,M2] ≈ M2 : B }}.
+#[export]
+Hint Resolve sub_lookup_var0 : mcpts.
+
+Lemma id_sub_lookup_var0 {P : PtsSig} : forall (Δ : gctx P) Γ M1 M2 B,
+    {{ Δ ; Γ ⊢ B }} ->
+    {{ Δ ; Γ ⊢ M1 : B }} ->
+    {{ Δ ; Γ ⊢ M2 : B }} ->
+    {{ Δ ; Γ ⊢ #0[Id,,M1,,M2] ≈ M2 : B }}.
 Proof.
   intros.
   eapply wf_exp_eq_conv;
@@ -1797,29 +2242,34 @@ Proof.
     mauto 4.
 Qed.
 
-
-Lemma sub_lookup_var1 {P : PtsSig} : forall (Δ : ctx P) Γ σ M1 M2 B,
-    {{ Δ ⊢s σ : Γ }} ->
-    {{ Γ ⊢ B }} ->
-    {{ Δ ⊢ M1 : B[σ] }} ->
-    {{ Δ ⊢ M2 : B[σ] }} ->
-    {{ Δ ⊢ #1[σ,,M1,,M2] ≈ M1 : B[σ] }}.
+#[export]
+Hint Resolve id_sub_lookup_var0 : mcpts.
+ 
+Lemma sub_lookup_var1 {P : PtsSig} : forall (Δ : gctx P) Γ Γ' σ M1 M2 B,
+    {{ Δ ; Γ' ⊢s σ : Γ }} ->
+    {{ Δ ; Γ ⊢ B }} ->
+    {{ Δ ; Γ' ⊢ M1 : B[σ] }} ->
+    {{ Δ ; Γ' ⊢ M2 : B[σ] }} ->
+    {{ Δ ; Γ' ⊢ #1[σ,,M1,,M2] ≈ M1 : B[σ] }}.
 Proof.
   intros.
-  assert {{ Γ, B ⊢ B[Wk] }} by mauto 4.
-  assert {{ Δ ⊢s σ,,M1 : Γ, B }} by mauto 3.
-  assert {{ Δ ⊢ B[Wk][σ,,M1] }} by mauto 4.
-  assert {{ Δ ⊢ B[Wk][σ,,M1] ≈ B[σ] }} by mauto 3.
-  assert {{ Δ ⊢ B[σ]}} by mauto 4.
-  assert {{ Δ ⊢ M2 : B[Wk][σ,,M1] }} by mauto 3.
+  assert {{ Δ ; Γ, B ⊢ B[Wk] }} by mauto 4.
+  assert {{ Δ ; Γ' ⊢s σ,,M1 : Γ, B }} by mauto 3.
+  assert {{ Δ ; Γ' ⊢ B[Wk][σ,,M1] }} by mauto 4.
+  assert {{ Δ ; Γ' ⊢ B[Wk][σ,,M1] ≈ B[σ] }} by mauto 3.
+  assert {{ Δ ; Γ' ⊢ B[σ]}} by mauto 4.
+  assert {{ Δ ; Γ' ⊢ M2 : B[Wk][σ,,M1] }} by mauto 3.
   transitivity {{{ #0[σ,,M1] }}}; mauto 3.
 Qed.
 
-Lemma id_sub_lookup_var1 {P : PtsSig} : forall (Γ : ctx P) M1 M2 B,
-    {{ Γ ⊢ B }} ->
-    {{ Γ ⊢ M1 : B }} ->
-    {{ Γ ⊢ M2 : B }} ->
-    {{ Γ ⊢ #1[Id,,M1,,M2] ≈ M1 : B }}.
+#[export]
+Hint Resolve sub_lookup_var1 : mcpts.
+
+Lemma id_sub_lookup_var1 {P : PtsSig} : forall (Δ : gctx P) Γ M1 M2 B,
+    {{ Δ ; Γ ⊢ B }} ->
+    {{ Δ ; Γ ⊢ M1 : B }} ->
+    {{ Δ ; Γ ⊢ M2 : B }} ->
+    {{ Δ ; Γ ⊢ #1[Id,,M1,,M2] ≈ M1 : B }}.
 Proof.
   intros.
   eapply wf_exp_eq_conv;
@@ -1827,107 +2277,90 @@ Proof.
     mauto 4.
 Qed.
 
-Lemma exp_eq_var_1_sub_q_sigma {P : PtsSig} : forall {Γ : ctx P} {A B σ Δ},
-    {{ Δ ⊢ B }} ->
-    {{ Δ, B ⊢ A }} ->
-    {{ Γ ⊢s σ : Δ }} ->
-    {{ Γ, B[σ], A[q σ] ⊢ #1[q (q σ)] ≈ #1 : B[σ][Wk∘Wk] }}.
+#[export]
+Hint Resolve id_sub_lookup_var1 : mcpts.
+
+Lemma wf_exp_eq_var_1_sub_q_sigma {P : PtsSig} : forall {Δ : gctx P} {Γ Γ' A B σ},
+    {{ Δ ; Γ' ⊢ B }} ->
+    {{ Δ ; Γ', B ⊢ A }} ->
+    {{ Δ ; Γ ⊢s σ : Γ' }} ->
+    {{ Δ ; Γ, B[σ], A[q σ] ⊢ #1[q (q σ)] ≈ #1 : B[σ][Wk∘Wk] }}.
 Proof with mautosolve 3.
   intros.
-  assert {{ ⊢ Δ }} by mauto 2.
-  assert {{ Γ, B[σ] ⊢s q σ : Δ, B }} by mauto 2.
-  assert {{ ⊢ Γ, B[σ] }} by mauto 3.
-  assert {{ ⊢ Γ, B[σ], A[q σ] }} by mauto 3.
-  assert {{ Δ, B ⊢ B[Wk]  }} by mauto 4.
-  assert {{ Δ ⊢ B }} by mauto 2.
-  assert {{ Δ, B ⊢ #0 : B[Wk] }} by mauto 4.
-  assert {{ Γ, B[σ] ⊢ A[q σ] }} by mauto 3.
-  assert {{ Γ, B[σ], A[q σ] ⊢ #0 : A[q σ][Wk] }} by mauto 4.
-  assert {{ Γ, B[σ], A[q σ] ⊢ A[q σ∘Wk] ≈ A[q σ][Wk] }} by mauto 4.
-  assert {{ Γ, B[σ], A[q σ] ⊢s q σ∘Wk : Δ, B }} by mauto 3.
-  assert {{ Γ, B[σ], A[q σ] ⊢ #0 : A[q σ∘Wk] }} by mauto 3.
-  assert {{ Γ ⊢ B[σ]  }} by mauto 2.
-  assert {{ Γ, B[σ] ⊢s Wk : Γ }} by mauto 2.
-  assert {{ Γ, B[σ], A[q σ] ⊢s Wk : Γ, B[σ] }} by mauto 2.
-  assert {{ Γ, B[σ] ⊢ B[σ][Wk]  }} by mauto 2.
-  assert {{ Γ, B[σ], A[q σ] ⊢ B[σ][Wk][Wk]  }} by mauto 3.
-  assert {{ Γ, B[σ] ⊢ B[Wk][q σ] ≈ B[σ][Wk]  }} by (eapply typ_eq_sub_sub_compose_cong_typ; mauto 3).
-  assert {{ Γ, B[σ], A[q σ] ⊢ B[Wk][q σ∘Wk] ≈ B[σ][Wk][Wk]  }} by (transitivity {{{ B[Wk][q σ][Wk] }}}; mauto 3).
-  assert {{ Γ, B[σ], A[q σ] ⊢ #1[q (q σ)] ≈ #0[q σ∘Wk] : B[σ][Wk][Wk] }} by (econstructor; mauto).
-  assert {{ Γ, B[σ], A[q σ] ⊢ #0[q σ∘Wk] ≈ #0[q σ][Wk] : B[σ][Wk][Wk] }} by (econstructor; mauto).
-  assert {{ Γ, B[σ] ⊢s σ∘Wk : Δ }} by mauto 2.
-  assert {{ Γ, B[σ] ⊢ #0 : B[σ∘Wk] }} by mauto 3.
-  assert {{ Γ, B[σ] ⊢ #0[q σ] ≈ #0 : B[σ∘Wk] }} by mauto 3.
-  assert {{ Γ, B[σ], A[q σ] ⊢ #0[q σ][Wk] ≈ #0[Wk] : B[σ∘Wk][Wk] }} by mauto 4.
-  assert {{ Γ, B[σ], A[q σ] ⊢ B[σ∘Wk][Wk] ≈ B[σ][Wk][Wk]  }} by mauto 4.
-  assert {{ Γ, B[σ], A[q σ] ⊢ #0[q σ][Wk] ≈ #0[Wk] : B[σ][Wk][Wk] }} by mauto 4.
-  assert {{ Γ, B[σ], A[q σ] ⊢ #1[q (q σ)] ≈ #1 : B[σ][Wk][Wk] }} by (do 2 etransitivity; mauto 2).
-  assert {{ Γ, B[σ], A[q σ] ⊢s Wk∘Wk : Γ }} by mauto 2.
+  assert {{ Δ ⊢ Γ' }} by mauto 2.
+  assert {{ Δ ; Γ, B[σ] ⊢s q σ : Γ', B }} by mauto 2.
+  assert {{ Δ ⊢ Γ, B[σ] }} by mauto 3.
+  assert {{ Δ ⊢ Γ, B[σ], A[q σ] }} by mauto 3.
+  assert {{ Δ ; Γ', B ⊢ B[Wk]  }} by mauto 4.
+  assert {{ Δ ; Γ' ⊢ B }} by mauto 2.
+  assert {{ Δ ; Γ', B ⊢ #0 : B[Wk] }} by mauto 4.
+  assert {{ Δ ; Γ, B[σ] ⊢ A[q σ] }} by mauto 3.
+  assert {{ Δ ; Γ, B[σ], A[q σ] ⊢ #0 : A[q σ][Wk] }} by mauto 4.
+  assert {{ Δ ; Γ, B[σ], A[q σ] ⊢ A[q σ∘Wk] ≈ A[q σ][Wk] }} by mauto 4.
+  assert {{ Δ ; Γ, B[σ], A[q σ] ⊢s q σ∘Wk : Γ', B }} by mauto 3.
+  assert {{ Δ ; Γ, B[σ], A[q σ] ⊢ #0 : A[q σ∘Wk] }} by mauto 3.
+  assert {{ Δ ; Γ ⊢ B[σ]  }} by mauto 2.
+  assert {{ Δ ; Γ, B[σ] ⊢s Wk : Γ }} by mauto 2.
+  assert {{ Δ ; Γ, B[σ], A[q σ] ⊢s Wk : Γ, B[σ] }} by mauto 2.
+  assert {{ Δ ; Γ, B[σ] ⊢ B[σ][Wk]  }} by mauto 2.
+  assert {{ Δ ; Γ, B[σ], A[q σ] ⊢ B[σ][Wk][Wk] }} by mauto 3.
+  assert {{ Δ ; Γ, B[σ] ⊢ B[Wk][q σ] ≈ B[σ][Wk] }} by (eapply wf_typ_eq_sub_compose_cong; mauto 3).
+  assert {{ Δ ; Γ, B[σ], A[q σ] ⊢ B[Wk][q σ∘Wk] ≈ B[σ][Wk][Wk] }} by (transitivity {{{ B[Wk][q σ][Wk] }}}; mauto 3).
+  assert {{ Δ ; Γ, B[σ], A[q σ] ⊢ #1[q (q σ)] ≈ #0[q σ∘Wk] : B[σ][Wk][Wk] }} by (econstructor; mauto).
+  assert {{ Δ ; Γ, B[σ], A[q σ] ⊢ #0[q σ∘Wk] ≈ #0[q σ][Wk] : B[σ][Wk][Wk] }} by (econstructor; mauto).
+  assert {{ Δ ; Γ, B[σ] ⊢s σ∘Wk : Γ' }} by mauto 2.
+  assert {{ Δ ; Γ, B[σ] ⊢ #0 : B[σ∘Wk] }} by mauto 3.
+  assert {{ Δ ; Γ, B[σ] ⊢ #0[q σ] ≈ #0 : B[σ∘Wk] }} by mauto 3.
+  assert {{ Δ ; Γ, B[σ], A[q σ] ⊢ #0[q σ][Wk] ≈ #0[Wk] : B[σ∘Wk][Wk] }} by mauto 4.
+  assert {{ Δ ; Γ, B[σ], A[q σ] ⊢ B[σ∘Wk][Wk] ≈ B[σ][Wk][Wk]  }} by mauto 4.
+  assert {{ Δ ; Γ, B[σ], A[q σ] ⊢ #0[q σ][Wk] ≈ #0[Wk] : B[σ][Wk][Wk] }} by mauto 4.
+  assert {{ Δ ; Γ, B[σ], A[q σ] ⊢ #1[q (q σ)] ≈ #1 : B[σ][Wk][Wk] }} by (do 2 etransitivity; mauto 2).
+  assert {{ Δ ; Γ, B[σ], A[q σ] ⊢s Wk∘Wk : Γ }} by mauto 2.
   econstructor; mauto 4.
 Qed.
 
-
-(** Lemmas about judgments for types *)
-Lemma wf_typ_sub_cong {P} : forall {Γ : ctx P} {A},
-    {{ Γ ⊢ A }} ->
-    forall Δ σ τ,
-      {{ Δ ⊢s σ : Γ }} ->
-      {{ Δ ⊢s τ : Γ }} ->
-      {{ Δ ⊢s σ ≈ τ : Γ }} ->
-      {{ Δ ⊢ A[σ] ≈ A[τ] }}.
-Proof.
-  induction 1;
-    intros;
-    assert {{ ⊢ Δ }} by mauto 3.
-  - transitivity {{{ Sort@s }}}; mauto 3.
-  - assert {{ Δ ⊢ A[σ] ≈ A[τ]  }} by mauto 3.
-    mauto 3.
-  - transitivity {{{ A[σ∘σ0] }}}; mauto 3.
-    transitivity {{{ A[σ∘τ] }}}; mauto 3.
-    eapply IHwf_typ; mauto 3.
-Qed.
-
+#[export]
+Hint Resolve wf_exp_eq_var_1_sub_q_sigma : mcpts.
 
 (** *** Type Presuppositions *)
-
-Lemma presup_exp_typ {P : PtsSig} : forall {Γ : ctx P} {M A},
-    {{ Γ ⊢ M : A }} ->
-    {{ Γ ⊢ A }}.
+Lemma presup_wf_exp_typ {P : PtsSig} : forall {Δ : gctx P} {Γ M A},
+    {{ Δ ; Γ ⊢ M : A }} ->
+    {{ Δ ; Γ ⊢ A }}.
 Proof with mautosolve 3.
-  induction 1; assert {{ ⊢ Γ }} by mauto 3; destruct_conjs; mauto 3.
-  - enough {{ Γ ⊢s Id,,N : Γ, A }}...
-Qed.
+  induction 1; assert {{ Δ ⊢ Γ }} by mauto 3; destruct_conjs; mauto 3.
+  - enough {{ Δ ; Γ ⊢s Id,,N : Γ, A }}...
+  - assert {{ Δ ; ⋅ ⊢ A }} by mauto 3.
+    (* For this case, we need to weaken a closed type with applying a substitution, which is not obvious *)
+    admit.
+Admitted.
 
-Lemma presup_exp {P : PtsSig} : forall {Γ : ctx P} {M A},
-    {{ Γ ⊢ M : A }} ->
-    {{ ⊢ Γ }} /\ {{ Γ ⊢ A }}.
+Lemma presup_wf_exp {P : PtsSig} : forall {Δ : gctx P} {Γ M A},
+    {{ Δ ; Γ ⊢ M : A }} ->
+    {{ ⊢ Δ }} /\ {{ Δ ⊢ Γ }} /\ {{ Δ ; Γ ⊢ A }}.
 Proof.
-  mauto 4 using presup_exp_typ.
+  intros; repeat split; mauto 2 using presup_wf_exp_typ.
 Qed.
 
-
-(* Lemma presup_typ {P : PtsSig} : forall {Γ : ctx P} {A}, *)
-(*     {{ Γ ⊢ A }} -> *)
-(*     {{ ⊢ Γ }}. *)
-(* Proof. *)
-(*   intros *. *)
-(*   inversion_clear 1. *)
-(*   - eassumption. *)
-(*   - eapply presup_exp; mauto 2. *)
-(*   - eapply presup_typ_ctx; mauto 2. *)
-(* Qed. *)
   
 (** *** Consistency Helper *)
 
 Lemma no_closed_neutral {P : PtsSig} : forall {A : exp P} {W : ne P},
-    ~ {{ ⋅ ⊢ W : A }}.
+    ~ {{ ⋅ ; ⋅ ⊢ W : A }}.
 Proof.
   intros * H.
   dependent induction H; destruct W;
     try (simpl in *; congruence);
     autoinjections;
     intuition.
-  inversion_by_head (@ctx_lookup P).
+  - inversion_by_head (@ctx_lookup P).
+  - inversion_by_head (@gctx_lookup P).
 Qed.
 #[export]
 Hint Resolve no_closed_neutral : mcpts.
+
+
+
+
+
+
+
